AURORA CONSTRUCTION MATERIALS
AR2520 pre-mixed concrete
manufactured at
Rockbank
Programme: The International EPD® System www.environdec.com
Programme operator: EPD International AB
Regional Programme: EPD Australasia www.epd-australasia.com
EPD Registration no. EPD-IES-0021754:001
Version date: 2025-08-15
Valid until: 2030-08-15
EPD of a single product from a manufacturer (from one location)
An EPD may be updated or depublished if conditions change.
To find the latest version of the EPD and to confirm its validity, see www.environdec.com
Environmental Product Declaration
In accordance with ISO 14025:2006 and EN 15804:2012+A2:2019/AC:2021

-- 1 of 25 --

Contents
General information 1
Information about EPD owner 2
Product information 3
Technical compliance 3
Geographical scope 3
Content declaration 4
LCA information 5
Declared unit 5
Scope of the Environmental Product Declaration 5
Product stage (A1-A3) 7
End-of-life stage (C1-C4) 8
Resource recovery stage (D) 8
Background data 10
Data quality assessment 10
Cut-off criteria 11
Allocation 12
Key assumptions 12
Life cycle assessment (LCA) indicators 13
Environmental performance 15
Additional scenarios 19
Abbreviations 21
Version history 21
References 22
Contact information 23
Disclaimer
EPDs within the same product category but published in different EPD programmes, may not be comparable.
For two EPDs to be comparable, they shall be based on the same PCR (including the same first-digit version
number) or be based on fully-aligned PCRs or versions of PCRs; cover products with identical functions,
technical performances and use (e.g. identical declared/functional units); have identical scope in terms of
included life-cycle stages (unless the excluded life-cycle stage is demonstrated to be insignificant); apply
identical impact assessment methods (including the same version of characterisation factors); and be valid at
the time of comparison. For further information about comparability, see EN 15804 and ISO 14025.

-- 2 of 25 --

1
General information
An Environmental Product Declaration (EPD) is a standardised way of quantifying the potential environmental impacts
of a product or system. EPDs are produced according to a consistent set of rules – Product Category Rules (PCR) – that
define the requirements within a given product category. These rules are a key part of ISO 14025 as they enable
transparency and comparability between EPDs. This EPD is a “cradle-to-gate with modules C1-C4, D” declaration
covering production and end-of-life life cycle stages.
This EPD is verified to be compliant with EN 15804. EPDs of construction products may not be comparable if they do
not comply with EN15804. EPDs within the same product category but from different programs or utilising different
PCR documents may not be comparable, see the disclaimer on the previous page. Aurora Construction Materials
Epping Pty Ltd (Aurora), as the EPD owner, has the sole ownership, liability, and responsibility for the EPD.
EPD Program Operator
(Regional programme)
EPD Program Operator
EPD International AB
Box 210 60, SE-100 31
Stockholm, Sweden,
E-mail:
support@environdec.com
Regional programme
EPD Australasia Limited
Address: 6 Cube Court
Richmond 7020, New Zealand
Web: www.epd-australasia.com
Email: info@epd-australasia.com
EPD registration number: EPD-IES-0021754:001
Published: 2025-08-15 Valid until: 2030-08-15 (5 years)
Reference year for data: 2023-01-07 – 2024-06-30 (Note: the mix design is current at time of publication)
Product Category Rules (PCR) CEN standard EN 15804 served as the core Product Category Rules (PCR)
PCR: PCR 2019:14 Construction Products, Version 2.0.1, 2025-06-05 (valid until 2030-04-07)
PCR review was conducted by: The Technical Committee of the International EPD® System. See www.environdec.com for a
list of members. Review chair: Rob Rouwette | start2see (chair), Noa Meron | thinkstep-anz
(co-chair).
The review panel may be contacted via the Secretariat www.environdec.com/contact.
c-PCR c-PCR-003 (to 2019:14) Concrete and concrete elements, version 2025-04-08
Third-party verification: Independent third-party verification of the declaration and data, according to ISO 14025:2006,
via:
🗷 Individual EPD verification without a pre-verified LCA/EPD tool
Third party verifier:
Approved by EPD Australasia Ltd
Claudia A. Peña
PINDA LCT SpA
Email: pinda.lct@gmail.com
Procedure for follow-up of
data during EPD validity
involves third-party verifier:
☐ Yes
🗷 No

-- 3 of 25 --

2
Information about the EPD Owner
Aurora Construction Materials (Aurora) is a leading provider of sustainable aggregate, crushed rock
and concrete products to the civil construction, residential and commercial building segments
throughout Victoria.
Aurora’s ethos of ‘construction materials redefined’ seeks to capture our commitment to
sustainability, recycling and waste minimisation. We participate in the circular economy. Aurora
understands its environmental footprint and continuously finds ways to minimise it. Our
processes use excavated rock, recycled water and proprietary admixture technology to provide
valuable aggregate and concrete products with a reduced environmental footprint, compared to
virgin materials.
We are a 100% Australian owned business that directly employs over 100 staff and utilises the
services of over 300 local suppliers that support the local economies in which we operate.
We continue to look at alternative methods and products to improve our efficiency and reliance
on virgin materials.
Over the last 18 years Aurora and its partners have invested nearly $2M in developing a carbon
reduced alternative to traditional concrete, called ALTRA.
Aurora currently operates four sites around Melbourne, Victoria:
• Quarry and concrete operations at 335A O’Herns Road Epping, 3076
• Quarry and concrete operations at 2-50 Meskos Road, Rockbank, 3335
• Quarry operations at 61 Minton Street, Beveridge, 3753
• Concrete operations at 1470 Ballarto Road, Clyde, 3978.
Declaration Owner
Aurora Construction Materials Epping Pty. Ltd. (Aurora)
Suite 2 Level 1, 20 English Street
Essendon Fields, VIC, 3041-Australia
Web: www.acm.com.au
Email: orders@acm.com.au
Phone: +61 (03) 7037 5551
LCA Accountability:
start2see Pty Ltd
Unit 8, 2-4 Kensington Rd, South Yarra, VIC 3141
Web: www.start2see.com.au
Email: Rob.Rouwette@start2see.com.au

-- 4 of 25 --

3
Product information
Aurora specialises in manufacturing concrete and quarry materials, ranging in properties
depending on application and requirements.
Aurora has a full range of decorative and standard concrete (general and premium); see our
website for details.
• Concrete products consist of a mixture of cementitious binder, supplementary
cementitious materials, aggregates, natural sand, water and admixtures.
• Quarry products include aggregates, crushed rock and filling materials made from “waste
rock”.
This EPD covers AR2520 concrete manufactured by Aurora in Rockbank, Melbourne, Victoria. The
product included in this EPD, its strength grade, density and application are shown below.
Technical Compliance
Aurora concrete products comply with relevant technical specifications as per AS 1379:2007
“Specification and supply of concrete”.
Geographical scope
The processes in modules A1-A3 have been modelled to represent concrete production in
Rockbank, near Melbourne, Australia. The raw materials are sourced from within Australia, and the
end-of-life (module C) of the product has been modelled to represent Australia as well (based on
the default scenario).
Product code Strength grade Density Applications
AR2520 25MPa 2 270 kg/m3 General use concrete

-- 5 of 25 --

4
Content declaration
The product composition per declared unit (1 m3 of concrete) is presented in Table 1. For reasons
of confidentiality, a range is provided.
Table 1: Product content
Constituent Mass
(kg/m3)
Post-consumer
recycled
material,
mass %
Biogenic
material,
mass % of
product
Biogenic
material, kg C
/ declared
unit
Cement* 50 - 375 0% 0% 0
Ground granulated blast furnace slag † 30 - 300 0% 0% 0
Recycled aggregates† 750 - 1 000 0% 0% 0
Recycled manufactured sand† 0 - 300 0% 0% 0
Natural Sand † 450 - 950 0% 0% 0
Admixtures 0 - 70 0% 0% 0
Water 150 - 200 0% 0% 0
Total 2 270 kg/m3 0% 0% 0
* Aurora uses General Purpose cement. Cement contains traces of Chromium VI (hexavalent).
† Crystalline-silica (quartz) may be a constituent of sand, crushed stone, gravel, and blast furnace slag used in any
particular concrete mix.
In this LCA, slag is considered a secondary material.
The product, as supplied, is non-hazardous. The product included in this EPD does not contain
any substances of very high concern as defined by European REACH regulation* in concentrations
>0.1% (m/m). Dust from this product is classified as Hazardous according to the Approved
Criteria for Classifying Hazardous Substances 3rd Edition (NOHSC 2004). Concrete products are
classified as non-dangerous goods according to the Australian Code for the Transport of
Dangerous Goods by Road and Rail. When concrete products are cut, sawn, abraded or crushed,
dust is created which contains crystalline silica, some of which may be respirable (particles small
enough to go into the deep parts of the lung when breathed in), and which is hazardous.
Exposure through inhalation should be avoided.
The product code for pre-mix concrete is UN CPC 375 (Articles of concrete, cement and plaster)
and ANZSIC 20330 (Concrete – ready mixed – except dry mix).
* Regulation (EC) No 1907/2006 of the European Parliament and of the Council of 18 December 2006
concerning the Registration, Evaluation, Authorisation and Restriction of Chemicals.

-- 6 of 25 --

5
LCA information
Declared unit
1 cubic metre (m3) of Premixed concrete with a 25MPa strength grade and identifying
characteristics (as outlined in the Product information section). The declared unit is defined as the
quantity ordered by the client.
The conversion factor to mass is equal to the density of the concrete: 2 270 kg/m3.
Scope of the Environmental Product Declaration
This EPD covers the cradle-to-gate plus end-of-life life cycle stages (modules A1-A3, C1-C4, D).
Construction and use stages have not been included as we cannot define a typical scenario for
the range of Premixed concrete products. These impacts are best determined at project level.
The modules declared, geographical scope, share of specific data (in GWP-GHG indicator) and
data variation are shown in Table 2.
Table 2: Scope of this EPD
X = module is included in this study
ND = module is not declared. When a module is not accounted for, the stage is marked with “ND” (Not Declared).
ND is used when a typical scenario cannot be defined.
Stages Product
Stage
Construction
Stage Use Stage End-of-life Stage
Benefits
beyond
system
boundary
Raw Materials	
Transport	
Production	
Transport	
Installation	
Use	
Maintenance	
Repair
Replacement	
Refurbishment	
Operational energy use	
Operational water use	
Deconstruction/Demolition	
Transport	
Waste Processing	
Disposal
Reuse, recovery, recycling	
potential
Modules A1 A2 A3 A4 A5 B1 B2 B3 B4 B5 B6 B7 C1 C2 C3 C4 D
Scenario Scenario Scenario Scenario
Modules Declared X X X ND ND ND ND ND ND ND ND ND X X X X X
Geography AU,
GLO
AU AU AU AU AU AU AU
Share of primary
data 36%
Variation
products 0% (n/a)
Variation sites 0% (n/a)

-- 7 of 25 --

6
Figure 1 – System boundary diagram of premixed concrete products

-- 8 of 25 --

7
Product Stage (A1-A3)
Raw Materials – Module A1
Extraction and processing of raw materials results in environmental impacts from the use of
energy and resources, as well as from process emissions and waste.
• Cement is produced from clinker (made from limestone) and gypsum.
• Aggregates are produced by ACM from waste rock (spalls). Natural sand is extracted from
quarries.
• Supplementary Cementitious Materials (SCM): GGBFS (ground granulated blast furnace
slag) is a rest product from steel production.
• Admixtures are specialised chemical formulations that are typically produced by blending
selected ingredients.
Transportation – Module A2
Raw materials are typically transported from suppliers to our site via (articulated) trucks. Transport
of raw materials has been included in the LCA based upon actual transport modes and distances
relevant to the site.
Manufacturing – Module A3
Ready-mix concrete products are manufactured by mixing the raw materials in selected quantities
for each mix design.
The “Construction process stage” and “Use stage” have been excluded from the life cycle
assessment, as the ready-mix concrete can be used for a range of different applications for which
the use scenarios are unknown. The impacts of these stages are best determined at project level.

-- 9 of 25 --

8
End of life stage (C1-C4)
The end-of-life modules for pre-mix concrete are based on generic scenarios. The scenarios
included are currently in use and are representative for one of the most probable
alternatives.
Module C1 covers demolition of the concrete at the end of its service life. We have used the end-
of-life scenario representative for Victorian building & demolition materials based on the National
Waste Report 2022 (NWR 2022). This scenario implies that 84% of the concrete is recycled and
the remaining 16% of the concrete is sent to landfill. Additional (module C3, C4 and D) results for
alternative scenarios representing 100% recycling and 100% landfill are declared in Table 13 and
Table 14.
Module C2 comprises the transport from the demolition site to a recycling centre or landfill site
(80km). Module C3 encompasses the recycling process (i.e. crushing of concrete), while Module
C4 represents disposal of concrete in a landfill site. The concrete in module C3 reaches end-of-
waste status when it is crushed and stockpiled as “recycled crushed concrete” (RCC) aggregates.
We have used the default values from Table 4 in the PCR to model the end-of-life impacts for
concrete with a density of 2 270 kg/m3.
Due to high uncertainty in the parameters and lack of data, CO2‑uptake (carbonation) has not
been included at end-of-life.
Resource recovery stage (D)
Module D includes any benefits and loads from net flows leaving the product system (that have
passed the end-of-waste state). For this EPD, any material collected for recycling and processed in
Module C3, is considered to go through to Module D. We have assumed that Recycled Crushed
Concrete aggregates (the output of module C3) replace virgin aggregates (crushed rocks) in
module D.
Per cubic metre of concrete, module D credits the avoided impacts for 1 110 kg of crushed virgin
aggregates. The net flow calculation is not affected by SCMs or admixtures.
Table 3: End-of-life scenario parameters
Processes Quantity per
m3 of concrete Unit
Collection process specified by type 2 270
0
kg collected separately
kg collected with mixed construction waste
Transport from demolition site to
recovery / disposal sites 80 km transport
Recovery system specified by type
0
1 908
0
kg for re-use
kg for recycling
kg for energy recovery
Disposal to landfill 362 kg product or material for final deposition
Assumptions for scenario
development
The default values from PCR 2019:14 (v2.0.1) table 4 have been
used to model modules C1, C2, C3 and C4

-- 10 of 25 --

9
Table 4: Default data for modelling modules C1, C2, C3 and C4
Module and processes Quantity Energy carrier / transport means
C1: Demolition/deconstruction of
concrete/reinforced concrete 23 kWh/m3 diesel
C2: Transport (for products/materials not to
be incinerated) 80 km 16-32 tonne lorry (EURO 5)
C3: Loading and unloading at sorting facility
C3: Mechanical sorting
C3: Crushing of concrete
4.1 kWh/m3
5.0 kWh/m3
4.5 kWh/m3
diesel
electricity
diesel
C4: Compacting of inert construction waste
for landfills (including backfilling) 3.6 kWh/m3 diesel

-- 11 of 25 --

10
Background Data
Primary data covers the 2024 financial year and has been sourced from Aurora. Background data
is predominantly sourced from EPDs, AusLCI and the AusLCI shadow database. Data for cement
has been sourced from our supplier’s EPD (registration number S-P-05506) (Boral 2023). Data for
admixtures has been sourced from EPDs published by EFCA (EFCA 2021a, 2021b, 2021c, 2021d).
As a result, the vast majority of the environmental profile of our products is based on life cycle
data less than three years old. Background data used is less than 10 years old.
Methodological choices have been applied in line with EN 15804:2012+A2:2019; deviations have
been recorded.
Data quality assessment
Table 5: Data quality assessment
* The share of primary data is calculated based on GWP-GHG results. It is a simplified indicator for data
quality that supports the use of more primary data, to increase the representativeness of and comparability
between EPDs. Note that the indicator does not capture all relevant aspects of data quality and is not
comparable across product categories.
Process Source
type Source Reference
year
Data
category
Share of
primary data
(GWP-GHG;
A1-A3)
Manufacturing of concrete Collected
data
EPD owner 2024 Primary data 0-1%
Generation of electricity
used in manufacturing of
concrete
Database AusLCI v1.42 2023 Primary data 0-1%
Transport of raw materials
to manufacturing site
Database EPD owner 2024 Primary data 1-8%
Production of GP cement EPD Supplier EPD 2023 Primary data,
Secondary
data
4-9%
Production of GGBFS EPD Supplier EPD 2023 Primary data,
Secondary
data
2-25%
Production of recycled
aggregates and
manufactured sand
Collected
data
EPD owner 2024 Primary data 1-3%
Admixtures EPD EFCA EPDs 2021 Proxy data 0%
Other Database AusLCI v1.42 2023 Secondary
data
0%
Total share of primary data*, of GWP-GHG results for A1-A3 36%

-- 12 of 25 --

11
The EPD covers pre-mixed concrete from one plant in Rockbank, which provided energy and
waste data for the concrete plant for the period July 2023 - June 2024. The mix designs, raw
materials, and supply chain details are current (August 2025). The ingredients are mixed in the
batching plant and sent to the customer as wet concrete. The EPD covers end-of-life in Australia,
although the default factors from the PCR are used to model module C (see Table 4). Background
data was sourced from EPDs and the AusLCI v1.42 database. Data quality was assessed according
to EN 15804:2012+A2:2019, Annex E (Table E.1 - UN Environment Global Guidance on LCA
database development). The use of very poor and poor data is disclosed in Table 6, together with
fair data with more than 30% of impact on any core indicator.
Table 6: Data quality information
Cut-off criteria
• The cut-off criteria applied are 1% of renewable and non-renewable primary energy usage,
1% of the total mass input of a process and 1% of environmental impacts.
• The contribution of capital goods (production equipment and infrastructure) and personnel is
excluded, as these processes are non-attributable and they contribute less than 10% to
GWP‑GHG.
Data set Criteria Data
quality
level
Reason for
level
Reason for
using
Relevance
Production of
admixtures
Geographical
Technical
Fair to
good
Very poor
to Fair
Proxy or
Generic
background
data
Best available
data
30-60% of ADPm&m
0-10% of other core
impact indicators

-- 13 of 25 --

12
Allocation
The key processes that require allocation are:
• Production of concrete mixes: All shared processes are attributed to concrete products based
on their volume.
• Blast Furnace Slag (BFS): BFS is a by-product from steelmaking. The supplier EPD used the
AusLCI data for BFS ('Blast Furnace Slag allocation, at steel plant / AU U'), which contain
impacts from pig iron production allocated to blast furnace slag using economic allocation.
One tonne of slag equals the environmental impact of 0.0127 tonnes of pig iron. Drying and
milling of slag is included in the supplier EPD based on their processes.
• Recycled aggregates, manufactured sand: Recycled aggregates and manufactured sand are
obtained by processing rock spalls. The rock spalls are unwanted material that is removed
from local construction projects and delivered to Aurora’s “quarries”. The disposing party
pays Aurora for acceptance of this material. The end-of-waste state is therefore attained
after the spalls are crushed and graded by size, at which point they fulfill the end-of-waste
criteria. Crushing and grading of spalls is assigned to the disposing life cycle in line with the
polluter-pays principle. The secondary materials are modelled with 50% of the diesel use of
Aurora’s “quarry” site. (The other 50% is attributed to handling of incoming material – before
the end-of-waste state is reached.)
Allocation approaches may have a material effect on concrete products containing ground
granulated blast furnace slag and recycled aggregates.
Key assumptions
• The concrete composition is provided by Aurora and has been accepted as is.
• Cement and admixture data are taken from supplier-specific and generic EPDs. This is
expected to greatly improve the accuracy of Aurora’s EPD results.
• Additional environmental impact indicators are not declared in the admixture EPDs, which
results in underreporting of these indicators.
• Allocation approaches may have a material effect on concrete products containing ground
granulated blast furnace slag and recycled aggregates.
• For core processes, electricity has been modelled using adjusted AusLCI data to represent the
estimated residual electricity grid mix in Victoria, Australia. This is done by removing
renewables from the Australian Energy Statistics 2024 data (Table O3). The GWP-GHG of the
electricity is 1.00 kg CO2e / kWh. The proxy residual grid mix is made up of brown coal
(94.2%), natural gas (5.1%), and oil products (0.8%). Given the low contribution of electricity
consumption to the GWP emissions, the selection of the electricity grid mix does not have a
material impact on the results.
• For other processes, electricity has been modelled using a location-based approach, mostly
based on Australian average electricity generation as per AusLCI.
• The end-of-life scenario is based on landfill and recycling rates for building and demolition
materials in Victoria, as per the National Waste Report 2022 (NWR 2022), table 37.
• A minor amount of biogenic carbon may be present in admixtures. The proxy admixture data
show a negative GWP-biogenic value, which ends up in module A1-A3 of our concrete EPD.
Although any biogenic matter in the admixtures would be bound in the concrete matrix, it is
release in module C3 as per the PCR requirements.

-- 14 of 25 --

13
Life Cycle Assessment (LCA) indicators
An LCA serves as the foundation for this EPD. An LCA analyses the production systems of a
product. It provides comprehensive evaluations of all upstream and downstream energy inputs
and outputs. The results are provided in a form which covers a range of environmental impact
categories.
Table 7: Environmental indicators legend (EN 15804+A2)
1 The results of this environmental impact indicator shall be used with care as the uncertainties on these results are high or as
there is limited experience with the indicator.
2 This impact category deals mainly with the eventual impact of low dose ionizing radiation on human health of the nuclear
fuel cycle. It does not consider effects due to possible nuclear accidents, occupational exposure nor due to radioactive waste
disposal in underground facilities. Potential ionizing radiation from the soil, from radon and some construction materials, is
also not measured by this indicator.
3 Note regarding various GWP indicators: GWP-total is calculated using the European Union’s Joint Research Centre’s
characterisation factors (CFs) based on the “EF 3.1 package” for CFs to be used in the EU’s Product Environmental Footprint
(PEF) framework. CFs listed by JRC are based on the IPCC AR6 method (IPCC 2021) and include indirect radiative forcing, which
results in higher numerical Global Warming Potential (GWP) values than the CFs in the internationally accepted (IPCC 2013).
The GWP-GHG indicator is identical to GWP-total except that the CFs for biogenic CO2 are set to zero. The GWP-GHG
indicator in PCR 2019:14 v2.0.1 differs from the GWP-GHG in earlier (pre v1.3) PCR 2019:14 versions. The “GWP-GHG (IPCC
AR5)” indicator is determined using the IPCC AR5 GWPs with a 100-year time horizon (IPCC 2013). This indicator is aligned
with Australia’s greenhouse gas reporting frameworks.
Core indicators Acronym Unit
Climate change – total GWP-total kg CO2 equivalent
Climate change – fossil GWP-fossil kg CO2 equivalent
Climate change – biogenic GWP-biogenic kg CO2 equivalent
Climate change – land use and land use change GWP-luluc kg CO2 equivalent
Ozone layer depletion ODP kg CFC-11 equivalent
Acidification AP mol H+ equivalent
Eutrophication aquatic freshwater EP-freshwater kg P equivalent
Eutrophication aquatic marine EP-marine kg N equivalent
Eutrophication terrestrial EP-terrestrial mol N equivalent
Photochemical ozone formation POCP kg NMVOC equivalent
Abiotic depletion potential – elements1 ADP minerals & metals kg Sb equivalent
Abiotic depletion potential – fossil fuels1 ADP fossil MJ, net calorific value
Water use1 WDP m3 world equivalent deprived
Additional indicators Acronym Unit
Global Warming Potential – Greenhouse gases GWP-GHG kg CO2 equivalent
Particulate matter emissions PM disease incidence
Ionising radiation, human health2 IRP kBq U235 equivalent
Ecotoxicity (freshwater)1 ETP-fw CTUe
Human toxicity, cancer effects1 HTP-c CTUh
Human toxicity, non-cancer effects1 HTP-nc CTUh
Land use related impacts / soil quality1 SQP - (dimensionless)
Additional GHG indicator Acronym Unit
Carbon footprint in line with IPCC AR53 GWP-GHG (IPCC AR5) kg CO2 eq

-- 15 of 25 --

14
Table 8: Legend for parameters describing resource use, waste and output flows
Table 9: Legend for EN 15804+A1 indicators
Indicator Acronym Unit
Global warming potential GWP kg CO2 equivalent
Ozone layer depletion potential ODP kg CFC-11 equivalent
Acidification potential AP kg SO2 equivalent
Eutrophication potential EP kg PO43- equivalent
Photochemical oxidation (Photochemical ozone creation) potential POCP kg ethylene equivalent
Abiotic depletion potential - elements ADPE kg Sb equivalent
Abiotic depletion potential – fossil fuels ADPF MJNCV
Parameter Acronym Unit
Parameters describing resource use
Use of renewable primary energy excluding renewable primary energy resources used as
raw materials
PERE MJNCV
Use of renewable primary energy resources used as raw materials PERM MJNCV
Total use of renewable primary energy resources PERT MJNCV
Use of non-renewable primary energy excluding non-renewable primary energy
resources used as raw materials
PENRE MJNCV
Use of non-renewable primary energy resources used as raw materials PENRM MJNCV
Total use of non-renewable primary energy resources PENRT MJNCV
Use of secondary material SM kg
Use of renewable secondary fuels RSF MJNCV
Use of non-renewable secondary fuels NRSF MJNCV
Use of net fresh water FW m3
Waste categories
Hazardous waste disposed HWD kg
Non-Hazardous waste disposed NHWD kg
Radioactive waste disposed RWD kg
Output flows
Components for re-use CRU kg
Materials for recycling MFR kg
Materials for energy recovery MER kg
Exported energy EE MJ

-- 16 of 25 --

15
Environmental performance
The following section presents the results for each Life Cycle Assessment module.
The results have been calculated using Simapro software v9.6.0.1, using characterisation factors
based on the “EF 3.1 package” for characterisation factors to be used in the EU’s Product
Environmental Footprint (PEF) framework.
Water flows have been disaggregated using the 36 ALCAS water catchments for which
characterisation factors are available for both Pfister WSI and the AWARE method.
To separate the use of primary energy into energy used as raw material and energy used as
energy carrier, Option B from Annex 3 of PCR 2019:14 has been applied.
Please consider the following mandatory statements when interpreting the results:
”The estimated impact results are only relative statements, which do not indicate the end-
points of the impact categories, exceeding threshold values, safety margins and/or risks”.
“
The results of the end-of-life stage (modules C1-C4) should be considered when using the results
of the product stage (modules A1-A3).”

-- 17 of 25 --

16
Table 10: Environmental indicators EN 15804+A2, AR2520, per m3
Environmental
Indicator Unit Module A1-A3 Module C1 Module C2 Module C3 Module C4 Module D
Core Indicators
GWP-total kg CO2-eq. 1.40E+02 1.20E+01 1.45E+01 8.03E+00 8.61E-01 -9.79E+00
GWP-fossil kg CO2-eq. 1.40E+02 1.20E+01 1.45E+01 7.82E+00 8.61E-01 -9.77E+00
GWP-biogenic kg CO2-eq. -2.40E-01 7.97E-04 8.98E-04 2.09E-01 6.95E-05 -1.92E-02
GWP-luluc kg CO2-eq. 1.19E-02 5.76E-06 6.86E-06 3.63E-06 4.18E-07 -1.51E-06
ODP kg CFC11-eq. 6.09E-06 1.92E-06 2.29E-06 9.88E-07 1.41E-07 -3.34E-07
AP mol H+ eq. 1.01E+00 1.32E-01 1.28E-01 2.15E-02 2.06E-03 -3.57E-02
EP-freshwater kg P eq. 5.14E-04 1.60E-06 8.73E-07 5.80E-06 1.17E-07 -7.03E-06
EP-marine kg N eq. 1.85E-01 5.75E-02 4.02E-02 3.83E-03 3.71E-04 -5.98E-03
EP-terrestrial mol N eq. 2.05E+00 6.31E-01 4.40E-01 4.18E-02 4.05E-03 -6.48E-02
POCP kg NMVOC eq. 5.15E-01 1.68E-01 1.07E-01 1.12E-02 1.09E-03 -1.70E-02
ADP minerals &
metals1 kg Sb eq. 3.35E-06 1.42E-08 1.69E-08 1.94E-06 1.01E-09 -1.43E-06
ADP fossil1 MJ (NCV) 1.20E+03 1.68E+02 2.00E+02 1.12E+02 1.23E+01 -1.40E+02
WDP1 m³ world eq.
deprived 5.32E+02 1.06E+00 1.26E+00 1.14E+00 7.74E-02 -6.53E+01
Additional indicators
GWP-GHG kg CO2-eq. 1.39E+02 1.20E+01 1.45E+01 7.83E+00 8.61E-01 -9.79E+00
PM Disease incidence 6.83E-06 3.50E-06 7.18E-07 1.43E-07 1.09E-08 -2.99E-07
IRP2 kBq U235 eq. 3.21E-01 2.45E-04 2.91E-04 1.58E-03 1.78E-05 -8.89E-04
ETP-fw1 CTUe 4.83E+02 3.72E+01 4.41E+01 1.93E+01 2.67E+00 -6.70E+00
HTP-c1 CTUh 3.19E-08 4.65E-10 6.23E-11 1.64E-10 6.81E-12 -4.25E-10
HTP-nc1 CTUh 5.57E-07 2.48E-09 1.19E-09 1.07E-09 8.23E-11 -2.68E-09
SQP1 - 2.68E+02 8.05E-01 8.96E-01 2.12E+04 2.03E+01 -2.01E+02
Carbon footprint
GWP-GHG (IPCC AR5) kg CO2 eq 139 12.0 14.5 7.83 0.861 -9.8

-- 18 of 25 --

17
1 The results of this environmental impact indicator shall be used with care as the uncertainties on these results are high or as there is limited experience with the indicator.
2 This impact category deals mainly with the eventual impact of low dose ionizing radiation on human health of the nuclear fuel cycle. It does not consider effects due to possible nuclear accidents,
occupational exposure nor due to radioactive waste disposal in underground facilities. Potential ionizing radiation from the soil, from radon and some construction materials, is also not measured
by this indicator.
Table 11: EN 15804+A2 parameters, AR2520, per m3
Parameter Unit Module A1-A3 Module C1 Module C2 Module C3 Module C4 Module D
PERE MJNCV 3.38E+01 2.60E-01 2.86E-01 1.93E+00 2.40E-02 -5.38E+00
PERM MJNCV 2.89E-01 0.00E+00 0.00E+00 -2.43E-01 0.00E+00 0.00E+00
PERT MJNCV 3.41E+01 2.60E-01 2.86E-01 1.69E+00 2.40E-02 -5.38E+00
PENRE MJNCV 1.20E+03 1.68E+02 2.00E+02 1.12E+02 1.23E+01 -9.43E+01
PENRM MJNCV 1.33E+00 0.00E+00 0.00E+00 -1.11E+00 0.00E+00 0.00E+00
PENRT MJNCV 1.20E+03 1.67E+02 2.00E+02 1.11E+02 1.23E+01 -9.43E+01
SM kg 1.38E+03 0.00E+00 0.00E+00 0.00E+00 0.00E+00 0.00E+00
RSF MJNCV 3.19E+00 0.00E+00 0.00E+00 0.00E+00 0.00E+00 0.00E+00
NRSF MJNCV 0.00E+00 0.00E+00 0.00E+00 0.00E+00 0.00E+00 0.00E+00
FW m3 2.02E+00 2.43E-02 2.89E-02 3.97E-02 1.78E-03 -1.03E+00
HWD kg 6.84E-06 0.00E+00 0.00E+00 0.00E+00 0.00E+00 0.00E+00
NHWD kg 1.04E+00 7.69E-04 8.47E-04 5.46E-03 3.63E+02 -1.59E-02
RWD kg 2.00E-03 0.00E+00 0.00E+00 0.00E+00 0.00E+00 0.00E+00
CRU kg 0.00E+00 0.00E+00 0.00E+00 0.00E+00 0.00E+00 0.00E+00
MFR kg 2.23E+01 0.00E+00 0.00E+00 1.91E+03 0.00E+00 0.00E+00
MER kg 0.00E+00 0.00E+00 0.00E+00 0.00E+00 0.00E+00 0.00E+00
EE MJ 0.00E+00 0.00E+00 0.00E+00 0.00E+00 0.00E+00 0.00E+00

-- 19 of 25 --

18
Table 12: EN 15804+A1 indicators*, AR2520, per m3
* Note: the indicators and characterisation methods are from EN 15804:2012+A1:2013, but other LCA rules (system boundaries, allocation, etc.) are according to EN 15804:2012+A2:2019; i.e., the
results of the “A1 indicators” shall not be claimed to be compliant with EN 15804:2012+A1:2013.
Environmental Indicator Unit Module A1-A3 Module C1 Module C2 Module C3 Module C4 Module D
GWP kg CO2 eq 1.39E+02 1.20E+01 1.45E+01 7.81E+00 8.59E-01 -6.56E+00
ODP kg CFC11 eq 4.83E-06 1.52E-06 1.81E-06 7.81E-07 1.11E-07 -1.78E-07
AP kg SO2 eq 6.12E-01 9.39E-02 7.07E-02 1.36E-02 1.65E-03 -7.57E-03
EP kg PO43- eq 7.19E-02 1.93E-02 1.35E-02 1.33E-03 1.27E-04 -1.40E-03
POCP kg C2H4 eq 3.50E-02 9.21E-03 4.57E-03 7.60E-04 8.24E-05 -5.22E-04
ADPE kg Sb eq 1.12E-05 1.44E-08 1.71E-08 1.94E-06 1.03E-09 -9.70E-07
ADPF MJNCV 1.20E+03 1.68E+02 2.00E+02 1.12E+02 1.23E+01 -9.43E+01

-- 20 of 25 --

19
Additional scenarios
Table 13: Environmental indicators EN 15804+A2, 100% end-of-life scenarios, AR2520, per m3
Environmental
Indicator Unit Module C3 Module C4 Module D Module C3 Module C4 Module D
Core Indicators 100% recycling 100% landfill
GWP-total kg CO2-eq. 6.56E+00 0.00E+00 -9.79E+00 0.00E+00 1.13E+00 2.32E+01
GWP-fossil kg CO2-eq. 6.55E+00 0.00E+00 -9.77E+00 0.00E+00 1.13E+00 2.32E+01
GWP-biogenic kg CO2-eq. 8.74E-03 0.00E+00 -1.92E-02 0.00E+00 7.51E-05 4.56E-02
GWP-luluc kg CO2-eq. 1.40E-06 0.00E+00 -1.51E-06 0.00E+00 5.42E-07 3.57E-06
ODP kg CFC11-eq. 4.36E-07 0.00E+00 -3.34E-07 0.00E+00 1.81E-07 7.92E-07
AP mol H+ eq. 4.47E-02 0.00E+00 -3.57E-02 0.00E+00 1.24E-02 8.47E-02
EP-freshwater kg P eq. 2.52E-06 0.00E+00 -7.03E-06 0.00E+00 1.51E-07 1.67E-05
EP-marine kg N eq. 1.54E-02 0.00E+00 -5.98E-03 0.00E+00 5.41E-03 1.42E-02
EP-terrestrial mol N eq. 1.68E-01 0.00E+00 -6.48E-02 0.00E+00 5.94E-02 1.54E-01
POCP kg NMVOC eq. 4.47E-02 0.00E+00 -1.70E-02 0.00E+00 1.58E-02 4.03E-02
ADP minerals &
metals1 kg Sb eq. 3.31E-09 0.00E+00 -1.43E-06 0.00E+00 1.33E-09 3.40E-06
ADP fossil1 MJ (NCV) 9.31E+01 0.00E+00 -1.40E+02 0.00E+00 1.58E+01 3.32E+02
WDP1 m³ world eq.
deprived 4.67E-01 0.00E+00 -6.53E+01 0.00E+00 9.99E-02 1.55E+02
Additional indicators 100% recycling 100% landfill
GWP-GHG kg CO2-eq. 6.56E+00 0.00E+00 -9.79E+00 0.00E+00 1.13E+00 2.32E+01
PM Disease incidence 9.12E-07 0.00E+00 -2.99E-07 0.00E+00 3.29E-07 7.09E-07
IRP2 kBq U235 eq. 5.73E-05 0.00E+00 -8.89E-04 0.00E+00 2.31E-05 2.11E-03
ETP-fw1 CTUe 8.78E+00 0.00E+00 -6.70E+00 0.00E+00 3.50E+00 1.59E+01
HTP-c1 CTUh 2.98E-10 0.00E+00 -4.25E-10 0.00E+00 4.38E-11 1.01E-09
HTP-nc1 CTUh 1.74E-09 0.00E+00 -2.68E-09 0.00E+00 2.33E-10 6.37E-09
SQP1 - 1.07E+01 0.00E+00 -2.01E+02 0.00E+00 7.58E-02 4.77E+02
Carbon footprint 100% recycling 100% landfill
GWP-GHG (IPCC AR5) kg CO2 eq 6.56E+00 0.00E+00 -9.79E+00 0.00E+00 1.13E+00 2.32E+01

-- 21 of 25 --

20
Table 14: EN 15804+A2 parameters, 100% end-of-life scenarios, AR2520, per m3
Parameter Unit Module C3 Module C4 Module D Module C3 Module C4 Module D
100% recycling 100% landfill
PERE MJNCV 3.95E+00 0.00E+00 -6.71E+00 0.00E+00 2.44E-02 7.01E+00
PERM MJNCV -2.89E-01 0.00E+00 0.00E+00 0.00E+00 0.00E+00 0.00E+00
PERT MJNCV 3.66E+00 0.00E+00 -6.71E+00 0.00E+00 2.44E-02 7.01E+00
PENRE MJNCV 9.31E+01 0.00E+00 -1.18E+02 0.00E+00 1.58E+01 1.23E+02
PENRM MJNCV -1.33E+00 0.00E+00 0.00E+00 0.00E+00 0.00E+00 0.00E+00
PENRT MJNCV 9.17E+01 0.00E+00 -1.18E+02 0.00E+00 1.58E+01 1.23E+02
SM kg 0.00E+00 0.00E+00 0.00E+00 0.00E+00 0.00E+00 0.00E+00
RSF MJNCV 0.00E+00 0.00E+00 0.00E+00 0.00E+00 0.00E+00 0.00E+00
NRSF MJNCV 0.00E+00 0.00E+00 0.00E+00 0.00E+00 0.00E+00 0.00E+00
FW m3 1.31E-02 0.00E+00 -1.29E+00 0.00E+00 2.29E-03 1.34E+00
HWD kg 0.00E+00 0.00E+00 0.00E+00 0.00E+00 0.00E+00 0.00E+00
NHWD kg 1.17E-02 0.00E+00 -1.98E-02 0.00E+00 2.27E+03 2.07E-02
RWD kg 0.00E+00 0.00E+00 0.00E+00 0.00E+00 0.00E+00 0.00E+00
CRU kg 0.00E+00 0.00E+00 0.00E+00 0.00E+00 0.00E+00 0.00E+00
MFR kg 2.27E+03 0.00E+00 0.00E+00 0.00E+00 0.00E+00 0.00E+00
MER kg 0.00E+00 0.00E+00 0.00E+00 0.00E+00 0.00E+00 0.00E+00
EE MJ 0.00E+00 0.00E+00 0.00E+00 0.00E+00 0.00E+00 7.71E+00

-- 22 of 25 --

21
Abbreviations
Abbreviation Definition
AusLCI Australian Life Cycle Inventory (database)
BFS / GGBFS blast furnace slag / ground granulated blast furnace slag
CEN European Committee for Standardization
CPC Central Product Classification
EF Environmental Footprint
EFCA European Federation of Concrete Admixtures Associations
EN European Norm (Standard)
EPD Environmental Product Declaration
GPI General Programme Instructions
ISO International Organization for Standardization
kg kilogram
km kilometre
kWh kilo Watt hour
LCA Life Cycle Assessment
m3 cubic metre
ND Not Declared
NWR National Waste Report
OHS Operational Health and Safety
PCR / c-PCR Product Category Rules / complimentary Product Category Rules
SCM Supplementary Cementitious Materials
SVHC Substances of Very High Concern
t tonne
UN United Nations
Version history
Version Notes
1 Original version of the EPD, published 2025-08-15

-- 23 of 25 --

22
References
AS 1379 Specification and supply of concrete, prepared by Committee BD-049 Manufacture of
Concrete, published on 20 September 2007 by Standards Australia, Sydney
AusLCI 2023 Australian Life Cycle Inventory database v1.42 published by the Australian Life Cycle
Assessment Society, 2023
Boral 2023 EPD of Victorian Bulk Cement and Cementitious Products (Geographical scope: Victoria),
EPD Australasia. EPD Declaration number S-P-05506, issued 2023-05-20 (version 1.0),
based on EN 15804+A2, PCR 2019:14 (v1.11) and c-PCR-001; EPD owner: Boral.
c-PCR-003 c-PCR-003 Concrete and concrete elements (EN 16757:2022), Product category rules for
concrete and concrete elements, version 8 April 2025
ECHA 2025 European Chemicals Association, Candidate List of substances of very high concern for
Authorisation, published in accordance with Article 59(10) of the REACH Regulation,
Helsinki | Accessed on 1 June 2025 from: https://echa.europa.eu/candidate-list-table
EFCA 2021a EPD of Air entrainers, IBU EPD Declaration number EPD-EFC-20210193-IBG1-EN, issued
2021-12-16, based on EN 15804 and PCR for concrete admixtures; EPD owner: EFCA -
European Federation of Concrete Admixtures Associations
EFCA 2021b EPD of Set Accelerators, IBU EPD Declaration number EPD-EFC-20210194-IBG1-EN, issued
2021-12-16, based on EN 15804 and PCR for concrete admixtures; EPD owner: EFCA -
European Federation of Concrete Admixtures Associations
EFCA 2021c EPD of Retarders, IBU EPD Declaration number EPD-EFC-20210195-IBG1-EN, issued 2021-
12-16, based on EN 15804 and PCR for concrete admixtures; EPD owner: EFCA - European
Federation of Concrete Admixtures Associations
EFCA 2021d EPD of Plasticizer and superplasticizer, IBU EPD Declaration number EPD-EFC-20210198-
IBG2-EN, issued 2021-12-16, based on EN 15804 and PCR for concrete admixtures; EPD
owner: EFCA - European Federation of Concrete Admixtures Associations
Environdec
2025
International EPD System, General Programme Instructions for the International EPD
System, Version 5.0.1, 27 February 2025
EN 15804+A2 EN 15804:2012+A2:2019/AC:2021, Sustainability of construction works – Environmental
product declarations – Core rules for the product category of construction products,
European Committee for Standardization (CEN), Brussels, August 2021
EN 15804+A1 EN 15804:2012+A1:2013, Sustainability of construction works – Environmental product
declarations – Core rules for the product category of construction products, European
Committee for Standardization (CEN), Brussels, November 2013
EN 16757 EN 16757:2022, Sustainability of construction works – Environmental product declarations
- Product Category Rules for concrete and concrete elements, European Committee for
Standardization (CEN), Brussels, October 2022
ISO 14025 Environmental labels and declarations - Type III environmental declarations - Principles
and procedures. International Organization for Standardization, Geneva, Switzerland, 2006
ISO 14040 Environmental management - Life cycle assessment - Principles and framework.
International Organization for Standardization, Geneva, Switzerland, 2006
ISO 14044 Environmental management - Life cycle assessment - Requirements and guidelines.
International Organization for Standardization, Geneva, Switzerland, 2006
NOHSC 2004 Australian Government, National Occupational Health and Safety Commission (NOHSC),
Approved Criteria for Classifying Hazardous Substances, 3rd Edition, October 2004
NWR 2022 Blue Environment, National Waste Report 2022, prepared for The Department of Climate
Change, Energy, the Environment and Water, Final version 1.2, 16 December 2022
(updated 10 February 2023)
PCR 2019:14 Product category rules for Construction products (EN 15804:2012+A2:2019), registration
number 2019:14, version 2.0.1, published on 5 June 2025.

-- 24 of 25 --

23
Contact information
This publication provides general information only and is no substitute for professional engineering advice. No
representations or warranties are made regarding the accuracy, completeness or relevance of the information
provided. Users must make their own determination as to the suitability of this information or any Aurora product
for their specific circumstances.
Aurora accepts no liability for any loss or damage resulting from any reliance on the information provided in this
publication.
©August 2025 Aurora Construction Materials Epping Pty Ltd (Aurora) ABN 61 605 039 254. All rights reserved.
We are a 100% Australian owned business.
We directly employ over 100 staff and utilise the services of over 300
local suppliers that support the local economies in which we operate.
Suite 2 Level 1, 20 English Street
Essendon Fields, VIC 3041
13 22 61 (13 ACM 1)
orders@acm.com.au

-- 25 of 25 --

