READY-MIX CONCRETE
Environmental Product Declaration (EPD)
QLD - Brisbane - ECOPact - QE252M100 - S25/20/100 Ecopact Concrete - General
use
An EPD may be updated or depublished if conditions
change. To find the latest version for the EPD and to
confirm its validity, see www.environdec.com.
In accordance with ISO 14025 and EN15804:2012+A2:2019/AC:2021
Programme: International EPD System | www.environdec.com
Programme operator: EPD International AB
Regional Programme: EPD Australasia | www.epd-australasia.com
Managed by: Holcim Certified EPD Process
EPD Process Certificate Number: 04
Accreditation Body: Epsten Group, Inc.
EPD Registration No.: EPD-IES-0029695:001
Valid from: 15/4/2026 | 15/4/2031
Revision Date: 15/4/2026
Revision Number: 1
EPD Process Geographical Scope: Australia

-- 1 of 21 --

Programme-related information and verification
EPD Owner
Evan Smith
Holcim (Australia) Pty Ltd
Level 40, Northpoint Tower, 100 Miller St, North
Sydney NSW 2060, Australia
Web: www.holcim.com.au
Phone: +61 2 9412 6600
Programme Operator
EPD International AB
Box 210 60, SE-100 31
Stockholm, Sweden
Web: www.environdec.com
E-mail: support@environdec.com
Regional Programme Operator
EPD Australasia Limited
6 Cube Court, Richmond, 7020 New Zealand
Web: www.epd-australasia.com
Email: info@epd-australasia.com
Phone: +61 2 8005 8206
EPD Produced by
Jonas Bengtsson, Sazal Kundu & Weiqi Xing
Edge Environment Pty Ltd
Level 3, Greenhouse, 180 George Street,
Sydney NSW 2000 Australia
Web: www.edgeimpact.global
Phone: +61 2 9438 0100
EPD Process Certified by
Epsten Group
Suite 2600, 101 Marietta St NW, Atlanta,
Georgia 30303, USA
Web: www.epstengroup.com
Approved by: EPD Australasia
EPD Registration Number EPD-IES-0029695:001
Valid From 15/4/2026
Revision Number 1
Valid Until 15/4/2031
Product group classification UN CPC 375 (Articles of concrete, cement and plaster)
Geographical Scope Australia
Reference Year for Data 2022 Plant Data, 2026 Mix/Materials Data
CEN standard EN 15804:2012+A2:2019/AC:2021 serves as the core Product Category Rules (PCR)
Product category rules PCR 2019:14 Construction Products, Version 2.0.1, 2025-06-05
c-PCR-003 Concrete and Concrete Elements, 2025-04-08
PCR review was conducted by
The Technical Committee of the International EPD System. A full list of members is
available on www.environdec.com
Review chair: Claudia A. Peña, University of Concepción, Chile. The review panel may
be contacted via the Secretariat www.environdec.com/contact
Independent third-party
verification of the declaration
and data, according to ISO
14025:2006:
☒ EPD process certification* without a pre-verified LCA/EPD tool
* EPD process certification involves an accredited certification body certifying and
periodically auditing the EPD process and conducting external and independent verification
of EPDs that are regularly published. More information can be found in the General
Programme Instructions on www.envrondec.com.
Process certification
Epsten Group, Inc., Megan Blizzard, is an approved
certification body accountable for third-party verification.
Third-party verifier is accredited by: A2LA, Certificate
#3142.03
Procedure for follow-up of data
during EPD validity involves
third party verifier:
☐ Yes
☒ No
Programme-related information and verification:
The EPD owner has the sole ownership, liability, and responsibility for the EPD. EPDs within the same product category but published in different
EPD programmes, may not be comparable. For two EPDs to be comparable, they shall be based on the same PCR (including the same first-digit
version number) or be based on fully aligned PCRs or versions of PCRs; cover products with identical functions, technical performances and use
(e.g. identical declared/functional units); have identical scope in terms of included life-cycle stages (unless the excluded life-cycle stage is
demonstrated to be insignificant); apply identical impact assessment methods (including the same version of characterisation factors); and be valid
at the time of comparison. For further information about comparability, see EN 15804 and ISO 14025.
Holcim - Ready-Mix Concrete - EPD 2

-- 2 of 21 --

TABLE OF CONTENTS
Introduction 5
About Holcim 5
A first for ready-mix concrete in Australia 5
LCA Information 7
EPD Product Description and Use 11
Environmental Performance 14
Other life cycle stages not included in this EPD 19
References 20
Holcim - Ready-Mix Concrete - EPD 3
Revision Number Revision Date Description of Changes
1 15/4/2026

-- 3 of 21 --

INTRODUCTION
Currently, the building environment account for 39% of
global CO2 emissions, with construction materials
comprising 11% of global CO2 emissions (World Green
Building Council). By 2030, the embodied carbon of all
construction materials needs to be at least 40% lower.
By 2050, all new construction materials need to be net
zero (World Green Building Council).
Environmental Product Declarations (EPDs) play a
crucial role in promoting transparency and sustainability
in the construction industry. By providing comprehensive
and standardised information about the environmental
performance of products, EPDs enable informed
decision-making among stakeholders, including
architects, engineers, builders, and consumers.
EPDs include data on a product's life cycle impacts,
such as its carbon footprint, energy consumption, and
resource use. This transparency empowers
stakeholders to make informed selections of products.
EPDs also serve as valuable tools for benchmarking
environmental performance and driving the
decarbonation of construction materials. Demand for
low carbon products backed by an EPD drives and
rewards the decarbonisation of the entire supply chain.
As a result, EPDs will play a key role in our mission to
decarbonise construction materials and the built
environment.
ABOUT HOLCIM
Holcim Australia is a leading supplier of construction
materials in Australia, dating back to 1901. Today
Holcim continues to supply essential construction
materials including aggregates, sand, ready-mix
concrete, engineered precast concrete and prestressed
concrete solutions to a range of customers and projects
throughout Australia.
Holcim operates right across the Australian continent
supplying concrete from a network of concrete plants,
quarries, precast and concrete pipe places, and mobile
and on-site project facilities.
Sustainability is at the core of our strategy, with our
industry’s first 2050 net-zero targets, endorsed by the
Science Based Targets initiative (SBTi).
Globally, Holcim is 63,000 people around the world who
are passionate about building progress for people and
the planet through four business segments: Cement,
Ready-Mix Concrete, Aggregates and Solutions &
Products.
A FIRST FOR READY-MIX CONCRETE
IN AUSTRALIA
In 2019, Holcim published the first EPD for ready-mix
concrete. This was an Australian first for ready-mix
concrete and covered Holcim’s Normal-class concrete
range across Australia. The EPD had 147 datasets for
normal-class concrete that representative of over 4,000
mix designs. The EPD also provided Special-class
concrete data for a major Infrastructure Sustainability and
Green Star building project. This EPD heralded the
introduction of rigorously verified life cycle impact data,
setting a new benchmark in transparency and
accountability within the Australian construction sector.
Fast forward to 2021, Holcim achieved Process EPD
Certification, a first not just within the concrete industry but
across all sectors in Australia. This certification empowers
Holcim to develop and register EPDs on demand for
ready-mix concrete.
To achieve EPD Process Certification, Holcim integrated
Life Cycle Assessment (LCA) processes and procedures
into its Management Systems. We then undergo ongoing
rigorous third-party verification in accordance with
internationally recognized ISO standards and guidelines.
This EPD has been developed using our EPD Process
Certification with production occurring at the following
sites.
Holcim - Ready-Mix Concrete - EPD 4

-- 4 of 21 --

READY-MIX CONCRETE
Summary of properties and classes
Concrete is prepared by mixing cement, coarse and fine
aggregates, and water, with or without the addition of
auxiliary agents and additives. The fresh concrete is
placed on the building site or prefabricated in factory
moulds, compacted and hardened in the desired shape
by the hydration of cement to form concrete.
General Australian Standard AS 1379 sets out ways of
specifying and ordering concrete to promote uniformity,
efficiency and economy in production and delivery. It
refers to two classes of concrete: normal-class and
special-class.
 Normal-class – designed for everyday applications
such as residential and commercial foundations,
driveways and footpaths.
 Special-class – typically supplied to major
construction projects from high rise buildings, dams
and spillways, roads, bridges to public works
infrastructure etc.
Special-class concrete is typically specified in
accordance with the technical parameters and
performance requirements, which can include high-
strength/high-performances concrete, high durability,
or marine application, post-tensioned, high-
pumpability, super workable, piling concrete,
architectural off-form finishes and other decorative
applications.
Holcim - Ready-Mix Concrete - EPD 5

-- 5 of 21 --

LCA INFORMATION
Declared Unit
1 m3 of ready-mix concrete.
Scope
The scope of this EPD is cradle to gate (modules A1-A3)
with options, modules A4-A5, modules C1-C4 and
module D.
Technical Lifetime
The reference service life is not specified as the scope
of Holcim’s operational control is from cradle to delivery.
Instead, AS 3600, the Australian Standard for concrete
structures, typically specifies a design life of 50 years.
For structures with a 100-year design life, like bridges,
AS 5100 is the relevant standard.
Time Representativeness
The plant data for the LCA is based on 2022 calendar
year production data. The mix data for the LCA is based
on 2026 calendar year production data.
LCA Methodology
This EPD has been produced in conformance with the
requirements of:
 c-PCR-003 Concrete and concrete element
 Product Category Rules (PCR) 2019:14 v2.0.1.
 EN 15804+A2
 General Program Instructions (GPI) v5.0.1
 Instructions of EPD Australasia v4.2
 EN 14040 and EN 14044
Databases and LCA Software Used
SimaPro® LCA software (v10.2) was used for the LCA
modelling which developed the LCA Calculator, used as
per the certified EPD Process. It uses background data
with the following preferences:
1. Product specific EPDs for cements, admixtures,
pigments and fibres
2. The Australian National Life Cycle Inventory
Database (AusLCI v2.45) (2025)
3. Ecoinvent 3.11 and EN15804+A2 package (2024).
The environmental impacts modelled from the existing
EPDs do not include impacts for EN15804+A1, and the
additional Green Star (v1.3) impact categories included
in the environmental impact tables. These indicators are
modelled separately based on generic processes. The
following impact categories were calculated manually for
the foreground data:
 Use of renewable primary energy resources used as
raw materials
 Use of non-renewable primary energy excluding
non-renewable primary energy resources used as
raw materials
 Use of secondary material
 Use of renewable secondary fuels
 Use of non-renewable secondary fuels
Allocation
Allocation was necessary to proportion inputs and
outputs to intermediate flows at the quarry and
processes at the batching plant level.
As much as possible, intermediate flows were allocated
physically based on weight (quarries) or based on m3 of
concrete (at the batching plant).
The impacts of fly ash, granulated blast furnace slag,
and silica fume are allocated based on the economic
values. Please refer to the “Recycled Material” section
for further detail.
Cut-Off Criteria
In accordance with the PCR 2019:14 v2.0.1, the
following system boundaries are applied to
manufacturing equipment and employees:
 The infrastructure associated with electricity and
heating supply in Module A3, and infrastructure in
the manufacturing site operated by Holcim, where
impacts such as those from the construction of
power plants and manufacturing plants, are
included.
 Environmental impact from other infrastructure,
construction, production equipment, and tools that
are not directly consumed in the production process
are not accounted for in the LCI. Capital equipment
and buildings typically account for less than a few
percent of nearly all LCIs and this is usually smaller
than the error in the inventory data itself. For this
project, it is assumed that capital equipment makes
a negligible contribution to the impacts as per
Frischknecht et al. (2007) with no further
investigation.
 Personnel-related impacts, such as transportation to
and from work, are also not accounted for in the
LCI. The impacts of employees are also excluded
from inventory impacts on the basis that if they were
not employed for this production or service function,
they would be employed for another. It is very hard
to decide what proportion of the impacts from their
whole lives should count towards their employment.
For this project, the impacts of employees are
excluded.
Based on this guidance, no energy or mass flows,
except packaging of materials were excluded. All
materials required for manufacturing are delivered via
trucks and ships without packaging.
Address and Contact Information
Holcim (Australia) Pty Ltd
Level 40, Northpoint Tower, 100 Miller St,
North Sydney, NSW 2060, Australia
Web: www.holcim.com.au
Phone: +61 2 9412 6600
Holcim - Ready-Mix Concrete - EPD 6

-- 6 of 21 --

Data Quality
Data quality was assessed in terms of geographic, technical and temporal representativeness. All data sources were
scored good or very good.
Background data sources were also assessed with respect to their timeliness, with all data sources being updated
within the 3 years required under PCR 2019:14.
Modul
e
Input/
outputs Sub-processes Data source & LCA Factor Temporal
scope
Technical
scope
Geographic
scope
A1
Cementitiou
s materials
Cement Supplier data and EPD factors Very good Very good Very good
Supplementary
cementitious
materials
Supplier data and database factors Very good Good Good
Coarse
aggregate
Manufacture
d sand
Fine
aggregate
Electricity Invoices and database factors Very good Very good Very good
Diesel Invoices and database factors Very good Good Good
LPG Invoices and database factors Very good Good Good
Pollutants National Pollution Inventory (NPI)
data and database factors Very good Very good Very good
Mains water Invoices and database factors Very good Very good Very good
Water – other
sources Metered and database factors Very good Very good Very good
Water
discharge from
site
Metered and database factors Very good Very good Very good
Explosives Supplier data and database factors Very good Good Good
Gravel Production data Very good Very good Very good
Other
aggregates
Recycled
aggregates Database factors Very good Good Good
Admixture Admixtures Supplier data and database factors Very good Good Good
Oxide Oxides Invoices and database / EPD
factors Very good Good Good
Fibre Plastic and
steel fibres
Invoices and database / EPD
factors Very good Good Good
A2
Raw
material
transport
Background
data used to
model
Holcim and supplier actual
transport distances and loads per
trip and database factors
Very good Good Good
A3
Concrete
batching
plant
Electricity Invoices and database factors Very good Very good Very good
Diesel Invoices and database factors Very good Good Good
Mains water Water meters, with utility invoices
as a back-up and database factors Very good Very good Very good
Water – other
sources
Estimate based on water balance
and database factors Very good Very good Very good
Water
discharge from
site
Estimate based on Holcim site
performance metrics and database
factors
Very good Very good Very good
Lubricating oil Invoices and database factors Very good Good Good
Conveyor belt
Concrete
mix designs
Background
data used to
model
Holcim internal technical database
containing mix designs Very good Good Good
A4 Distribution
Background
data used to
model
Actual transport data and database
factors Very good Good Good
A5 Installation
Electricity Typical scenario & database
factors Very good Good Good	Diesel
Water
C1 Deconstructio
n Excavation Typical scenario & database
factors Very good Good Good
C2 Transport
Background
data used to
model
Typical scenario & database
factors Very good Good Good
C3 Waste
processing
Concrete
recycling
Typical scenario & database
factors Very good Good Good
C4 Final disposal Inert waste
landfilling
Typical scenario & database
factors Very good Good Good
D Benefits and
loads beyond Crushed gravel Typical scenario & database
factors Very good Good Good
Holcim - Ready-Mix Concrete - EPD 7

-- 7 of 21 --

System Diagram
The processes included in the LCA are presented in a process diagram in the figure below.
Holcim - Ready-Mix Concrete - EPD 8

-- 8 of 21 --

Description of System Boundaries and Excluded Lifecycle Stages
The scope of the LCA and EPD is from cradle to gate (A1-A3) with options, modules A4-A5, modules C1-C4 and
module D. The following life cycle stages have not been declared (marked as ND), as they are deemed not applicable
for Holcim’s ready-mix concrete ranges: Material emissions from usage (B1); Maintenance (B2); Repair (B3);
Replacement (B4); Refurbishment (B5); Operational energy use (B6), and Operational water use (B7).
Product Stage Constructi
on Stage Usage Stage End of Life Stage
Benefits &
loads for
the next
product
system
Raw Material Supply
Transport
Manufacturing
Transport
Construction/installation
process
Use
Maintenance incl.
transport
Repair incl. transport
Replacement incl.
transport
Refurbishment incl.
transport
Operational Energy Use	
Operational Water Use
De-construction &
demolition	
Transport
Re-use recycling
Final Disposal
Reuse, Recovery	
Recycling potential
Module A1 A2 A3 A4 A5 B1 B2 B3 B4 B5 B6 B7 C1 C2 C3 C4 D
Modules declared X X X X X ND ND ND ND ND ND ND X X X X X
Geography GL
O AU AU AU AU - - - - - - - AU AU AU AU AU
Share of specific
data* 17.3 % - - - - - - - - - - - - - -
Variation –
products 0% - - - - - - - - - - - - - -
Variation – sites <10% - - - - - - - - - - - - - -
* The share of primary data is calculated based on GWP-GHG results. It is a simplified indicator for data quality that supports the use of more
primary data, to increase the representativeness of and comparability between EPDs. Note that the indicator does not capture all relevant aspects
of data quality and is not comparable across product categories.
* The reported share of primary data is associated with uncertainty, as several EPDs used as data source lack information on the share of primary
data.
Upstream processes
The upstream processes include those involved in Module A1 – Raw material supply. This module includes:
 Extraction, transport, and manufacturing of raw materials.
 Generation of electricity from primary and secondary energy resources, also including their extraction, refining
and transport for Modules A1.
Core Processes
The core processes include those involved in Module A2 and Module A3, including:
 External transportation of materials to the core processes and internal transport.
 Manufacturing of concrete (excluding mixing, which occurs in the mixing truck and is considered part of the A4
module).
 Treatment of waste and wastewater generated from the manufacturing processes.
Downstream Processes
The downstream processes include those involved in Module A4 to D, including:
 Distribution of concrete mixes.
 Installation of the ready-mix concrete on the site.
 Wastage of construction products (This is accounted for in module A5. This includes waste concrete on site).
 Transport of equipment and use of materials for deconstruction at the end of life.
 Transport of waste generated at the end of life.
 Treatment of waste generated at the end of life.
Other Environmental Information
Other environmental information includes process involved in Module D. This module indicates the environmental
benefits from reuse, recovery, and recycling of wastes.
Holcim - Ready-Mix Concrete - EPD 9

-- 9 of 21 --

EPD PRODUCT DESCRIPTION AND USE
QLD - Brisbane - ECOPact - QE252M100 - S25/20/100 Ecopact Concrete - General use
UN CPC code: 375 (articles of concrete, cement and plaster). ANZSIC Classification: 2033 Ready Mix Concrete
Manufacturing.
Product lifespan: The product lifespan is not declared because the lifespan of the product can vary significantly
depending on its application, usage and maintenance. Additionally, according to Section 4.2.2 of the PCR for
Construction Products version 2.0.1, the product lifespan is not relevant since the use stage modules are not
declared.
Product description: A generic description of ready-mix concrete has been provided on page 5. A detailed
breakdown of the functional properties of the ready-mix concrete, including the mix design covered in this EPD, is
provided below.
Product environmental information should only be compared when the products are functionally equivalent and used
in the same context.
Strength
(MPa) Mix Code Weight (kg/m3) Mix Description Applications / intended use
25 QE252M100 2319 S25/20/100 Ecopact
Concrete General use
Production Sites
Brisbane City, Acacia Ridge, Beaudesert, Beenleigh, Boonah, Darra, Cleveland, Geebung, Narangba, Wacol, Murarrie,
Caboolture, Brendale, Raceview.
Content Declaration
The gross weight of this declared material is 2319 kg per cubic meter makes up a minimum of 99% of the products
covered by this EPD. The following table provides a summary of the materials included in Holcim ready-mix concrete
and their relative composition by weight.
Material % by weight
Post-consumer
recycled material,
weight % of product
Biogenic material, weight-%
of product Biogenic material, kg C/m3
General purpose
cement 5 - 21 0 0 0
Aggregate 67 - 84 0 0 0
Supplementary
cementitious
materials
0 - 11 0 0 0
Water 11.6 - 12 0 0 0
Admixtures 0 0 0 0
Holcim Ready-mix concrete is classified as Non-Dangerous Goods according to the Australian Code for the Transport
of Dangerous Goods by Road and Rail. The safety data sheet for pre-mixed concrete lists all associated hazard
phrases. None of the products contain one or more substances that are listed in the “Candidate List of Substances of
Very High Concern for authorisation”. According to the PCR 2019:14, if one or more substances of the “Candidate List
of Substances of Very High Concern (SVHC) for authorisation” are present in a product and their total content
exceeds 0.1% of the weight of the product, they need to be reported.
Holcim - Ready-Mix Concrete - EPD 10

-- 10 of 21 --

Packaging
Holcim ready-mix concrete is delivered in bulk with no packaging.
Recycled Material
BS EN 16757:2017 specifically lists the following materials relevant to the study as co-products:
 Fly ash,
 Ground granulated blast furnace slag; and
 Silica fume.
As such, the above materials are considered as co-products of their production process and the impacts for their
production process are allocated according to PCR 2019:14 Construction Products and Construction Services (co-
produced goods, multi-output allocation).
According to PCR 2019:14, economic allocation shall be used for processes producing co-products for use in cement
and concrete. It should be based on market prices, preferably in long-term averages (≥3 years). While assessing the
environmental burden of the high value co-products (e.g., steel, electricity, silicon), the environmental burden allocated
to the low value co-products used in cement and concrete can be omitted as a conservative estimate. Therefore, the
economic allocation method is applied to the below materials:
 Fly ash: It is sourced directly from coal fired electricity generation. The environmental impact of fly ash is derived
from coal-fired electricity, converted from the heating value of coal on a per-kWh basis.
 Ground granulated blast furnace slag: The environmental impact is allocated to blast furnace slag at the point of
generation during pig iron production, based on both production volumes and market prices. However, the specific
energy and processing impacts associated with grinding the slag into ground granulated blast furnace slag are
included in stage A1.
 Silica fume: It is sourced as a co-product of ferrosilicon production. The raw material impact of silica fume is
allocated directly from ferrosilicon, considering the relative production volumes and market prices.
Since SCM market price fluctuate and full datasets are often confidential and not disclosed by upstream suppliers,
economic allocation has been based on the mix of primary and secondary data, from Holcim internal records, the
AusLCI database and values reported in a peer-reviewed Australian LCA study (Mohammadi & South, 2017). The
AusLCI dataset conforms to EN 15804+A2 when applying allocation to its various processes and sub-processes.
Cradle to Gate (Modules A1 – A3)
Raw materials for producing Holcim’s ready-mix concrete include cementitious materials, aggregates, admixtures,
oxides, fibres, water, and ice. These raw materials are generally transported from various locations around Australia,
China, Indonesia, and Europe. The raw materials are stored in silos, hoppers, ground bins or tanks. The materials are
feed to batching plant hopper with calibrated scale. Then all the raw materials are discharged via a chute into the
ready-mix concrete truck. Water is then weighed, or volume metered and discharged into the mixer truck through the
same charging tank.
Holcim’s ready-mix concrete is manufactured across ACT, NSW, QLD, SA, VIC, and WA, Australia. State-specific
residual electricity mix available in the AusLCI database is used to model electricity in the foreground processes. The
AusLCI dataset was last updated in 2025 to reflect the latest residual electricity mix source from the FY2023.
State Energy source in residual electricity mix
GWP-GHG
(kg CO2
eq./kWh)
NSW&ACT 69% black coal, 12% solar, 6% wind, 5% hydro, and 8% others 8.6E-01
QLD 71% black coal, 13% solar, 10% natural gas, and 6% others 9.3E-01
SA 34% wind, 31% natural gas, 24% solar, 9% brown coal, and 2% others 1.6E-01
VIC 64% brown coal, 15% wind, 8% solar, 7% hydro, and 6% others 1.0E+00
WA 44% natural gas, 30% black coal, 13% solar, 13% wind, and <1% others 7.2E-01
Holcim - Ready-Mix Concrete - EPD 11

-- 11 of 21 --

Gate to Site (Module A4)
Distribution is dependent on the market requirements of ready-mix concrete products. All Holcim ready-mix concrete
products transported in Australia is by EURO5 28t – 32t trucks. The transport distances from manufacturing gate to
the site is 11.89 km. The product weight for 1m3 ready-mix concrete is the sum of weights from all raw material inputs.
Vehicle Fuel use
(L/tkm)
Fuel
type
Carrying
capacity
Density of
products
Average load
factor
Volume capacity utilization
factor
EURO 5
Truck 2.3E-02 Diesel 28 t – 32 t 2319 kg/m3 50% <1
Installation (Module A5)
As Holcim does not have operational control over the installation of ready-mix concrete at the construction site,
assumptions for construction inputs and installation waste are made based on industrial expertise and experience,
and the GCCA tool. The inputs account for the pouring of concrete from a ready-mix truck and pump, excluding any
pre-installation activities such as site work and forms. The concrete slabs are then manually finished, and no
additional inputs are required to be modelled.
Construction inputs and waste Value Unit
Concrete losses that go to landfill 3.0E+00 %
Water use 6.7E+02 L
Electricity use 2.8E+00 kWh
Diesel, in building machine 1.7E+00 L
Wastewater 6.7E-01 L
Deconstruction and End of Life (Modules C1 – C4)
EN 15804 (chapter 7.2.3.3) and applicable PCRs discourage the use of the results of modules A1-A3 & (A1-A5 for
services) without considering the results of module C.
Following the supply of ready-mix concrete products, Holcim has no control over the end-of-life fate for their products.
The recommended cradle to gate environmental profile will be based on the most common scenario as the majority of
construction products are generally deconstructed and transported for recycling. The following assumptions have
been used in this study to model deconstruction and end of life scenarios of Holcim’s ready-mix concrete:
 Deconstruction is modelled as the physical process of drilling and removing the concrete. Hydraulic excavator is
assumed as the operating tool for deconstruction. This process is based on ecoinvent v3.11 (2024) database and
the diesel used is extracted from the process.
 100% of the products ( 2319 kg) are assumed to be separately collected during deconstruction.
 25 km delivery distance to landfilling as well as reprocessing facility is assumed for waste collection process since
there was no primary data available.
 This EPD assumes 100% of the product is reprocessed/recycled as Module C3. The National Waste Report
(DCCEEW, 2023) notes that the current recycling and recovery rate of waste aggregate and concrete is 80%.
However, as PCR 2.0.1 requires that if any declared scenario is a mix of end-of-life alternatives (reuse, recycling,
incineration with energy recovery, landfill, etc.), a 100% scenario must be declared (e.g., 100% reuse, 100%
recycling, 100% incineration with energy recovery, or 100% landfill), a 100% recycling scenario has been used for
Module D of this EPD.
 The remaining waste concrete undergoes inert waste landfill as Module C4.
Vehicle Fuel use
(L/tkm)
Fuel
type
Carrying
capacity
Average load
factor
Volume capacity
utilization factor
EURO 5
Truck 2.2E-02 Diesel 40 t 50% <1
Holcim - Ready-Mix Concrete - EPD 12

-- 12 of 21 --

Module Parameter Value Unit
C1 – Deconstruction Diesel 1.3E-01 L
C2 – Transportation Distance to processing 2.5E+01 km
C3 – Waste processing Concrete recycling 1.9E+03 kg
C4 – Final disposal Inert waste landfill 4.8E+02 kg
Benefits and loads beyond the system boundary (Module D)
The end-of-life recyclers process the waste concrete into a recycled aggregate, which can be replaced with virgin
coarse aggregate for a range of applications depending on the product's performance requirements. This EPD
assumes 100% of the product is reprocessed/recycled as Module C3. The National Waste Report (DCCEEW, 2023)
notes that the current recycling and recovery rate of waste aggregate and concrete is 80%. However, as PCR 2.0.1
requires that if any declared scenario is a mix of end-of-life alternatives (reuse, recycling, incineration with energy
recovery, landfill, etc.), a 100% scenario must be declared (e.g., 100% reuse, 100% recycling, 100% incineration with
energy recovery, or 100% landfill), a 100% recycling scenario has been used for Module D of this EPD.
For Holcim’s internal aggregate production, waste concrete coarse and fine aggregates are able to be recycled and
repurposed as recycled coarse aggregate and sand. The environmental benefits from avoiding the use of virgin
materials are fully accounted for.
In the consideration of Module C, the end-of-life recyclers process the waste concrete into a recycled aggregate,
which can be replaced with virgin coarse aggregate for a range of applications depending on the products
performance requirements.
Holcim - Ready-Mix Concrete - EPD 13

-- 13 of 21 --

ENVIRONMENTAL PERFORMANCE
The environmental impacts considered in this EPD are listed in the table below. EN 15804+A2 reference package
based on EF 3.1 (Environmental Footprint) or a later version has been used. All further tables from this point will
contain abbreviation only.
Impact Category Abbreviation Measurement Unit
Potential Environmental Impact indicators
Total global warming potential GWP – T kg CO2 equivalents (GWP100)
Global warming potential (fossil) GWP – F kg CO2 equivalents (GWP100)
Global warming potential (biogenic) GWP – B kg CO2 equivalents (GWP100)
Global warming potential (land use/ land transformation) GWP – Luluc kg CO2 equivalents (GWP100)
Ozone depletion potential ODP kg CFC 11 equivalents
Acidification potential AP mol H+ eq.
Eutrophication – aquatic freshwater EP – freshwater kg P equivalent
Eutrophication – aquatic marine EP - marine kg N equivalent
Eutrophication – terrestrial EP – terrestrial mol N equivalent
Photochemical ozone creation potential POCP kg NMVOC equivalents
Abiotic depletion potential (elements)* ADPE kg Sb equivalents
Abiotic depletion potential (fossil fuels)* ADPF MJ net calorific value
Water Depletion Potential* WDP m3 equivalent deprived
Resource use indicators
Use of renewable primary energy excluding renewable primary
energy resources used as raw materials PERE MJ, net calorific value
Use of renewable primary energy resources used as raw materials PERM MJ, net calorific value
Total use of renewable primary energy resources (primary energy
and primary energy resources used as raw materials) PERT MJ, net calorific value
Use of non-renewable primary energy excluding non-renewable
primary energy resources used as raw materials PENRE MJ, net calorific value
Use of non-renewable primary energy resources used as raw
materials PENRM MJ, net calorific value
Total use of non-renewable primary energy resources (primary
energy and primary energy resources used as raw materials) PENRT MJ, net calorific value
Use of secondary material SM kg
Use of renewable secondary fuels RSF MJ, net calorific value
Use of non-renewable secondary fuels NRSF MJ, net calorific value
Use of net fresh water FW m3
Holcim - Ready-Mix Concrete - EPD 14

-- 14 of 21 --

Holcim - Ready-Mix Concrete - EPD 15
Impact Category Abbreviation Measurement Unit
Waste categories and Output flows indicators
Hazardous waste disposed HWD kg
Non-hazardous waste disposed NHWD kg
Radioactive waste disposed/stored RWD kg
Components for reuse CFR kg
Materials for recycling MFR kg
Materials for energy recovery MFEE kg
Exported energy EE - e MJ per energy carrier
Exported energy, thermal EE - t MJ per energy carrier
Additional environmental impact indicators
Global warming potential, excluding biogenic uptake, emissions and
storage GWP-GHG kg CO2 equivalents (GWP100)
Global warming potential, aligned with the IPCC 2013 Fifth Assessment
Report *
GWP-GHG
(AR5) kg CO2 equivalents (GWP100)
Particulate matter PM disease incidence
Ionising radiation – human health IRP kBq U-235 eq
Eco-toxicity (freshwater)* ETP-fw CTUe
Human toxicity potential – cancer effects* HTP-c CTUh
Human toxicity potential – non cancer effects* HTP-nc CTUh
Soil quality* SQP dimensionless
Potential environmental Impact Indicators (EN15804+A1)
Global warming (GWP100a) – A1 GWP (A1) kg CO2 equivalents
Ozone layer depletion (ODP) – A1 ODP (A1) kg CFC-11 equivalents
Acidification – A1 AP (A1) kg SO2 equivalents
Eutrophication – A1 EP (A1) kg PO43- equivalents
Photochemical oxidation – A1 POCP (A1) kg C2H4 equivalents
Abiotic depletion – A1 ADPE (A1) kg Sb equivalents
Abiotic depletion (fossil fuels) – A1 ADPF (A1) MJ, net calorific value
Global warming (GWP100a) – A1 GWP (A1) kg CO2 equivalents
Additional Greenstar v1.3 Indicators
Human Toxicity cancer Green Star HTc (GS) CTUh
Human Toxicity non-cancer Green Star HTnc (GS) CTUh
Land use Green Star LU (GS) kg C deficit equivalents
Ionising radiation Green Star IR (GS) kBq U-235 equivalents
Particulate Matter Green Star PM (GS) kg PM2.5 equivalents
WSI Green Star WSI (GS) m3 equivalents
*Disclaimer – The results of these environmental impact indicators shall be used with care as the uncertainties on these results are high or as
there is limited experience with the indicator.
**Disclaimer – This impact category deals mainly with the eventual impact of low dose ionizing radiation on human health of the nuclear fuel
cycle. It does not consider effects due to possible nuclear accidents, occupational exposure nor due to radioactive waste disposal in
underground facilities. Potential ionizing radiation from the soil, from radon and from some construction materials is also not measured by this
indicator.
*** - GWP-GHG (IPCC AR5) is an additional GWP100 indicator that is aligned with the Intergovernmental Panel on Climate Change (IPCC)
2013 Fifth Assessment Report (AR5) (IPCC 2013), national greenhouse gas reporting frameworks in Australia and New Zealand and previous
versions of the Construction Products PCR (PCR2019:14). It excludes biogenic carbon and indirect radiative forcing.

-- 15 of 21 --

QLD - Brisbane - ECOPact - QE252M100 - S25/20/100 Ecopact Concrete - General use
The use of results of modules A1-A3 or A1-A5, without considering the results of module C may mislead the communication and decision-making. The estimated impact
results are only relative statements, which do not indicate the endpoints of the impact categories, exceeding threshold values, safety margins and/or risks.
PRIMARY ENVIRONMENTAL INDICATORS (in accordance with EN 15804:2012+A2:2019) – 1m3 of ready-mix concrete
Abbreviation Unit A1-A3 A4 A5 C1 C2 C3 C4 D
GWP-Total kg CO2 eq. 146 2.58 12.9 0.522 4.31 10.4 0 -18.5
GWP-Fossil kg CO2 eq. 145 2.58 12.8 0.522 4.31 10.3 0 -18.5
GWP-Biogenic kg CO2 eq. 0.822 0.0000896 0.0299 0.0000223 0.000150 0.00865 0 -0.0150
GWP-Luluc kg CO2 eq. 0.0489 0.0000661 0.0104 0.0000184 0.000110 0.00810 0 -0.0168
ODP kg CFC 11 eq. 1.33E-6 3.40E-8 1.40E-7 7.80E-9 5.68E-8 1.32E-7 0 -9.01E-9
AP mol H+ eq. 0.829 0.0134 0.0992 0.00491 0.0224 0.0915 0 -0.105
EP-F kg P eq. 0.0173 1.91E-6 0.000527 4.73E-7 3.19E-6 0.0000222 0 -0.000715
EP-M kg N eq. 0.112 0.00351 0.0332 0.00231 0.00587 0.0386 0 -0.0266
EP-T mol N eq. 1.91 0.0392 0.384 0.0253 0.0655 0.422 0 -0.292
POCP kg NMVOC eq. 0.523 0.0148 0.112 0.00748 0.0247 0.125 0 -0.0931
ADPE kg Sb eq. 0.0147 8.67E-8 0.000440 2.15E-8 1.45E-7 1.69E-6 0 -2.29E-6
ADPF MJ 1029 33.5 125 6.89 56.0 121 0 -243
WDP m3 equivalent
deprived
26.3 0.0122 43.7 0.00925 0.0204 2.41 0 -32.6
RESOURCE USE PARAMETERS (in accordance with EN 15804:2012+A2:2019) – 1m3 of ready-mix concrete
Abbreviation Unit A1-A3 A4 A5 C1 C2 C3 C4 D
PERE MJ 43.6 0.0561 6.43 0.0129 0.0937 4.42 0 -23.4
PERM MJ 0 0 0 0 0 0 0 0
PERT MJ 43.6 0.0561 6.43 0.0129 0.0937 4.42 0 -23.4
PENRE MJ 1038 33.5 125 6.89 56.0 121 0 -243
PENRM MJ 0 0 0 0 0 0 0 0
PENRT MJ 1038 33.5 125 6.89 56.0 121 0 -243
SM kg 167 0 5.00 0 0 0 0 0
RSF MJ 1.58 0 0.0475 0 0 0 0 0
NRSF MJ 34.6 0 1.04 0 0 0 0 0
FW m3 0.483 0.000426 0.668 0.000222 0.000712 0.0417 0 -0.784
Holcim - Ready-Mix Concrete - EPD 16

-- 16 of 21 --

WASTE CATEGORIES AND OUTPUT FLOWS (in accordance with EN 15804:2012+A2:2019) – 1m3 of ready-mix concrete
Abbreviation Unit A1-A3 A4 A5 C1 C2 C3 C4 D
HWD kg 0.946 0.000230 0.0289 0.0000113 0.000383 0.000770 0 -0.000841
NHWD kg 49.6 0.000861 71.1 2.19E-6 0.00144 0.115 0 -0.235
RWD kg 0.0000348 1.27E-6 5.44E-6 0 2.12E-6 7.44E-6 0 -0.000518
CRU kg 0 0 0 0 0 0 0 0
MFR kg 0.156 0 0.00467 0 0 2319 0 0
MFRE kg 0 0 0 0 0 0 0 0
EE - e MJ 0 0 0 0 0 0 0 0
EE - t MJ 0 0 0 0 0 0 0 0
ADDITIONAL ENVIRONMENTAL IMPACT INDICATORS (in accordance with EN 15804:2012+A2:2019) – 1m3 of ready-mix concrete
Abbreviation Unit A1-A3 A4 A5 C1 C2 C3 C4 D
GWP-GHG kg CO2 eq. 146 2.58 12.9 0.522 4.31 10.4 0 -18.5
GWP-GHG (AR5) kg CO2 eq. 148 2.59 12.9 0.523 4.32 10.4 0 -18.5
PM disease incidence 0.0000167 2.34E-7 2.32E-6 1.41E-7 3.90E-7 2.36E-6 0 -1.66E-6
IRP kBq U-235 eq 370 0.00245 11.1 0.000526 0.00408 0.0126 0 -0.800
ETP-fw CTUe 352 1.25 13.8 0.250 2.09 5.18 0 -33.5
HTP-c CTUh 1.92E-7 1.03E-10 6.20E-9 2.81E-11 1.73E-10 8.63E-10 0 -2.08E-9
HTP-nc CTUh 5.36E-6 5.22E-9 1.74E-7 5.14E-10 8.72E-9 1.81E-8 0 -7.91E-8
SQP dimensionless 315 0.0499 19.1 0.0133 0.0833 31.8 0 -156
Holcim - Ready-Mix Concrete - EPD 17

-- 17 of 21 --

ADDITIONAL ENVIRONMENTAL IMPACT INDICATORS (in accordance with EN 15804:2012+A1:2013) – 1m3 of ready-mix concrete
Abbreviation Unit A1-A3 A4 A5 C1 C2 C3 C4 D
GWP (A1) kg CO2 eq. 147 2.58 12.9 0.522 4.31 10.3 0 -18.5
ODP (A1) kg CFC 11 eq. 1.33E-6 3.40E-8 1.40E-7 7.80E-9 5.68E-8 1.32E-7 0 -9.01E-9
AP (A1) kg SO2 eq. 0.829 0.0134 0.0992 0.00491 0.0224 0.0915 0 -0.105
EP (A1) kg PO43- eq. 0.0853 0.00122 0.0127 0.000779 0.00204 0.0131 0 -0.0113
POCP (A1) kg C2H4 eq. 0.523 0.0148 0.112 0.00748 0.0247 0.125 0 -0.0931
ADPE (A1) kg SO2 eq. 0.0147 8.67E-8 0.000440 2.15E-8 1.45E-7 1.69E-6 0 -2.29E-6
ADPF (A1) MJ 1029 33.5 125 6.89 56.0 121 0 -243
ADDITIONAL GREEN STAR (V1.3) IMPACT INDICATORS – 1m3 of ready-mix concrete
Abbreviation Unit A1-A3 A4 A5 C1 C2 C3 C4 D
HTc (GS) CTUh 6.05E-9 2.41E-11 2.58E-10 3.60E-12 4.03E-11 1.04E-10 0 -4.73E-10
HTnc (GS) CTUh 2.11E-10 2.65E-12 9.11E-12 2.08E-13 4.42E-12 4.74E-12 0 -2.19E-11
LU (GS) kg C deficit eq. 57.8 0.0275 2.06 0.00637 0.0459 2.97 0 -494
IR (GS) kBq U235 eq. 0.141 0.00246 0.0121 0.000526 0.00410 0.0127 0 -0.805
PM (GS) kg PM2.5 eq. 0.0000167 2.34E-7 2.32E-6 1.41E-7 3.90E-7 2.36E-6 0 -1.66E-6
WSI (GS) m3 1.36 0.000415 2.28 0.000309 0.000693 0.122 0 -1.04
Holcim - Ready-Mix Concrete - EPD 18

-- 18 of 21 --

OTHER LIFE CYCLE STAGES NOT INCLUDED IN
THIS EPD
While the LCA study and EPD only consider the cradle to gate (modules A1-A3) with options modules A4-A5, modules
C1-C4 and module D of the environmental impacts of Holcim’s ready-mix concrete, practitioners using the EPD for the
purpose of whole-of-life building studies or the functional comparison of different building products on a whole-of-life
basis will consider concrete’s other life cycle stages. Some of the environmental impacts of benefits associated with
other life cycle stages not included in this EPD are described in the following sections.
Lifetime absorption of CO2
Carbonation is a natural process whereby concrete absorbs carbon dioxide (CO2) from the atmosphere through a
chemical reaction between the CO2 in the ambient air and hydration products within the concrete (CaOH2). Ready-mix
concrete can be subject to carbonation from the use stage onward (i.e. after construction and curing). From a life cycle
impact accounting perspective, this process can also be referred to as ‘reabsorption’, since the CO2 emitted during the
cement manufacturing process can be partly offset by the lifetime absorption of CO2, therefore reducing the net CO2
emissions associated with concrete over its lifetime.
The carbonisation process is a commonly known process in building design and is typically taken into consideration by
engineers when specifying special-class concrete.
The total amount of CO2 absorption during the life cycle of concrete is subject to a range of factors and varies over
time. The calculation has been standardised in the British and European Standard BS EN 16757:2017 Sustainability
of construction works – Environmental Product Declarations – Product Category Rules for concrete and concrete
elements. It is recommended that practitioners make use of this standard when conducting whole-of-life building
studies and if the building materials include substantial amounts of concrete. Please note that CO2 absorption has not
been considered in this EPD and is not reflected in the EPD results tables.
Holcim - Ready-Mix Concrete - EPD 19

-- 19 of 21 --

REFERENCES
AusLCI. (2025) AusLCI Database – v2.45. Retrieved from Australian Life Cycle Inventory Database Initiative:
www.auslci.com.au/
Australasian EPD Programme. (2024). A Regional Annex to the General Programme Instructions of the International
EPD System V4.2. Published 2024-04-12.
Department of Climate Change, Energy, the Environment and Water. (2023). National Waste Report 2022. Retrieved
from https://www.dcceew.gov.au/environment/protection/waste/national-waste-reports/2022.
Ecoinvent Centre. (2024). Ecoinvent version 3.11 database. Zurich: ETH, Agroscope, EMPA, EPFL, PSI. Retrieved
from www.ecoinvent.org.
EPD International. (2025). General Programme Instructions (GPI) for the International EPD System V5.0.1. Published
2025-02-07. Retrieved from www.envirodec.com.
EPD International. (2025). Product Category Rules for Construction Products and Construction Services, PCR2019:14
v2.0.1. Published 2025-06-05. Stockholm: EPD International.
European Committee for Standardization. (2021). Sustainability of construction works. Environmental product
declarations. Core rules for the product category of construction products, EN 15804:2012+A2:2019/AC:2021.
European Committee for Standardization. (2022). European Committee for Standardization. (2022). Sustainability of
construction works - Environmental product declarations - Product Category Rules for concrete and concrete
elements, EN 16757:2022. European Committee for Standardization.
European Committee for Standardization. (2024). Sustainability of construction works - Data quality for environmental
assessment of products and construction work - Selection and use of data, EN 15941:2024. European Committee for
Standardization.
Green Building Council of Australia. (2022). An upfront conversation about upfront carbon. Retrieved from GBCA:
https://new.gbca.org.au/news/gbca-news/upfront-conversation-about-upfront-carbon/
ISO. (2020). Environmental labels and declarations – Type III environmental declarations – Principles and procedures,
ISO 14025:2006. Geneva: International Organization for Standardization.
ISO. (2020). Environmental management – Life cycle assessment – Principles and framework, ISO
14040:2006+A2:2020. Geneva: International Organization for Standardization.
ISO. (2020). Environmental management. Life cycle assessment. Requirements and guidelines, ISO
14044:2006+A2:2020. Geneva: International Organization for Standardization.
Man Yu, Thomes Wiedmann, Robert Crawford, Catriona Tait, ‘The Carbon Footprint of Australia’s Construction
Sector’, Procedia Engineering, Volume 180, 2017, Pages 211-220, ISSN 1877-7058,
(http://www.sciencedirect.com/science/article/pii/S1877705817316879)
Mohammadi, J., & South, W. (2017). Life cycle assessment (LCA) of benchmark concrete products in Australia. The
International Journal of Life Cycle Assessment, 22(10), 1588-1608.
World Green Building Council. (2019). Bringing embodied carbon upfront. Retrieved from World Green Building
Council: https://worldgbc.org/advancing-net-zero/embodied-carbon/
Holcim - Ready-Mix Concrete - EPD 20

-- 20 of 21 --

Contact your Holcim representative today for more information.
Customer Service Centre 131 188
Holcim (Australia) Pty Ltd
Level 40/100 Miller St,
North Sydney NSW 2060, Australia
Phone 02 9412 6600
ABN 87 099 732 297
www.holcim.com.au
This publication supersedes all previous literature on this subject. As the specifications and details
contained in this publication may change, please check with Holcim Customer Service for
confirmation of current issue. This publication provides general information only and is no substitute
for professional technical engineering advice. Users must make their own determination as to the
suitability of this information or any Holcim product for their specific circumstances. Holcim accepts
no liability for any loss or damage resulting from their specific circumstances. Holcim accepts no
liability for a loss or damage resulting from any reliance on the information provided in this
publication. Holcim is a registered trademark of Holcim Ltd.
© 2026 Holcim (Australia) Pty Ltd ABN 87 732 297. All rights reserved.
This guide or any part of it may not be reproduced without prior written consent of Holcim.
Holcim - Ready-Mix Concrete - EPD 21

-- 21 of 21 --

