READY-MIX CONCRETE
Environmental Product Declaration
VIC - Melbourne Metro - ECOPact- VE322EAMF
In accordance with ISO 14025 and EN15804+A2
Programme: The International EPD® System | www.environdec.com
Programme operator: EPD International AB
Regional Programme: EPD Australasia | www.epd-australasia.com
Managed by: Holcim Certified EPD Process
EPD Process Certificate Number: 04
Accreditation Body: Epsten Group, Inc.
EPD Registration No.: EPD-IES-20602:001
Valid from: 15/04/2025 | 15/04/2030
Revision Date: 15/04/2025
Revision Number: 1
EPD Process Geographical Scope: Australia

-- 1 of 20 --

Programme-related information and verification
EPD Owner
Evan Smith
Holcim (Australia) Pty Ltd
Level 40, Northpoint Tower, 100 Miller St, North
Sydney NSW 2060, Australia
Web: www.holcim.com.au
Phone: +61 2 9412 6600
Programme Operator
EPD International AB,
Box 210 60, SE-100 31
Stockholm, Sweden,
E-mail: info@environdec.com
Regional Programme Operator
EPD Australasia Limited
315a Hardy Street Nelson 7010, New Zealand
Web: www.epd-australasia.com
Email: info@epd-australasia.com
Phone: +61 2 8005 8206
EPD Produced by
Jonas Bengtsson, Sazal Kundu & Weiqi Xing
Edge Environment Pty Ltd
Level 3, Greenhouse, 180 George Street, Sydney
NSW 2000 Australia
Web: www.edgeimpact.global
Phone: +61 2 9438 0100
EPD Process Certified by
Epsten Group
Suite 2600, 101 Marietta St NW, Atlanta, Georgia
30303, USA
Web: www.epstengroup.com
EPD Registration Number EPD-IES-20602:001
Valid From 15/04/2025
Revision Number 1
Valid Until 15/04/2030
Product group classification UN CPC 375 (Articles of concrete, cement and plaster)
Geographical Scope Australia
Reference Year for Data 2022 Plant Data, 2025 Mix/Materials Data
CEN standard EN 15804:2012+A2:2019/AC:2021 served as the core Product Category Rules (PCR)
Product category rules PCR 2019:14 Construction Products, Version 1.3.4, 2024-04-30
c-PCR-003 Concrete and Concrete Elements, 2024-04-30
PCR review was conducted by
The Technical Committee of the International EPD System. See www.environdec.com
for a list of members. Review chair: Claudia A. Peña, University of Concepción, Chile.
The review panel may be contacted via the Secretariat www.environdec.com/contact
Independent third-party
verification of the declaration and
data, according to ISO
14025:2006:
☒ EPD process certification*
*For EPD Process Certification, an accredited certification body certifies and reviews the
management process and verifies EPDs published on a regular basis. For details about third-
party verification procedure of the EPDs, see the GPI.
Process certification
Epsten Group, Inc., Megan Blizzard, is an approved
certification body accountable for third-party
verification. Third-party verifier is accredited by:
A2LA, Certificate #3142.03
Programme-related information and verification:
The EPD owner has the sole ownership, liability, and responsibility for the EPD. EPDs within the same product category but registered in different
EPD programmes, or not compliant with EN 15804, may not be comparable. For two EPDs to be comparable, they must be based on the same
PCR (including the same version number) or be based on fully-aligned PCRs or versions of PCRs; cover products with identical functions, technical
performances and use (e.g. identical declared/functional units); have equivalent system boundaries and descriptions of data; apply equivalent data
quality requirements, methods of data collection, and allocation methods; apply identical cut-off rules and impact assessment methods (including
the same version of characterisation factors); have equivalent content declarations; and be valid at the time of comparison. For further information
about comparability, see EN 15804 and ISO 14025.
Holcim - Ready-Mix Concrete - EPD 2

-- 2 of 20 --

TABLE OF CONTENTS
Introduction.........................................................................................................................................5
About Holcim......................................................................................................................................5
A first for ready-mix concrete in Australia.............................................................................................5
LCA Information..................................................................................................................................7
EPD Product Description and Use...................................................................................................11
Environmental Performance.............................................................................................................14
Other life cycle stages not included in this EPD...............................................................................19
References.......................................................................................................................................20
Revision Number Revision Date Description of Changes
1 15/04/2025
Holcim - Ready-Mix Concrete - EPD 3

-- 3 of 20 --

INTRODUCTION
Currently, the building environment account for 39% of
global CO2 emissions, with construction materials
comprising 11% of global CO2 emissions (World Green
Building Council). By 2030, the embodied carbon of all
construction materials needs to be at least 40% lower.
By 2050, all new construction materials need to be net
zero (World Green Building Council).
Environmental Product Declarations (EPDs) play a
crucial role in promoting transparency and sustainability
in the construction industry. By providing comprehensive
and standardised information about the environmental
performance of products, EPDs enable informed
decision-making among stakeholders, including
architects, engineers, builders, and consumers.
EPDs include data on a product's life cycle impacts,
such as its carbon footprint, energy consumption, and
resource use. This transparency empowers
stakeholders to make informed selections of products.
EPDs also serve as valuable tools for benchmarking
environmental performance and driving the
decarbonation of construction materials. Demand for
low carbon products backed by an EPD drives and
rewards the decarbonisation of the entire supply chain.
As a result, EPDs will play a key role in our mission to
decarbonise construction materials and the built
environment.
ABOUT HOLCIM
Holcim Australia is a leading supplier of construction
materials in Australia, dating back to 1901. Today
Holcim continues to supply essential construction
materials including aggregates, sand, ready-mix
concrete, engineered precast concrete and prestressed
concrete solutions to a range of customers and projects
throughout Australia.
Holcim operates right across the Australian continent
supplying concrete from a network of concrete plants,
quarries, precast and concrete pipe places, and mobile
and on-site project facilities.
Sustainability is at the core of our strategy, with our
industry’s first 2050 net-zero targets, endorsed by the
Science Based Targets initiative (SBTi).
Globally, Holcim is 63,000 people around the world who
are passionate about building progress for people and
the planet through four business segments: Cement,
Ready-Mix Concrete, Aggregates and Solutions &
Products.
A FIRST FOR READY-MIX CONCRETE
IN AUSTRALIA
In 2019, Holcim published the first EPD for ready-mix
concrete. This was an Australian first for ready-mix
concrete and covered Holcim’s Normal-class concrete
range across Australia. The EPD had 147 datasets for
normal-class concrete that representative of over 4,000
mix designs. The EPD also provided Special-class
concrete data for a major Infrastructure Sustainability and
Green Star building project. This EPD heralded the
introduction of rigorously verified life cycle impact data,
setting a new benchmark in transparency and
accountability within the Australian construction sector.
Fast forward to 2021, Holcim achieved Process EPD
Certification, a first not just within the concrete industry but
across all sectors in Australia. This certification empowers
Holcim to develop and register EPDs on demand for
ready-mix concrete.
To achieve EPD Process Certification, Holcim integrated
Life Cycle Assessment (LCA) processes and procedures
into its Management Systems. We then undergo ongoing
rigorous third-party verification in accordance with
internationally recognized ISO standards and guidelines.
This EPD has been developed using our EPD Process
Certification with production occurring at the following
sites.
Holcim - Ready-Mix Concrete - EPD 4

-- 4 of 20 --

READY-MIX CONCRETE
Summary of properties and classes
Concrete is prepared by mixing cement, coarse and fine
aggregates, and water, with or without the addition of
auxiliary agents and additives. The fresh concrete is placed
on the building site or prefabricated in factory moulds,
compacted and hardened in the desired shape by the
hydration of cement to form concrete.
General Australian Standard AS 1379 sets out ways of
specifying and ordering concrete to promote uniformity,
efficiency and economy in production and delivery. It refers
to two classes of concrete: normal-class and special-class.
 Normal-class – designed for everyday applications
such as residential and commercial foundations,
driveways and footpaths.
 Special-class – typically supplied to major
construction projects from high rise buildings, dams
and spillways, roads, bridges to public works
infrastructure etc.
Special-class concrete is typically specified in
accordance with the technical parameters and
performance requirements, which can include high-
strength/high-performances concrete, high durability,
or marine application, post-tensioned, high-
pumpability, super workable, piling concrete,
architectural off-form finishes and other decorative
applications.
Holcim - Ready-Mix Concrete - EPD 5

-- 5 of 20 --

LCA INFORMATION
Declared Unit
1 m3 of ready-mix concrete.
Scope
The scope of this EPD is cradle to gate (modules A1-A3)
with options, modules A4-A5, modules C1-C4 and
module D.
Reference Service Life (RSL)
The RSL is not specified as the scope of Holcim’s
operational control is from cradle to delivery.
Time Representativeness
The plant data for the LCA is based on 2022 calendar
year production data. The mix data for the LCA is based
on 2025 calendar year production data.
Databases and LCA Software Used
SimaPro® LCA software (v 9.5) was used for the LCA
modelling which developed the LCA Calculator, used as
per the certified EPD Process. It uses background data
with the following preferences:
1. Product specific EPDs for cements, admixtures,
pigments and fibres
2. The Australian National Life Cycle Inventory
Database (AusLCI v1.42) (2023)
3. Ecoinvent 3.9.1 (2023).
The environmental impacts modelled from the existing
EPDs do not include impacts for EN15804+A1, and the
additional Green Star (v1.3) impact categories included
in the environmental impact tables. These indicators are
modelled separately based on generic processes. The
following impact categories were calculated manually for
the foreground data:
 Use of renewable primary energy resources
used as raw materials
 Use of non-renewable primary energy excluding
non-renewable primary energy resources used
as raw materials
 Use of secondary material
 Use of renewable secondary fuels
 Use of non-renewable secondary fuels
Allocation
Allocation was necessary to proportion inputs and
outputs to intermediate flows at the quarry and
processes at the batching plant level.
As much as possible, intermediate flows were allocated
physically based on weight (quarries) or based on m2 of
concrete (at the batching plant). At the quarry level,
whenever physical allocation was not possible,
economic allocation was carried out based on Holcim’s
internal cost system.
Regarding inputs, it was assumed that fly ash and silica
fumes are waste products and therefore burden-free.
Ground granulated blast furnace slag from steel blast
furnace production was allocated economically. Please
refer to the “Recycled Material” section for further detail.
Cut-Off Criteria
In accordance with the PCR 2019:14, the following
system boundaries are applied to manufacturing
equipment and employees:
 Environmental impact from infrastructure,
construction, production equipment, and tools
that are not directly consumed in the production
process are not accounted for in the LCI. Capital
equipment and buildings typically account for
less than a few percent of nearly all LCIs and
this is usually smaller than the error in the
inventory data itself. For this project, it is
assumed that capital equipment makes a
negligible contribution to the impacts as per
Frischknecht et al. (2007) with no further
investigation.
 Personnel-related impacts, such as
transportation to and from work, are also not
accounted for in the LCI. The impacts of
employees are also excluded from inventory
impacts on the basis that if they were not
employed for this production or service function,
they would be employed for another. It is very
hard to decide what proportion of the impacts
from their whole lives should count towards their
employment. For this project, the impacts of
employees are excluded.
Based on this guidance, no energy or mass flows,
except packaging of materials were excluded. All
materials required for manufacturing are delivered via
trucks and ships without packaging.
Address and Contact Information
Holcim (Australia) Pty Ltd
Level 40, Northpoint Tower, 100 Miller St,
North Sydney, NSW 2060, Australia
Web: www.holcim.com.au
Phone: +61 2 9412 6600
Holcim - Ready-Mix Concrete - EPD 6
Ready-mix & LCA

-- 6 of 20 --

Data Quality
Data quality was assessed in terms of geographic and temporal representativeness. All data sources were scored
good or very good.
Background data sources were also assessed with respect to their timeliness, with all data sources being updated
within the 10 years required under PCR 2019:14.
Module Input/outputs Sub-processes Data source & LCA Factor Temporal
scope
Geographic
scope Quality
A1
Cementitious
materials
Cement Supplier data and EPD factors 2022 All states Very good
Supplementary
cementitious
materials
Supplier data and Ecoinvent factors 2022 National Good
Coarse
aggregate
Manufactured
sand
Fine
aggregate
Electricity Invoices and AusLCI factors 2022 All states Very good
Diesel Invoices and Ecoinvent factors 2022 All states Very good
LPG Invoices and Ecoinvent factors 2022 All states Very good
Pollutants National Pollution Inventory (NPI)
data and Ecoinvent factors 2022 All states Very good
Mains water Invoices and Ecoinvent factors 2022 All states Very good
Water – other
sources Metered and Ecoinvent factors 2022 All states Very good
Water discharge from
site Metered and Ecoinvent factors 2022 All states Very good
Explosives Supplier data and Ecoinvent factors 2022 All states Very good
Gravel Production data 2022 All states Very good
Other
aggregates Recycled aggregates Ecoinvent database 2023 National Good
Admixture Admixtures Supplier data and Ecoinvent factors 2023 National Good
Oxide Oxides Invoices and Ecoinvent / EPD factors 2023 National Good
Fibre Plastic and steel
fibres Invoices and Ecoinvent / EPD factors 2023 National Good
A2 Raw material
transport
Background data
used to model
Holcim and supplier actual transport
distances and loads per trip and
AusLCI factors
2022 All states Very good
A3
Concrete
batching plant
Electricity Invoices and Ecoinvent factors 2022 All states Very good
Diesel Invoices and Ecoinvent factors 2022 All states Very good
Mains water Water meters, with utility invoices as
a back-up and Ecoinvent factors 2022 All states Very good
Water – other
sources
Estimate based on water balance and
Ecoinvent factors 2022 All states Very good
Water discharge from
site
Estimate based on Holcim site
performance metrics and Ecoinvent
factors
2022 All states Very good
Lubricating oil Invoices and Ecoinvent factors 2023 National Good
Conveyor belt
Concrete mix
designs
Background data
used to model
Holcim internal technical database
containing mix designs 2022 All states Very good
A4 Distribution Background data
used to model
Actual transport data and Ecoinvent
factors 2022 All states Very good
A5 Installation
Electricity
Typical scenario & Ecoinvent factors 2023 National Good	Diesel
Water
C1 Deconstruction Excavation Typical scenario & Ecoinvent factors 2023 National Good
C2 Transport Background data
used to model Typical scenario & Ecoinvent factors 2023 National Good
C3 Waste
processing Concrete recycling Typical scenario & Ecoinvent factors 2023 National Good
C4 Final disposal Inert waste landfilling Typical scenario & Ecoinvent factors 2023 National Good
D Benefits and
loads beyond Crushed gravel Typical scenario & Ecoinvent factors 2023 National Good
Holcim - Ready-Mix Concrete - EPD 7

-- 7 of 20 --

System Diagram
The processes included in the LCA are presented in a process diagram in the figure below.
Holcim - Ready-Mix Concrete - EPD 8

-- 8 of 20 --

Description of System Boundaries and Excluded Lifecycle Stages
The scope of the LCA and EPD is from cradle to gate (A1-A3) with options, modules A4-A5, modules C1-C4 and
module D. The following life cycle stages have not been declared, as they are deemed not applicable for Holcim’s
ready-mix concrete ranges: Material emissions from usage (B1); Maintenance (B2); Repair (B3); Replacement (B4);
Refurbishment (B5); Operational energy use (B6), and Operational water use (B7).
Product Stage Construction
Stage Usage Stage End of Life Stage
Benefits &
loads for the
next product
system
Raw Material Supply
Transport
Manufacturing
Transport
Construction/installation
process
Use
Maintenance incl. transport
Repair incl. transport
Replacement incl. transport	
Refurbishment incl. transport
Operational Energy Use	
Operational Water Use
De-construction & demolition
Transport
Re-use recycling
Final Disposal
Reuse, Recovery Recycling
potential
Module A1 A2 A3 A4 A5 B1 B2 B3 B4 B5 B6 B7 C1 C2 C3 C4 D
Modules declared X X X X X ND ND ND ND ND ND ND X X X X X
Geography
AU
&
GLO
AU AU AU AU - - - - - - - AU AU AU AU AU
Share of specific data 63.8 % - - - - - - - - - - - - - -
Variation – products 0% - - - - - - - - - - - - - -
Variation – sites 0% - - - - - - - - - - - - - -
Upstream processes
The upstream processes include those involved in Module A1 – Raw material supply. This module includes:
 Extraction, transport and manufacturing of raw materials.
 Generation of electricity from primary and secondary energy resources, also including their extraction, refining
and transport for Modules A1 and A3.
Core Processes
The core processes include those involved in Module A2 and Module A3, including:
 External transportation of materials to the core processes and internal transport.
 Manufacturing of concrete (excluding mixing, which occurs in the mixing truck and is considered part of the A4
module).
 Treatment of waste and wastewater generated from the manufacturing processes.
Downstream Processes
The downstream processes include those involved in Module A4 to D, including:
 Distribution of concrete mixes.
 Installation of the ready-mix concrete on the site.
 Wastage of construction products (This is accounted for in module A5. This includes waste concrete on site).
 Transport of equipment and use of materials for deconstruction at the end of life.
 Transport of waste generated at the end of life.
 Treatment of waste generated at the end of life.
Other Environmental Information
Other environmental information includes process involved in Module D. This module indicates the environmental
benefits from reuse, recovery, and recycling of deconstructed concrete.
Holcim - Ready-Mix Concrete - EPD 9

-- 9 of 20 --

EPD PRODUCT DESCRIPTION AND USE
VIC - Melbourne Metro - ECOPact- VE322EAMF
A detailed breakdown of the functional properties of the ready-mix concrete included in this EPD are provided below.
Product environmental information should only be compared with consideration of the product’s requisite function.
Strength (MPa) Mix Code Mix Description Applications / intended use
32.0 VE322EAMF S32@56D 20mm 120SL ECOPactMAX
FIB CONC General
Production Sites
Laverton, Truganina, Footscray, Epping, Keilor,
Preston, Oaklands Junction, Melbourne Airport,
Bayswater, Springvale, Lyndhurst, Seaford,
Pakenham, Hastings, Rosebud
Content Declaration
The gross weight of this declared material is 2,400 kg per cubic meter makes up a minimum of 99% of the products
covered by this EPD. The following table provides a summary of the materials included in Holcim ready-mix concrete
and their relative composition by weight.
Material % by weight
Post-consumer
recycled material,
weight % of product
Biogenic material, weight-%
of product Biogenic material, kg C/m3
General purpose
cement
5 - 21 0.0 0.0 0.0
Aggregate 67 - 84 0.0 0.0 0.0
Supplementary
cementitious
materials
0 - 11 0.0 0.0 0.0
Water 11.6 - 12 0.0 0.0 0.0
Admixtures 0.0 0.0 0.0 0.0
Holcim Ready-mix concrete is classified as Non-Dangerous Goods according to the Australian Code for the Transport
of Dangerous Goods by Road and Rail. The safety data sheet for pre-mixed concrete lists all associated hazard
phrases. None of the products contain one or more substances that are listed in the “Candidate List of Substances of
Very High Concern for authorisation”. According to the PCR 2019:14, if one or more substances of the “Candidate List
of Substances of Very High Concern (SVHC) for authorisation” are present in a product and their total content
exceeds 0.1% of the weight of the product, they need to be reported.
Holcim - Ready-Mix Concrete - EPD 10

-- 10 of 20 --

Packaging
Holcim ready-mix concrete is delivered in bulk with no packaging.
Recycled Material
BS EN 16757:2017 specifically lists the following materials relevant to the study as co-products:
 Fly ash,
 Ground granulated blast furnace slag; and
 Silica fume.
As such, the above materials are considered as co-products of their production process and the impacts for their
production process are allocated according to PCR 2019:14 Construction Products and Construction Services (co-
produced goods, multi-output allocation).
Default background data from LCA databases was used to model the above co-products:
 Fly ash: AusLCI process for fly ash treats it as a waste material and only includes transport impacts.
 Ground granulated blast furnace slag: the AusLCI process for slag is allocated based on economic value, as
the product has a significant economic value at the point of collection.
 Silica fume: the ecoinvent process for silica fume treat it as a waste material and only includes transport
impacts.
The allocation approach of the AusLCI LCA database was adopted as a default for secondary data and processes
(e.g. secondary fuel in cement production). The AusLCI dataset conforms to EN 15804 when applying allocation to its
various processes and sub-processes.
Cradle to Gate (Modules A1 – A3)
Raw materials for producing Holcim’s ready-mix concrete include cementitious materials, aggregates, admixtures,
oxides, fibres, water, and ice. These raw materials are generally transported from various locations around Australia,
China, Indonesia, and Europe. The raw materials are stored in silos, hoppers, ground bins or tanks. The materials are
feed to batching plant hopper with calibrated scale. Then all the raw materials are discharged via a chute into the
ready-mix concrete truck. Water is then weighed, or volume metered and discharged into the mixer truck through the
same charging tank.
Holcim’s ready-mix concrete is manufactured across ACT, NSW, QLD, SA, VIC, and WA, Australia. State-specific
electricity mix available in the AusLCI database is used to model electricity in the foreground processes. The AusLCI
dataset was last updated in 2023.
State Energy source in electricity mix
GWP-GHG
(kg CO2
eq./kWh)
NSW&ACT Black coal (75%), photovoltaic (17%), natural gas (3%), hydropower (3%), others (2%) 0.72
QLD Black coal (71%), natural gas (12%), photovoltaic (8%), oil (4%), others (5%) 0.80
SA Wind power (61%), natural gas (34%), photovoltaic (4%), others (1%) 0.30
VIC Natural gas (44%), brown coal (41%), wind power (8%), hydropower (3%), others (4%) 0.84
WA Natural gas (65%), wind power (26%), black coal (8%), others (1%) 0.57
Gate to Site (Module A4)
Distribution is dependent on the market requirements of ready-mix concrete products. All Holcim ready-mix concrete
products transported in Australia is by EURO5 28t – 32t trucks. The transport distances from manufacturing gate to
the site is 12.22 km. The product weight for 1m3 ready-mix concrete is the sum of weights from all raw material inputs.
Holcim - Ready-Mix Concrete - EPD 11

-- 11 of 20 --

Vehicle Fuel use
(L/tkm)
Fuel
type
Carrying
capacity
Density of
products
Average load
factor
Volume capacity utilization
factor
EURO 5
Truck 1.97E-02 Diesel 28 t – 32 t 2,400 kg/m3 50% <1
Installation (Module A5)
As Holcim does not have operational control over the installation of ready-mix concrete at the construction site,
assumptions for construction inputs and installation waste are made based on industrial expertise and experience,
and the GCCA tool. The inputs account for the pouring of concrete from a ready-mix truck and pump, excluding any
pre-installation activities such as site work and forms. The concrete slabs are then manually finished, and no
additional inputs are required to be modelled.
Construction inputs and waste Value Unit
Concrete losses that go to landfill 3.00E+00 %
Water use 6.69E+02 L
Electricity use 2.78E+00 kWh
Diesel, in building machine 1.67E+00 L
Wastewater 6.69E-01 L
Deconstruction and End of Life (Modules C1 – C4)
EN 15804 (chapter 7.2.3.3) and applicable PCRs discourage the use of the results of modules A1-A3 & (A1-A5 for
services) without considering the results of module C.
Following the supply of ready-mix concrete products, Holcim has no control over the end-of-life fate for their products.
The recommended cradle to gate environmental profile will be based on the most common scenario as the majority of
construction products are generally deconstructed and transported for recycling. The following assumptions have
been used in this study to model deconstruction and end of life scenarios of Holcim’s ready-mix concrete:
 Deconstruction is modelled as the physical process of drilling and removing the concrete. Hydraulic excavator
is assumed as the operating tool for deconstruction. This process is based on ecoinvent v3.9.1 (2023)
database and the diesel used is extracted from the process.
 100% of the products (2,400 kg) are assumed to be separately collected during deconstruction.
 25 km delivery distance to landfilling as well as reprocessing facility is assumed for waste collection process
since there was no primary data available.
 Assume 80% of the product is reprocess / recycled as Module C3. This is based on the 2022 National Waste
Report (DCCEEW, 2023).
 The remaining waste concrete undergoes inert waste landfill as Module C4.
Module Parameter Value Unit
C1 – Deconstruction Diesel 1.31E-01 L
C2 – Transportation Distance to processing 2.50E+01 km
C3 – Waste processing Concrete recycling 1.92E+03 kg
C4 – Final disposal Inert waste landfill 4.80E+02 kg
Benefits and loads beyond the system boundary (Module D)
The recycling and recovery rate of waste concrete is 80% based on the National Waste Report rate (DCCEEW, 2023).
The end-of-life recyclers process the waste concrete into a recycled aggregate, which can be replaced with virgin
coarse aggregate for a range of applications depending on the products performance requirements.
Holcim - Ready-Mix Concrete - EPD 12

-- 12 of 20 --

ENVIRONMENTAL PERFORMANCE
The environmental impacts considered in this EPD are listed in the table below. EN 15804 reference package based
on EF 3.1 (Environmental Footprint) or a later version has been used. All further tables from this point will contain
abbreviation only.
Impact Category Abbreviation Measurement Unit
Potential Environmental Impact indicators
Total global warming potential GWP – T kg CO2 equivalents (GWP100)
Global warming potential (fossil) GWP – F kg CO2 equivalents (GWP100)
Global warming potential (biogenic) GWP – B kg CO2 equivalents (GWP100)
Global warming potential (land use/ land transformation) GWP – Luluc kg CO2 equivalents (GWP100)
Ozone depletion potential ODP kg CFC 11 equivalents
Acidification potential AP mol H+ eq.
Eutrophication – aquatic freshwater EP – freshwater kg P equivalent
Eutrophication – aquatic marine EP - marine kg N equivalent
Eutrophication – terrestrial EP – terrestrial mol N equivalent
Photochemical ozone creation potential POCP kg NMVOC equivalents
Abiotic depletion potential (elements)* ADPE kg Sb equivalents
Abiotic depletion potential (fossil fuels)* ADPF MJ net calorific value
Water Depletion Potential* WDP m3 equivalent deprived
Resource use indicators
Use of renewable primary energy excluding renewable primary
energy resources used as raw materials PERE MJ, net calorific value
Use of renewable primary energy resources used as raw
materials PERM MJ, net calorific value
Total use of renewable primary energy resources (primary
energy and primary energy resources used as raw materials) PERT MJ, net calorific value
Use of non-renewable primary energy excluding non-renewable
primary energy resources used as raw materials PENRE MJ, net calorific value
Use of non-renewable primary energy resources used as raw
materials PENRM MJ, net calorific value
Total use of non-renewable primary energy resources (primary
energy and primary energy resources used as raw materials) PENRT MJ, net calorific value
Use of secondary material SM kg
Use of renewable secondary fuels RSF MJ, net calorific value
Use of non-renewable secondary fuels NRSF MJ, net calorific value
Use of net fresh water FW m3
Holcim - Ready-Mix Concrete - EPD 13

-- 13 of 20 --

Impact Category Abbreviation Measurement Unit
Waste categories and Output flows indicators
Hazardous waste disposed HWD kg
Non-hazardous waste disposed NHWD kg
Radioactive waste disposed/stored RWD kg
Components for reuse CFR kg
Materials for recycling MFR kg
Materials for energy recovery MFEE kg
Exported energy EE - e MJ per energy carrier
Exported energy, thermal EE - t MJ per energy carrier
Additional environmental impact indicators
Global warming potential, excluding biogenic uptake, emissions and
storage GWP-GHG kg CO2 equivalents (GWP100)
Global warming potential, aligned with the IPCC 2013 Fifth Assessment
Report *
GWP-GHG
(AR5) kg CO2 equivalents (GWP100)
Particulate matter PM disease incidence
Ionising radiation – human health IRP kBq U-235 eq
Eco-toxicity (freshwater)* ETP-fw CTUe
Human toxicity potential – cancer effects* HTP-c CTUh
Human toxicity potential – non cancer effects* HTP-nc CTUh
Soil quality* SQP dimensionless
Potential environmental Impact Indicators (EN15804+A1)
Global warming (GWP100a) – A1 GWP (A1) kg CO2 equivalents
Ozone layer depletion (ODP) – A1 ODP (A1) kg CFC-11 equivalents
Acidification – A1 AP (A1) kg SO2 equivalents
Eutrophication – A1 EP (A1) kg PO43- equivalents
Photochemical oxidation – A1 POCP (A1) kg C2H4 equivalents
Abiotic depletion – A1 ADPE (A1) kg Sb equivalents
Abiotic depletion (fossil fuels) – A1 ADPF (A1) MJ, net calorific value
Global warming (GWP100a) – A1 GWP (A1) kg CO2 equivalents
Additional Greenstar v1.3 Indicators
Human Toxicity cancer Green Star HTc (GS) CTUh
Human Toxicity non-cancer Green Star HTnc (GS) CTUh
Land use Green Star LU (GS) kg C deficit equivalents
Ionising radiation Green Star IR (GS) kBq U-235 equivalents
Particulate Matter Green Star PM (GS) kg PM2.5 equivalents
WSI Green Star WSI (GS) m3 equivalents
*Disclaimer – The results of these environmental impact indicators shall be used with care as the uncertainties on these results are high or as
there is limited experience with the indicator.
**Disclaimer – This impact category deals mainly with the eventual impact of low dose ionizing radiation on human health of the nuclear fuel
cycle. It does not consider effects due to possible nuclear accidents, occupational exposure nor due to radioactive waste disposal in
underground facilities. Potential ionizing radiation from the soil, from radon and from some construction materials is also not measured by this
indicator.
*** - GWP-GHG (IPCC AR5) is an additional GWP100 indicator that is aligned with the Intergovernmental Panel on Climate Change (IPCC)
2013 Fifth Assessment Report (AR5) (IPCC 2013), national greenhouse gas reporting frameworks in Australia and New Zealand and previous
versions of the Construction Products PCR (PCR2019:14v1.11). It excludes biogenic carbon and indirect radiative forcing.
Holcim - Ready-Mix Concrete - EPD 14

-- 14 of 20 --

VIC - Melbourne Metro - ECOPact- VE322EAMF
The use of results of modules A1-A3 or A1-A5, without considering the results of module C may mislead the communication and decision-making. The estimated impact
results are only relative statements, which do not indicate the endpoints of the impact categories, exceeding threshold values, safety margins and/or risks.
PRIMARY ENVIRONMENTAL INDICATORS (in accordance with EN 15804:2012+A2:2019) – 1m3 of ready-mix concrete
Abbreviation Unit A1-A3 A4 A5 C1 C2 C3 C4 D
GWP-Total kg CO2 eq. 105 2.05 8.81 0.532 3.99 7.61 1.28 -15.7
GWP-Fossil kg CO2 eq. 104 2.05 8.79 0.532 3.99 7.60 1.28 -15.7
GWP-Biogenic kg CO2 eq. 0.781 0.000153 0.0240 0.0000409 0.000299 0.00704 0.000230 -0.0216
GWP-Luluc kg CO2 eq. 0.0184 9.54E-7 0.000263 0.0000227 1.86E-6 3.50E-6 0.0000626 -0.0139
ODP kg CFC 11 eq. 1.97E-6 3.18E-7 1.06E-7 7.69E-9 6.21E-7 9.54E-7 1.85E-8 -1.12E-7
AP mol H+ eq. 0.771 0.0130 0.0691 0.00501 0.0254 0.0208 0.0116 -0.0851
EP-F kg PO43- eq. 0.00714 2.08E-7 0.0000531 3.67E-6 4.05E-7 0.0000362 0.0000371 -0.00500
EP-M kg P eq. 0.171 0.00302 0.0295 0.00235 0.00590 0.00370 0.00526 -0.0225
EP-T kg N eq. 2.08 0.0338 0.321 0.0256 0.0659 0.0404 0.0571 -0.235
POCP mol N eq. 0.560 0.00833 0.0937 0.00750 0.0162 0.0108 0.0171 -0.0741
ADPE kg NMVOC eq. 0.0000504 2.34E-9 2.65E-7 2.15E-8 4.56E-9 1.87E-6 4.94E-8 -1.69E-6
ADPF kg Sb eq. 931 27.6 109 6.85 53.9 102 16.0 -193
WDP MJ 40.9 0.178 46.5 0.00908 0.347 2.33 0.0222 -26.1
RESOURCE USE PARAMETERS (in accordance with EN 15804:2012+A2:2019) – 1m3 of ready-mix concrete
Abbreviation Unit A1-A3 A4 A5 C1 C2 C3 C4 D
PERE MJNCV 41.2 0.0398 2.84 0.0118 0.0118 1.86 0.0712 -16.8
PERM MJNCV 0 0 0 0 0 0 0 0
PERT MJNCV 41.2 0.0398 2.84 0.0118 0.0118 1.86 0.0712 -16.8
PENRE MJNCV 931 27.6 109 6.85 6.85 102 16.0 -193
PENRM MJNCV 0 0 0 0 0 0 0 0
PENRT MJNCV 931 27.6 109 6.85 6.85 102 16.0 -193
SM kg 286 0 0 0 0 0 0 0
RSF MJNCV 0 0 0 0 0 0 0 0
NRSF MJNCV 0 0 0 0 0 0 0 0
FW m3 0.840 0.00411 0.593 0.000346 0.000346 0.0368 0.000837 -0.635
Holcim - Ready-Mix Concrete - EPD 15

-- 15 of 20 --

WASTE CATEGORIES AND OUTPUT FLOWS (in accordance with EN 15804:2012+A2:2019) – 1m3 of ready-mix concrete
Abbreviation Unit A1-A3 A4 A5 C1 C2 C3 C4 D
HWD kg 0.00241 6.56E-6 0.000545 0.0000460 0.0000128 0.0000305 0.000103 -0.000466
NHWD kg 0.884 0.00125 69.0 0.000513 0.00244 0.104 460 -0.679
RWD kg 0.0000577 1.70E-9 4.00E-6 2.64E-7 3.32E-9 5.95E-7 9.47E-7 -0.000435
CRU kg 0 0 0 0 0 0 0 0
MFR kg 0.00371 0 0 0 0 0 0 0
MFRE kg 0 0 0 0 0 0 0 0
EE - e MJ 0 0 0 0 0 0 0 0
EE - t MJ 0 0 0 0 0 0 0 0
ADDITIONAL ENVIRONMENTAL IMPACT INDICATORS (in accordance with EN 15804:2012+A2:2019) – 1m3 of ready-mix concrete
Abbreviation Unit A1-A3 A4 A5 C1 C2 C3 C4 D
GWP-GHG kg CO2 eq. 105 2.05 8.81 0.532 3.99 7.61 1.28 -15.7
GWP-GHG (AR5) kg CO2 eq. 110 2.02 8.65 0.521 3.95 7.56 1.25 -15.2
PM disease incidence 0.0000667 1.98E-7 1.76E-6 1.41E-7 3.86E-7 1.38E-7 3.20E-7 -1.27E-6
IRP kBq U-235 eq 100.0 0.0000483 0.0191 0.00132 0.0000942 0.00422 0.00439 -1.79
ETP-fw CTUe 274 8.04 34.3 2.80 15.7 27.0 6.25 -31.4
HTP-c CTUh 7.38E-8 6.86E-11 4.05E-10 2.01E-11 1.34E-10 1.26E-9 7.11E-11 -1.55E-9
HTP-nc CTUh 2.47E-6 4.90E-9 3.34E-8 2.33E-9 9.55E-9 3.93E-8 1.11E-8 -1.11E-7
SQP dimensionless 103 0.124 9.64 0.0119 0.242 20488 19.0 -125
ADDITIONAL ENVIRONMENTAL IMPACT INDICATORS (in accordance with EN 15804:2012+A1:2013) – 1m3 of ready-mix concrete
Abbreviation Unit A1-A3 A4 A5 C1 C2 C3 C4 D
GWP (A1) kg CO2 eq. 109 2.02 8.63 0.520 3.94 7.55 1.24 -15.2
ODP (A1) kg CFC 11 eq. 1.97E-6 3.18E-7 1.06E-7 7.69E-9 6.21E-7 9.54E-7 1.85E-8 -1.12E-7
AP (A1) kg SO2 eq. 0.771 0.0130 0.0691 0.00501 0.0254 0.0208 0.0116 -0.0851
EP (A1) kg PO43- eq. 0.0926 0.00123 0.0102 0.000805 0.00240 0.00198 0.00189 -0.0230
POCP (A1) kg C2H4 eq. 0.560 0.00833 0.0937 0.00750 0.0162 0.0108 0.0171 -0.0741
ADPE (A1) kg SO2 eq. 0.0000504 2.34E-9 2.65E-7 2.15E-8 4.56E-9 1.87E-6 4.94E-8 -1.69E-6
ADPF (A1) MJ 931 27.6 109 6.85 53.9 102 16.0 -193
Holcim - Ready-Mix Concrete - EPD 16

-- 16 of 20 --

ADDITIONAL GREEN STAR (V1.3) IMPACT INDICATORS – 1m3 of ready-mix concrete
Abbreviation Unit A1-A3 A4 A5 C1 C2 C3 C4 D
HTc (GS) CTUh 2.95E-9 1.33E-11 1.30E-10 3.31E-12 2.60E-11 1.22E-10 1.27E-11 -2.81E-10
HTnc (GS) CTUh 5.98E-10 4.15E-12 6.60E-11 2.39E-13 8.10E-12 4.92E-11 6.15E-13 -8.94E-12
LU (GS) kg C deficit eq. 4.28 0.00186 0.262 0.00592 0.00362 2179 1.36 -392
IR (GS) kBq U235 eq. 0.247 0.0000483 0.0192 0.00132 0.0000943 0.00422 0.00440 -1.79
PM (GS) kg PM2.5 eq. 0.0000667 1.98E-7 1.76E-6 1.41E-7 3.86E-7 1.38E-7 3.20E-7 -1.27E-6
WSI (GS) m3 1.67 0.00582 2.23 0.000430 0.0113 0.102 0.000977 -0.835
Holcim - Ready-Mix Concrete - EPD 17

-- 17 of 20 --

OTHER LIFE CYCLE STAGES NOT
INCLUDED IN THIS EPD
While the LCA study and EPD only consider the cradle to gate (modules A1-A3) with options modules A4-A5, modules
C1-C4 and module D of the environmental impacts of Holcim’s ready-mix concrete, practitioners using the EPD for the
purpose of whole-of-life building studies or the functional comparison of different building products on a whole-of-life
basis will consider concrete’s other life cycle stages. Some of the environmental impacts of benefits associated with
other life cycle stages not included in this EPD are described in the following sections.
Lifetime absorption of CO2
Carbonation is a natural process whereby concrete absorbs carbon dioxide (CO2) from the atmosphere through a
chemical reaction between the CO2 in the ambient air and hydration products within the concrete (CaOH2). Ready-mix
concrete can be subject to carbonation from the use stage onward (i.e. after construction and curing). From a life cycle
impact accounting perspective, this process can also be referred to as ‘reabsorption’, since the CO2 emitted during the
cement manufacturing process can be partly offset by the lifetime absorption of CO2, therefore reducing the net CO2
emissions associated with concrete over its lifetime.
The carbonisation process is a commonly known process in building design and is typically taken into consideration by
engineers when specifying special-class concrete.
The total amount of CO2 absorption during the life cycle of concrete is subject to a range of factors and varies over
time. The calculation has been standardised in the British and European Standard BS EN 16757:2017 Sustainability
of construction works – Environmental Product Declarations – Product Category Rules for concrete and concrete
elements. It is recommended that practitioners make use of this standard when conducting whole-of-life building
studies and if the building materials include substantial amounts of concrete. Please note that CO2 absorption has not
been considered in this EPD and is not reflected in the EPD results tables.
Holcim - Ready-Mix Concrete - EPD 18

-- 18 of 20 --

REFERENCES
AusLCI. (2023) AusLCI Database – v1.42. Retrieved from AusLCI: www.auslci.com.au/
Australasian EPD Programme. (2017). Guidance on the use of INA in EPDs.
Australasian EPD Programme. (2018). Guidance on the use of background LCI data.
Australasian EPD Programme. (2024). Instructions of the Australasian EPD Programme V4.2.
Australian Life Cycle Inventory Database Initiative (AusLCI). (2023). Guidelines for Data Development for an
Australian Life Cycle Inventory Database, Data Standard.
British Standards Institution. (2019). Sustainability of construction works. Environmental product declarations. Core
rules for the product category of construction products, BS EN 15804:2012+A2:2019. British Standards Institution.
British Standards Institution. (2017). Sustainability of construction works – Environmental product declarations –
Product Category Rules for concrete and concrete elements, BS EN 16757:2017. British Standards Institution.
Department of Climate Change, Energy, the Environment and Water. (2023). National Waste Report 2022. Retrieved
from https://www.dcceew.gov.au/environment/protection/waste/national-waste-reports/2022.
Ecoinvent Centre. (2023). Ecoinvent version 3.9.1 database. Zurich: ETH, Agroscope, EMPA, EPFL, PSI. Retrieved
from www.ecoinvent.org.
EPD International. (2024). General Programme Instructions (GPI) for the International EPD System V5.0. Retrieved
from www.envirodec.com.
EPD International. (2024). Product Category Rules for Construction Products and Construction Services, PCR2019:14
v1.3.4. Stockholm: EPD International.
European Committee for Standardization. (2022). Sustainability of construction works - Environmental product
declarations - Product Category Rules for concrete and concrete elements, EN 16757:2022. European Committee for
Standardization.
ISO. (2006). Environmental labels and declarations – Type III environmental declarations – Principles and procedures,
ISO 14025:2006. Geneva: International Organization for Standardization.
ISO. (2006). Environmental management – Life cycle assessment – Principles and framework, ISO 14040:2006.
Geneva: International Organization for Standardization.
ISO. (2018). Environmental management. Life cycle assessment. Requirements and guidelines, ISO
14044:2006+A1:2018. Geneva: International Organization for Standardization.
Green Building Council of Australia. (2022). An upfront conversation about upfront carbon. Retrieved from GBCA:
https://new.gbca.org.au/news/gbca-news/upfront-conversation-about-upfront-carbon/
Man Yu, Thomes Wiedmann, Robert Crawford, Catriona Tait, ‘The Carbon Footprint of Australia’s Construction
Sector’, Procedia Engineering, Volume 180, 2017, Pages 211-220, ISSN 1877-7058,
(http://www.sciencedirect.com/science/article/pii/S1877705817316879)
World Green Building Council. (2019). Bringing embodied carbon upfront. Retrieved from World Green Building
Council: https://worldgbc.org/advancing-net-zero/embodied-carbon/
Holcim - Ready-Mix Concrete - EPD 19

-- 19 of 20 --

Contact your Holcim representative today for more information.
Customer Service Centre 131 188
Holcim (Australia) Pty Ltd
Level 40/100 Miller St,
North Sydney NSW 2060, Australia
Phone 02 9412 6600
ABN 87 099 732 297
www.holcim.com.au
This publication supersedes all previous literature on this subject. As the specifications and details
contained in this publication may change, please check with Holcim Customer Service for
confirmation of current issue. This publication provides general information only and is no substitute
for professional technical engineering advice. Users must make their own determination as to the
suitability of this information or any Holcim product for their specific circumstances. Holcim accepts
no liability for any loss or damage resulting from their specific circumstances. Holcim accepts no
liability for a loss or damage resulting from any reliance on the information provided in this
publication. Holcim is a registered trademark of Holcim Ltd.
© 2025 Holcim (Australia) Pty Ltd ABN 87 732 297. All rights reserved.
This guide or any part of it may not be reproduced without prior written consent of Holcim.
Holcim - Ready-Mix Concrete - EPD 20

-- 20 of 20 --

