GE322LPF2
Hutchinson Builders - Woolworths
Doolandella
QUEENSLAND - BRISBANE
Environmental Product Declaration
In Accordance with Environdec c-PCR-003 Concrete, concrete elements (EN 16757:2023), ISO 14025
and EN15804:A2
Programme Operator: EPD International AB
Regional Programme: EPD Australasia
An EPD should provide current information and may be updated or depublished if conditions change. To
find the latest version of the EPD and to confirm its validity, see www.environdec.com.
EPD Registration Number:
Date of Publication:
Valid Until:
Date of Version: 1.0 2024-11-19
2029-11-19
2024-11-19
EPD-IES-0014785:001

-- 1 of 24 --

Contents
1. Heidelberg Materials story
2. Life cycle and process
3. Product environmental performance
4. References
2

-- 2 of 24 --

Heidelberg
Materials
Australia

-- 3 of 24 --

Heidelberg Materials is one of the
world’s largest building materials
companies focused on producing
materials to build our future.
Who is Heidelberg Materials?
Overview | Heidelberg Materials
50 countries
51,000 employees
3,000 locations
4
Leading market positions in cement,
aggregates and ready-mixed concrete.
Revenue in 2023 – 21.2 Billion Euro
4

-- 4 of 24 --

With more than 4,000 employees across 300 sites,
we have an extensive production and logistics
network across Australia.
We think global and act local - we benefit from
global research and development enhanced by
national collaboration to offer a comprehensive
range of high-quality concrete, aggregates, road
base, sand and asphalt products. We also produce a
wide range of sustainable and recycled construction
materials for civil construction and infrastructure
projects.
We are driven by excellence and high performance
and together we will shape Australia’s construction
materials industry building a legacy for generations
to come.
Global expertise, Local experience

-- 5 of 24 --

6

-- 6 of 24 --

Life Cycle and
Process

-- 7 of 24 --

Product EPD Process
• This EPD Process is certified using GCCA international modelling of energy use and environmental
impact to obtain a suitable estimation for products manufactured.
• Pre-defined cement and clinker data provided by the GCCA tool are used only where no better
(supplier/source specific) information is available.
Assumptions & Limitations
Heidelberg Materials EPD
8 In Accordance with Environdec c-PCR-003 Concrete, concrete elements (EN 16757),
ISO 14025 and EN15804:A2
• The average bill of materials (BOM) for the concrete mix selected in the range of concrete plants
specified including their average raw material travel distance, or the calculated BOM based on
actual delivered materials incl. travel distances (average or specific) for the producing plants.
• The average fuel, water and energy consumption per declared unit between those plants;
• Plant production waste based on a nationally calculated figure;
• Recarbonation of concrete is determined through pre-defined values within GCCA tool for the
type of construction project (-3.167644102 kg CO2 eq./ m³ at Stage B, -1.069641016 kg CO2 eq./
m³ at Stage C3, and -2.722027046 kg CO2 eq./ m³ at Stage C4), where known; and,
• End of life recycling is based upon industry data.
Declared Unit is 1m3 of Concrete
• The process is used to produce an accurate estimation at all stages of the product life cycle from
cradle to grave. Estimation at each stage is based on actual data which is a combination of both
current and prior year average consumption per declared unit.
Life Cycle Assessment Tool
• For the purposes of creating this Environmental Product Declaration (EPD), the Global Cement &
Concrete Association (GCCA) concrete EPD tool v. 4.2 (short: GCCA tool) has been employed.
EPDs are created under either of 2 streams:
• Generic Stream - The class of product modelled is used for a particular geographical region using
averaged data across operations.
• Project-specific stream – Models the manufacture of specific products required for a particular
project being delivered from specific plant(s) using weighted average data where relevant and
possible. Reports created after the completion of a project offer the highest accuracy, including
all mix variations for each delivery.
The main data categories include:
• This is a project-specific EPD.
• All modelling assumptions adopted from the GCCA Tool.
• Raw material (inbound) transport distances is the previous year’s travel distance average
weighted according to deliveries across operations.
• Concrete mixes are assumed to use an equal amount of site fuel and energy and responsible for
an equal amount of waste flows.
• Agreed mixes are used to calculate the BOMs. Production is assumed to be equal across all plants
included in the study. Concrete plants in the study include: Jindalee, Coopers Plains, Ipswich
• The project-specific travel distances for diesel truck from the main plant to the construction site
were applied. Truck type of >32 tonne was assumed to be fully utilized travelling to construction
site with empty returns.
• Water usage in operations is averaged over the full geographic region of study.
• Grid purchased electricity mixes is based on the specific state’s energy mix from OpenNEM. For
this project, energy mix was sourced from coal and peat (66%), gas (7%), solar (21%), wind (4%),
hydro (2%), and biomass (<1%). The electricity emission (GWP-GHG) is 0.83 kg CO2e/kWh.
• Travel for materials sources internationally included from shipping origin.
• Reference Service Life (RSL) is set to 50 years as per default. It's based on the lowest exposure
class A1 & A2 (AS 3600:2018 "Concrete Structures") in relatively benign environments.

-- 8 of 24 --

Hazard information related to concrete placement
GHS classifications
• Skin Corrosion Category 1
• Serious Eye Damage –Category 1
• Skin Sensitisation Category 1
• Specific Target Organ Toxicity (Repeated Exposure) Category 2
Hazard Statement(s)
• H302 –Harmful if swallowed
• P280 –Wear protective gloves/clothing/eye protection.
• H314 –Causes severe skin burns and eye damage
• H317 –May cause an allergic skin reaction
• H318 – Causes serious eye damage
• H373 –May cause damage to lungs by inhalation (dust from dried product)
Product EPD Process
By-Products, Recycled Materials & Allocations
Co-products would be allocated via economic allocations and then normalized based on BOM. The
following materials are the product of waste streams of other industrial processes:
Fly ash
• A by-product of coal-fired power stations, fly ash is considered to carry no environmental impact
for the purposes of this EPD, hence an economic allocation of $0 has been applied to fly ash. The
only burdens are of transport to manufacturing sites.
Ground Granulated Blast Furnace Slag (GGBFS)
• Blast furnace slag is a by-product of steel production that is dried and ground for use in concrete
production. To duly allocate the environmental impacts, economic allocation has been employed.
Silica fume
• As a by-product of silicon production, silica fume is considered to carry no environmental burden
for the purposes of this EPD.
Recycled concrete aggregate
• A component of the boarder category of construction and demolition waste, environmental
impacts are allocated on the basis of reprocessing the material following delivery to the recycling
facility.
Manufactured Sand
• A by-product of processing coarse aggregate. This manufactured sand is a direct replacement for
natural sand and prevents the need to extract natural resources.
Packaging
• This concrete is not produced with any packaging, instead delivered directly to site immediately
following production.
Heidelberg Materials EPD
9 In Accordance with Environdec c-PCR-003 Concrete, concrete elements (EN 16757),
ISO 14025 and EN15804:A2
Bill of Materials Low Level [%] High Level [%]
Cement 4 13
Supplementary Cementitious Materials 0 13
Aggregates 59 86
Water 7 15
Admixtures 0 <1
Reinforcements 0 <1
The materials (by mass%) contained in Hutchinson Builders - Woolworths Doolandella mixes are
summarized in the table above.

-- 9 of 24 --

Product Lifecycle Stages
• All stages of the product lifecycle
have been considered for this EPD –
cradle to grave. By its nature, there
are some stages of the lifecycle that
are not applicable to the concrete
product.
• The scenario applied for the use
stage assumes that under normal
use, no maintenance repair or
replacement of the product during its
service life is required. As a result,
the values are displayed as zero.
• Those stages that, due to
practicality, cannot be assessed
accurately draw on default values of
the underlying GCCA tool.
• For Project-specific EPDs, allocation
is determined by the supplying plants
with estimates as to the likely
volume to be delivered from each.
Where existing and sufficient data
exists, historical data will be used to
make this determination.
Heidelberg Materials EPD
10
Product Stage Construction
Stage Use Stage End of Life Stage
Benefits & loads
for the next
product system
Raw Material Supply
Transport
Manufacturing
Transport
Construction/installation process
Use
Maintenance incl. transport
Repair incl. transport
Replacement incl. transport	
Refurbishment incl. transport
Operational Energy Use	
Operational Water Use
De
-construction & demolition
Transport
Re
-use recycling
Final Disposal
Reuse, Recovery Recycling
Module A1 A2 A3 A4 A5 B1 B2 B3 B4 B5 B6 B7 C1 C2 C3 C4 D
Modules
declared X X X X X X X X X X X X X X X X X
Geography GLO GLO AU AU AU AU AU AU AU AU AU AU AU AU AU AU AU
Specific
data 77%
Variation
products Not Relevant
Variation
sites <10%

-- 10 of 24 --

Product Lifecycle Stages
• The lifecycle model and system boundary is the same for
both Generic and Project-specific concrete EPDs, as
detailed in the graphic.
• All stages of the lifecycle, from quarry to recycling are
covered by the EPD.
Cut-off rules
The cut-off threshold for the LCA study was flows
contributing less than 1% for any individual input included in
the LCA. No flows were deliberately excluded due to this
threshold, however particularly minor impacts (e. g.
packaging of chemical admixtures) were not considered. Cut
off will occur only when data, or reliable estimates, are not
practical to source. The contribution of capital goods
(production equipment and infrastructure) and personnel are
non-attributable and excluded for the system boundary.
Heidelberg Materials EPD
11

-- 11 of 24 --

Product Data Sources
Heidlelberg Materials EPD
12
LCA Stage Item Source Timing Data
Source
Data Quality
Geographical Technical Time
Product
Description
Product description and
density
ERP report Bill of Materials and material specific data Upon EPD creation Primary Very good Very good Very good
A1-3 Materials Raw Materials ERP report BOM and Mix design compilation used in conjunction with material template
Note. Upstream process for raw materials utilise data from ecoinvent 3.5. Specific cement EPD data by the cement
manufacturer was used if available. Published cement EPDs were used to create concrete EPDs.
In the rare case that specific cement data was not possible, region-specific default cement and clinker values
(default values provided by the GCCA tool) would have been used. This would be reflected in “Specific data.”
Upon EPD creation Secondary Very good Good Very good
A1-3 Materials Inbound travel (raw
materials)
ERP report 2. Inbound Travel drawing from actual deliveries from sources to operations.
Where delivery data not available, travel calculated based on Google Maps.
Train travel (only for operations around Melbourne) calculated by actual Google Maps distance.
Full prior year data,
average per delivery
Actual travel distances
between source and
operation.
Primary Very good Good Very good
A1-3 Materials Allocation Factor (for
secondary co products):
Slag: AusLCI
Fly Ash & Silica fume: no allocation as they are industrial by-products.
Upon EPD creation Secondary Very good Good Very good
1-3
Manufacturing
Plant Energy and Fuel
Consumption
ERP Report 3. Concrete Energy Use, drawing on actual invoiced usage. Full prior year data,
average per cubic metre
Primary Very good Very good Very good
A1-3
Manufacturing
Electricity Energy
Sources
Sourced from OpenNEM
https://opennem.org.au; Australian Energy Market Operator. Excludes imports.
Full year prior data, state-
based, percentages
Secondary Very good Very good Very good
A1-3 Waste
Management
Waste and waste water Waste water volume set to 9L per 1 m3 Static Secondary Very good Good Very good
A4-5
Construction
Outbound Travel For generic EPDs: ERP report 5. Outbound travel drawing from actual deliveries from operations to customer sites.
Where data not available, travel calculated based on Google Maps.
For project-specific EPDs: The project-specific travel distances from the main plant to the construction site was
applied.
For both scenarios, diesel truck is used to transport deliveries to customer site/s. A5 uses default GCCA Tool
settings for: 2.8 kWh electricity, 1.7 L diesel in building machine, 669 kg water, and 0.7 m3 wastewater. Note that
internal concrete losses are at ~1% (based on internal reports)
Generic EPD: Full prior year
data, average per delivery.
Project-specific EPD: Actual
travel distances between
plant and construction site.
Primary Very good Good Very good
B. Use Re-carbonation Default GCCA Tool settings NA Proxy Good Good Very good

-- 12 of 24 --

Product Data Sources
Heidlelberg Materials EPD
13
LCA Stage Item Source Timing Data
Source
Data Quality
Geographical Technical Time
C. End of Life
Demolition
Demolition Default GCCA Tool settings (2.674 L diesel in building machine, 0.0365 mg PM2.5, 0.184 mg PM10, 0.139 mg
PM>10). PM refers to particulate matter.
NA Proxy Good Good Very good
C. End of Life
Transport
Transport Default GCCA Tool settings NA Proxy Good Good Very good
C. End of Life
Waste Processing
Recycling Rate at EOL Masonry materials recycling rate obtained from annual National Waste Report published (e. g. for National Waste
Report 2022, page 41, figure 29). Referenced recycling rate is used in industry as closest to concrete-specific value.
National Waste Reports
Prior year National Waste
Report if available. If not,
then latest available
Proxy Good Good Very good
C. End of Life
Disposal
Disposal Rate at EOL Disposal rate inverse of masonry materials recycling rate obtained from annual National Waste Report published
National Waste Reports
Prior year National Waste
Report if available. If not,
then latest available
Proxy Good Good Very good
D Benefits and
Loads
Default GCCA Tool settings NA NA NA NA NA
General General EcoInvent database used by the GCCA tool
Note: This covers environmental information for all raw materials and energy sources. Cement, where data is
available, employs specific raw material and energy data for the product manufacture and for each component
draws on Eco Invent Data.
NA Secondary Very good Good Very good

-- 13 of 24 --

Product environmental
performance

-- 14 of 24 --

Product Environmental Performance
Heidelberg Materials EPD
15
Comment All information about goal and scope necessary for results interpretation are present in the latest version of the “LCA Model” report, available in
GCCA’s Industry EPD Tool.
Declared GWP-GHG results for modules A1-A3 are <10%.
The estimated impact results are only relative statements, which do not indicate the endpoints of the impact categories, exceeding threshold
values, safety margins and/or risks. Since Module C is included in the EPD, the use of Module A1-A3 results without considering the results of
Module C is discouraged.
EF3.0 based EN15804+A2 impact assessment methodology has been is used for the GWP indicators.
The removals and emissions associated with biogenic carbon content of i) the product and ii) the packaging are not significant or even not
relevant in the sector. The only limitation is the uptake of CO2 in A1-A3 (e.g. biobased insulation materials in precast elements or biobased
packaging materials) and reemission in A5 (packaging end-of-life) or C3-C4 (product end-of-life). This does not affect the GWP-tot indicator.
The tool does not calculate the ‘Radioactive waste disposed’ indicator, it is considered not to be significant for the sector.
Core Environmental Impact Indicators GWP-GHG (Global Warming Potential, GHG) • GWP-tot (Global Warming Potential total) • GWP-fos (Global Warming Potential fossil fuels) •
GWP-bio (Global Warming Potential biogenic) • GWP-luc (Global Warming Potential land use and land use change) • ODP (Depletion potential of
the stratospheric ozone layer) • AP (Acidification potential, Accumulated Exceedance) • EP-fw (Eutrophication potential, freshwater) • EP-mar
(Eutrophication potential, fraction of nutrients reaching marine end compartment) • EP-ter (Eutrophication potential, Accumulated Exceedance)
• POCP (Formation potential of tropospheric ozone) • ADPE1 (Abiotic depletion potential for non- fossil resources) • ADPF1 (Abiotic depletion for
fossil resources potential) • WDP1 (Water (user) deprivation potential, deprivation-weighted water consumption)
1 The results of this environmental impact indicator shall be used with care as the uncertainties of the results are high and as there is limited experience with the indicator.

-- 15 of 24 --

Product Environmental Performance
Heidelberg Materials EPD
16
Additional Environmental Impact
Indicators PM (Potential incidence of disease due to PM emissions) • IRP2 (Potential Human exposure efficiency relative to U235) • ETP1 (Potential
Comparative Toxic Unit for ecosystems) • HTPC1 (Potential Comparative Toxic Unit for humans - cancer) • HTPNC1 (Potential Comparative
Toxic Unit for humans - non-cancer) • SQP1 (Potential soil quality index)
Parameters Describing Resource Use PERE (Use of renewable primary energy excluding renewable primary energy resources used as raw materials) • PERM (Use of renewable
primary energy resources used as raw materials) • PERT (Total use of renewable primary energy resources) • PENRE (Use of non renewable
primary energy excluding non-renewable primary energy resources used as raw materials) • PENRM (Use of non-renewable primary energy
resources used as raw materials) • PENRT (Total use of non-renewable primary energy resources) • SM (Use of secondary materials) • RSF
(Use of renewable secondary fuels) • NRSF (Use of non-renewable secondary fuels) • NFW (Net use of fresh water)
Waste Categories HWD (Hazardous waste disposed) • NHWD (Non-hazardous waste disposed) • RWD (Radioactive waste disposed)
Output Flows CRU (Components for re-use) • MFR (Materials for recycling) • MER (Materials for energy recovery) • EE (Exported energy)
Extra Indicators CC1 (Emissions from calcination and removals from carbonation) • CWRS (Emissions from combustion of waste from renewable sources used
in production processes) • CWNRS (Emissions from combustion of waste from non-renewable sources used in production processes) • GWP-
prod (Removals and emissions associated with biogenic carbon content of the bio-based product) • GWP-pack (Removals and emissions
associated with biogenic carbon content of the bio-based packaging)
1 The results of this environmental impact indicator shall be used with care as the uncertainties of the results are high and as there is limited experience with the indicator.
2 This impact category deals mainly with the eventual impact of low dose ionizing radiation on human health of the nuclear fuel cycle. It does not consider effects due to possible nuclear accidents, occupational exposure nor
due to radioactive waste disposal in underground facilities. Potential ionizing radiation from the soil, from radon and from some construction materials is also not measured by this indicator.

-- 16 of 24 --

Product Environmental Performance
Heidelberg Materials EPD
17
[hm_slide1]
Product identification 	GE322LPF2
EPD Registration Number 	EPD-IES-0014785:001
Production site(s) 	Brisbane
Compressive strength 	32
Density 	2355.5 kg/m³
Reference service life 	50 Years
Recycling Rate At EoL 	78%
Declared unit 	1 m3
Scope 	A1-A3 + A4-A5 + B1-B7 + C1-C4 + D, cradle-to-grave
Methodology 	GCCA’s Industry EPD Tool for Cement and Concrete (V4.2), International version
Reference Year 	2023

-- 17 of 24 --

Product Environmental Performance
Heidelberg Materials EPD
18
[hm_slide2]
EPD Registration Number 	EPD-IES-0014785:001
Core environmental impact indicators
A1-A3 A4 A5 B1 B2 B3 B4 B5 B6 B7 C1 C2 C3 C4 D
GWP-GHG kg CO₂ eq. 	1.45E+02 3.41E+00 1.01E+01 -3.17E+00 0.00E+00 0.00E+00 0.00E+00 0.00E+00 0.00E+00 0.00E+00 8.99E+00 9.03E+00 5.19E+00 2.85E+00 -1.41E+01
GWP-tot kg CO₂ eq. 	1.45E+02 3.41E+00 1.01E+01 -3.17E+00 0.00E+00 0.00E+00 0.00E+00 0.00E+00 0.00E+00 0.00E+00 8.99E+00 9.03E+00 5.19E+00 2.85E+00 -1.41E+01
GWP-fos kg CO₂ eq. 	1.45E+02 3.41E+00 1.01E+01 -3.17E+00 0.00E+00 0.00E+00 0.00E+00 0.00E+00 0.00E+00 0.00E+00 8.99E+00 9.01E+00 5.16E+00 2.84E+00 -1.40E+01
GWP-bio kg CO₂ eq. 	4.83E-02 1.33E-03 4.38E-03 0.00E+00 0.00E+00 0.00E+00 0.00E+00 0.00E+00 0.00E+00 0.00E+00 1.60E-03 6.45E-03 1.93E-02 1.88E-03 -5.65E-02
GWP-luc kg CO₂ eq. 	3.21E-02 1.15E-03 3.34E-03 0.00E+00 0.00E+00 0.00E+00 0.00E+00 0.00E+00 0.00E+00 0.00E+00 1.13E-03 5.24E-03 1.47E-02 1.53E-03 -2.45E-02
ODP kg CFC 11 eq. 	6.63E-06 6.49E-07 1.30E-06 0.00E+00 0.00E+00 0.00E+00 0.00E+00 0.00E+00 0.00E+00 0.00E+00 1.62E-06 1.52E-06 3.71E-07 9.27E-07 -9.57E-07
AP mol H+ eq. 	6.89E-01 1.76E-02 9.03E-02 0.00E+00 0.00E+00 0.00E+00 0.00E+00 0.00E+00 0.00E+00 0.00E+00 9.42E-02 5.45E-02 3.93E-02 2.73E-02 -9.94E-02
EP-fw kg P eq. 	3.01E-02 2.54E-04 2.05E-03 0.00E+00 0.00E+00 0.00E+00 0.00E+00 0.00E+00 0.00E+00 0.00E+00 4.02E-04 1.21E-03 3.06E-03 3.34E-04 -5.88E-03
EP-mar kg N eq. 	2.23E-03 2.21E-05 6.88E-04 0.00E+00 0.00E+00 0.00E+00 0.00E+00 0.00E+00 0.00E+00 0.00E+00 3.34E-05 8.91E-05 2.12E-04 3.15E-05 -3.81E-04
EP-ter mol N eq. 	1.54E+00 6.31E-02 3.32E-01 0.00E+00 0.00E+00 0.00E+00 0.00E+00 0.00E+00 0.00E+00 0.00E+00 4.44E-01 1.92E-01 7.34E-02 9.77E-02 -2.48E-01
POCP kg NMVOC eq. 	4.24E-01 1.90E-02 9.15E-02 0.00E+00 0.00E+00 0.00E+00 0.00E+00 0.00E+00 0.00E+00 0.00E+00 1.22E-01 5.61E-02 2.07E-02 2.87E-02 -6.28E-02
ADPE kg Sb eq. 	1.80E-04 6.35E-06 7.31E-06 0.00E+00 0.00E+00 0.00E+00 0.00E+00 0.00E+00 0.00E+00 0.00E+00 2.66E-06 1.59E-05 4.57E-06 3.10E-06 -1.60E-04
ADPF MJ, net calorific value 1.10E+03 5.36E+01 1.29E+02 0.00E+00 0.00E+00 0.00E+00 0.00E+00 0.00E+00 0.00E+00 0.00E+00 1.30E+02 1.34E+02 7.63E+01 7.92E+01 -1.61E+02
WDP m³ world eq. deprived 7.54E+01 3.95E-01 -1.38E+00 0.00E+00 0.00E+00 0.00E+00 0.00E+00 0.00E+00 0.00E+00 0.00E+00 7.67E-01 1.17E+00 1.07E+00 3.83E+00 -2.73E+01
Parameters describing resource use
A1-A3 A4 A5 B1 B2 B3 B4 B5 B6 B7 C1 C2 C3 C4 D
PERE MJ, net calorific value 4.81E+01 1.55E+00 5.52E+00 0.00E+00 0.00E+00 0.00E+00 0.00E+00 0.00E+00 0.00E+00 0.00E+00 7.59E-01 4.92E+00 8.34E+00 2.06E+00 -1.32E+01
PERM MJ, net calorific value 0.00E+00 0.00E+00 0.00E+00 0.00E+00 0.00E+00 0.00E+00 0.00E+00 0.00E+00 0.00E+00 0.00E+00 0.00E+00 0.00E+00 0.00E+00 0.00E+00 0.00E+00
PERT MJ, net calorific value 4.81E+01 1.55E+00 5.52E+00 0.00E+00 0.00E+00 0.00E+00 0.00E+00 0.00E+00 0.00E+00 0.00E+00 7.59E-01 4.92E+00 8.34E+00 2.06E+00 -1.32E+01
PENRE MJ, net calorific value 1.11E+03 5.36E+01 1.29E+02 0.00E+00 0.00E+00 0.00E+00 0.00E+00 0.00E+00 0.00E+00 0.00E+00 1.30E+02 1.34E+02 7.63E+01 7.92E+01 -1.61E+02
PENRM MJ, net calorific value 0.00E+00 0.00E+00 0.00E+00 0.00E+00 0.00E+00 0.00E+00 0.00E+00 0.00E+00 0.00E+00 0.00E+00 0.00E+00 0.00E+00 0.00E+00 0.00E+00 0.00E+00
PENRT MJ, net calorific value 1.11E+03 5.36E+01 1.29E+02 0.00E+00 0.00E+00 0.00E+00 0.00E+00 0.00E+00 0.00E+00 0.00E+00 1.30E+02 1.34E+02 7.63E+01 7.92E+01 -1.61E+02
SM kg 	1.63E+02 0.00E+00 1.63E+00 0.00E+00 0.00E+00 0.00E+00 0.00E+00 0.00E+00 0.00E+00 0.00E+00 0.00E+00 0.00E+00 0.00E+00 0.00E+00 0.00E+00
RSF MJ, net calorific value 2.29E+00 0.00E+00 2.29E-02 0.00E+00 0.00E+00 0.00E+00 0.00E+00 0.00E+00 0.00E+00 0.00E+00 0.00E+00 0.00E+00 0.00E+00 0.00E+00 0.00E+00
NRSF MJ, net calorific value 3.81E+01 0.00E+00 3.81E-01 0.00E+00 0.00E+00 0.00E+00 0.00E+00 0.00E+00 0.00E+00 0.00E+00 0.00E+00 0.00E+00 0.00E+00 0.00E+00 0.00E+00
NFW m³ 	2.14E+00 1.18E-02 1.18E-01 0.00E+00 0.00E+00 0.00E+00 0.00E+00 0.00E+00 0.00E+00 0.00E+00 1.99E-02 3.60E-02 4.34E-02 8.92E-02 -6.53E-01

-- 18 of 24 --

Product Environmental Performance
Heidelberg Materials EPD
19
[hm_slide3]
EPD Registration Number 	EPD-IES-0014785:001
Additional environmental impact indicators
A1-A3 A4 A5 	B1 	B2 	B3 	B4 	B5 	B6 	B7 	C1 	C2 	C3 	C4 	D
PM 	Disease incidence 	5.84E-06 3.14E-07 1.67E-06 0.00E+00 0.00E+00 0.00E+00 0.00E+00 0.00E+00 0.00E+00 0.00E+00 2.45E-06 8.41E-07 3.51E-07 5.09E-07 -1.17E-06
IRP 	kBq U235 eq. 	4.38E+02 2.82E-01 4.93E+00 0.00E+00 0.00E+00 0.00E+00 0.00E+00 0.00E+00 0.00E+00 0.00E+00 6.08E-01 7.71E-01 8.19E-01 3.66E-01 -1.32E+00
ETP 	CTUe 	4.25E+02 1.13E+01 8.02E+00 0.00E+00 0.00E+00 0.00E+00 0.00E+00 0.00E+00 0.00E+00 0.00E+00 1.76E+00 2.36E+01 1.60E+00 1.50E+00 -6.80E+00
HTPC 	CTUh 	7.64E-07 2.18E-08 1.89E-07 0.00E+00 0.00E+00 0.00E+00 0.00E+00 0.00E+00 0.00E+00 0.00E+00 6.36E-08 1.02E-07 6.35E-08 2.49E-08 -3.36E-07
HTPNC CTUh 	1.08E-05 6.10E-07 8.99E-07 0.00E+00 0.00E+00 0.00E+00 0.00E+00 0.00E+00 0.00E+00 0.00E+00 2.46E-07 1.41E-06 2.92E-07 1.59E-07 -2.00E-06
SQP 	dimensionless 	8.35E+02 9.52E+01 3.81E+01 0.00E+00 0.00E+00 0.00E+00 0.00E+00 0.00E+00 0.00E+00 0.00E+00 7.71E+00 2.19E+02 6.24E+01 1.48E+02 -2.11E+02
Other environmental information describing waste categories
A1-A3 A4 A5 	B1 	B2 	B3 	B4 	B5 	B6 	B7 	C1 	C2 	C3 	C4 	D
HWD 	kg 	0.00E+00 0.00E+00 0.00E+00 0.00E+00 0.00E+00 0.00E+00 0.00E+00 0.00E+00 0.00E+00 0.00E+00 0.00E+00 0.00E+00 0.00E+00 0.00E+00 0.00E+00
NHWD kg 	4.87E-02 0.00E+00 5.16E+00 0.00E+00 0.00E+00 0.00E+00 0.00E+00 0.00E+00 0.00E+00 0.00E+00 0.00E+00 0.00E+00 0.00E+00 5.16E+02 0.00E+00
RWD 	kg 	0.00E+00 0.00E+00 0.00E+00 0.00E+00 0.00E+00 0.00E+00 0.00E+00 0.00E+00 0.00E+00 0.00E+00 0.00E+00 0.00E+00 0.00E+00 0.00E+00 0.00E+00
Environmental information describing output flows
A1-A3 A4 A5 	B1 	B2 	B3 	B4 	B5 	B6 	B7 	C1 	C2 	C3 	C4 	D
CRU 	kg 	0.00E+00 0.00E+00 0.00E+00 0.00E+00 0.00E+00 0.00E+00 0.00E+00 0.00E+00 0.00E+00 0.00E+00 0.00E+00 0.00E+00 0.00E+00 0.00E+00 0.00E+00
MFR 	kg 	0.00E+00 0.00E+00 1.84E+01 0.00E+00 0.00E+00 0.00E+00 0.00E+00 0.00E+00 0.00E+00 0.00E+00 0.00E+00 0.00E+00 1.84E+03 0.00E+00 0.00E+00
MER 	kg 	0.00E+00 0.00E+00 0.00E+00 0.00E+00 0.00E+00 0.00E+00 0.00E+00 0.00E+00 0.00E+00 0.00E+00 0.00E+00 0.00E+00 0.00E+00 0.00E+00 0.00E+00
EE 	kg 	0.00E+00 0.00E+00 0.00E+00 0.00E+00 0.00E+00 0.00E+00 0.00E+00 0.00E+00 0.00E+00 0.00E+00 0.00E+00 0.00E+00 0.00E+00 0.00E+00 0.00E+00
Extra indicators
A1-A3 A4 A5 	B1 	B2 	B3 	B4 	B5 	B6 	B7 	C1 	C2 	C3 	C4 	D
CC 	kg CO₂ eq. 	5.52E+01 0.00E+00 4.83E-01 -3.17E+00 0.00E+00 0.00E+00 0.00E+00 0.00E+00 0.00E+00 0.00E+00 0.00E+00 0.00E+00 -1.07E+00 0.00E+00 0.00E+00
CWRS kg CO₂ eq. 	2.87E-03 0.00E+00 2.87E-05 0.00E+00 0.00E+00 0.00E+00 0.00E+00 0.00E+00 0.00E+00 0.00E+00 0.00E+00 0.00E+00 0.00E+00 0.00E+00 0.00E+00
CWNRS kg CO₂ eq. 	3.23E+00 0.00E+00 3.23E-02 0.00E+00 0.00E+00 0.00E+00 0.00E+00 0.00E+00 0.00E+00 0.00E+00 0.00E+00 0.00E+00 0.00E+00 0.00E+00 0.00E+00
GWP-prod kg CO₂ 	0.00E+00 0.00E+00 0.00E+00 0.00E+00 0.00E+00 0.00E+00 0.00E+00 0.00E+00 0.00E+00 0.00E+00 0.00E+00 0.00E+00 0.00E+00 0.00E+00 0.00E+00
GWP-pack kg CO₂ 	0.00E+00 0.00E+00 0.00E+00 0.00E+00 0.00E+00 0.00E+00 0.00E+00 0.00E+00 0.00E+00 0.00E+00 0.00E+00 0.00E+00 0.00E+00 0.00E+00 0.00E+00

-- 19 of 24 --

Product Environmental Performance
Heidelberg Materials EPD
20
The EPD values presented are indicative of local material performance at the time of publishing and are subject to change based on
material availability and seasonal factors.
1More detailed information is provided in the mix-specific tables and assumptions covered in Life Cycles & Processes section.
Product
Identification EPD Registration Number Compressive strength
[MPa]
A1-A3 GWP-tot1
[kg CO2 eq./m3]
Full Lifecycle GWP-tot1
[kg CO2 eq./m3] Application
CM201AJ53 	EPD-IES-0014780:001 	20 	131 	153 	Block wall
CM251AF41 	EPD-IES-0014781:001 	25 	145 	166 	General works
GE252VW12 	EPD-IES-0014782:001 	25 	129 	152 	General works
GE252WA06 	EPD-IES-0014783:001 	25 	127 	149 	General works
GE322LPE8 	EPD-IES-0014784:001 	32 	141 	164 	General works
GE322LPF2 	EPD-IES-0014785:001 	32 	145 	167 	General works
GE401VC95 	EPD-IES-0014786:001 	40 	180 	203 	General works
GE402AHTK 	EPD-IES-0014787:001 	40 	166 	189 	Slabs
GE402AJAW 	EPD-IES-0014788:001 	40 	243 	264 	Slabs
GE402AJBH 	EPD-IES-0014789:001 	40 	243 	264 	Internal polished slabs
GE402AZRH 	EPD-IES-0014790:001 	40 	244 	265 	Internal polished slabs
GE402ZGR3 	EPD-IES-0014791:001 	40 	170 	194 	Slabs
GE501AU08 	EPD-IES-0014792:001 	50 	261 	282 	General works
P4020120 	EPD-IES-0014793:001 	40 	173 	196 	General works
SS0GSAA14 	EPD-IES-0014794:001 	No guarenteed strength 	109 	122 	Back filling
SYP40SF35 	EPD-IES-0014795:001 	40 	297 	317 	Pump priming
ZLIQ5 	EPD-IES-0014796:001 	No guarenteed strength 	138 	148 	Back filling
ZWP40210 	EPD-IES-0014797:001 	40 	286 	307 	Internal Slabs

-- 20 of 24 --

References

-- 21 of 24 --

22
EPD Owner Heidelberg Materials Australia Pty Ltd
L14, 35 Clarence St, Sydney NSW 2000
Phone: 1300 136 464
Online: www.heidelbergmaterials.com.au
Programme Operator EPD International AB Box 210 60 SE-100 31 Stockholm Sweden
Online: www.environdec.com
Email: info@environdec.com
Regional Programme EPD Australasia Limited, 315a Hardy St, Nelson 7010 New Zealand
Online: epd-australasia.com
Email: info@epd-Australasia.com
Process EPD Certified By Megan Blizzard
Epsten Group, Inc.
101 Marietta St. NW, Suite 2600, Atlanta, Georgia 30303, USA
www.epstengroup.com
Accredited by: A2LA, Certificate #3142.03
Product Category Rules CEN standard EN 15804:A2 (PCR 2019:14 Construction Products, Version 1.3.4) served as the core PCR.
Environdec c-PCR-003 Concrete, concrete elements (EN 16757:2023) served as sub-PCR.
EN 15804 PCR Review The Technical Committee of the International EPD®System. Chair: Claudia A. Peña.
The review panel may be contacted via info@environdec.com.
EPD Registration Number EPD-IES-0014785:001
Independent Verification of the Declaration and
Data, According to ISO 14025:
❑ EPD process certification
❑ EPD verification
Valid From 2024-11-19
Valid To 2029-11-19
Version 1.0 2024-11-19
Description of Version Differences (if NOT VERSION
1.0)
N/A
Geographical Scope QUEENSLAND - BRISBANE
Important Notes EPDs within the same product category but from different programmes may not be comparable.
EPDs of construction products may not be comparable if they do not comply with EN 15804.
The EPD Owner maintains full ownership, liability and responsibility for the EPD.
Product Group Classification UN CPC 88 - Concrete, cement and plaster article manufacturing services
ANZSIC Classification 2033 Ready Mix Concrete Manufacturing
x

-- 22 of 24 --

References
Heidelberg Materials EPD
23
1) Australian Life Cycle Assessment Society. (2015). Australian Life Cycle Inventory Database Initiative. Retrieved from http://www.auslci.com.au
2) National Waste Report. (2022). https://www.dcceew.gov.au/environment/protection/waste/publications/national-waste-reports. Canberra: Department of Climate
Change, Energy, the Environment and Water.
3) Ecoinvent. (2023, Nov 23). ecoinvent 3.5 (database). Retrieved from https://ecoinvent.org
4) EPD International. (2024). General Programme Instructions for the International EPD® System v5.0. Retrieved from envirodec.com
5) EPD Australasia Regional Annex (2024) – Version 4.2 Retrieved from epd-australasia.com
6) European Committee for Standardisation (CEN). (2022). EN 16757:2022: Sustainability of construction works - Environmental product declarations - Product Category
Rules for concrete and concrete elements.
7) European Committee for Standardisation (CEN). (2017, February). EN 16908:2017: Cement and building lime - Environmental Product Declarations - Product Category
Rules complementary to EN 15804. Brussels.
8) European Committee for Standardisation (CEN). (2019). EN 15804:2012+A2:2019: Sustainability of construction works - Environmental product declarations - Core rules
for the product category of construction products. Brussels.
9) Google. (n.d.). Google Maps. Retrieved from https://www.google.com.au/maps/
10) International Organization for Standardization. (2015). ISO14020 Environmental Labels and Declarations - General Principles.
11) International Organization for Standardization. (2017). ISO14025 Environmental Labels and Declarations - Type III Environmental Declarations - Principles and
Procedures.
12) International Organization for Standardization. (2020). ISO 14044 Environmental Management - Life Cycle Assessment - Requirements and Guidelines.
13) McConnell, D., Holmes a Court, S., Tan, S., & Cubrilovic, N. (2022). OpenNEM. Retrieved 2023, from https://opennem.org.au/
14) Quantis. (2024). GCCA's Industry EPD Tool for Cement and Concrete. Retrieved from https://concrete-epd-tool.org/
15) Green Star Mat–4 Concrete Credit User Guide (2012). Retrieved from Mat-4 (gbca.org.au)

-- 23 of 24 --

CO2 service offer
Heidelberg Materials EPD
24
CO2 is set to become a crucial budgeting currency in the construction sector.
As such, it must be managed accordingly. Most provided embodied carbon
emission data out there is based on estimates and typically handed over to
the customer before a project starts.
At Heidelberg Materials Australia, we believe there’s a better way to
communicate carbon values, which also eliminates the current gap of carbon
monitoring options during the construction phase in the market:
1) Pre-project: Predicting - We can provide you indicative CO2 values for
your specific project with our 3rd party verified CO2 calculator (targeted
& fast & reliable).
2) Running project: Monitoring - You get regular updates of your deliveries
and how you track towards your carbon targets (no more surprises).
3) Post-project: Verification - You’ll receive a final report and a project-
specific EPD based on actual deliveries (highest accuracy).
Pre-
Project
Running
Project
Post
Project

-- 24 of 24 --

