ENVIRONMENTAL PRODUCT DECLARATION
IN ACCORDANCE WITH ISO 14025:2006,
EN 15804:2012+A2:2019/AC:2021
PREMIX CONCRETE – S32MPA GREENCRETE 70
Piave Premix Concrete Pty Ltd
ARKER-GEO5
Programme operator: The international EPD® system, www.environdec.com
Regional operator: EPD Australasia Ltd
EPD registration number: EPD-IES-23043
Publication date: 2025-03-31
Valid until: 2030-03-31
Geographical scope: Victoria
Product-specific EPD of one product manufactured at one site.
MOVALMARKER-GEO6
An EPD should provide current information and may be updated if conditions change. The stated validity is therefore subject to the continued
registration and publication at www.environdec.com.

-- 1 of 16 --

2
Premix Concrete – S32MPa GreenCrete 70
PROGRAMME INFORMATION AND
VERTIFICATION
Declaration
Owner:
Owner Piave Premix Concrete Pty Ltd
Address 262 Salmon Street Port Melbourne VIC 3207
Contact details info@piave.com.au
Website https://www.piave.com.au/
EPD
Programme
Operator:
EPD International AB Box 210 60, SE-100 31 Stockholm, Sweden,
Email: info@environdec.com
Regional
Programme:
EPD Australasia Ltd Address: 315a Hardy Street
Nelson 7010, New Zealand
Web: www.epd-australasia.com
Email: info@epd-australasia.com
Phone: +61 2 8005 8206 (AU)
EPD Produced
By:
Crema Constructions Address: 262 Salmon Street
Port Melbourne, VIC 3207, Australia
Web: www.crema.com.au
Email: info@epd-australasia.com
Phone: +61 3 9644 1101 (AU)
EPD Registration Number: EPD-IES-23043
Date of Publication: 2025-03-31
Reference Year for Data: 2022-01-01 to 2022-12-31
Version: 1.0
Valid Until: 2030-03-31
Geographical Scope: Victoria
PCR: PCR 2019:14 Construction Products, Version 1.3.4, 2024-04-
30 (valid until 2025-06-20),
C-PCR-003 (to 2019:14) Concrete and concrete elements,
version 2024-04-30
PCR Review was
Conducted by:
The Technical Committee of the International EPD® System.
See www.environdec.com for a list of members. Most
recent review chair: Claudia A. Peña, University of
Concepción, Chile.
The review panel may be contacted via the Secretariat
www.environdec.com/contact.
Product category
rules
The CEN standard EN 15804 serves as the core PCR. In
addition, the Int’l EPD System PCR 2019:14 Construction
products, version 1.3.4 is used. c-PCR 003 Concrete and
elements
EPD Verifier Andrew D. Moore
Life Cycle Logic Pty Ltd
www.lifecyclelogic.com.au
+61424320057
Andrew@lifecyclelogic.com.au
(External, Third party verifier approved by EPD Australasia
and The International EPD System)
EPD verification Independent verification of this EPD and data, according to
ISO 14025:
☐ Internal verification ☒ External verification
Procedure for follow-
up of data during the
EPD validity involves
third-party verifier
☐ No
☒ Yes
The manufacturer has the sole ownership, liability, and responsibility for the EPD. EPDs within the same product
category but registered in different EPD programmes may not be comparable. For two EPDs to be comparable, they
must be based on the same PCR (including the same version number) or be based on fully-aligned PCRs or versions
of PCRs; cover products with identical functions, technical performances and use (e.g. identical declared/functional
units); have equivalent system boundaries and descriptions of data; apply equivalent data quality requirements,
methods of data collection, and allocation methods; apply identical cut-off rules and impact assessment methods
(including the same version of characterisation factors); have equivalent content declarations; and be valid at the
time of comparison.
EPDs of construction products may not be comparable if they do not comply with EN 15804.

-- 2 of 16 --

3
Premix Concrete – S32MPa GreenCrete 70
PRODUCT IDENTIFICATION
Product name Premix Concrete – S32MPa GreenCrete 70
Additional label(s)
Product number /
reference
S32MPa GreenCrete 70
Production Site: 262 Salmon Street Port Melbourne VIC 3207
CPC code UN CPC 375 (Articles of concrete, cement and
plaster)
ANZSIC 20330 (Concrete – ready mixed – except
dry mix)

-- 3 of 16 --

4
Premix Concrete – S32MPa GreenCrete 70
INTRODUCTION
ABOUT PIAVE
Piave was founded in 1993 by Anthony Schieven and Louis Crema, with a name coined by Loui’s father Beppi, inspired by the Piave river in Northern Italy.
Originally existing predominantly as a means to supply their construction company’s jobs, they built a plant in Port Melbourne, with Anthony managing the
plant and Louis looking after finance and administration.
Piave now supplies a wide range of cementitious products used by the building and construction industry within Victoria.
Since its commencement we’ve set solid foundations for thousands of Melbourne buildings and homes. Now, still family-owned and run, a passionate new
generation is propelling Piave into the future.
OUR COMMITMENT
We understand the crucial role the construction industry has to play in addressing our global carbon crisis, and are committed to playing our part in this journey,
to ensure a brighter outlook for future generations.
SCOPE
This EPD covers premix concrete products for the Victorian metropolitan region. This EPD covers life cycle stages Cradle to gate with modules C1–C4 and module
D (A1–A3 + C + D).

-- 4 of 16 --

5
Premix Concrete – S32MPa GreenCrete 70
PRODUCT INFORMATION
PRODUCT DESCRIPTION
Concrete is prepared by mixing cement, coarse and fine aggregates, and
water, with or without the addition of auxiliary agents and additives. The
fresh concrete is placed on the building site or prefabricated in factory
moulds, compacted, and hardened in the desired shape by the hydration
of cement to form concrete.
PRODUCT APPLICATION
Normal-class - designed for residential applications, low rise buildings,
paving and driveways etc. Its specification and ordering have been
simplified as far as practicable.
Special-class - allows the purchaser to incorporate into the project
specification any special requirements for the project.
PRODUCT STANDARDS
The concrete products within the EPD conform to AS 1379:2007
Specification and Supply of Concrete. General Australian Standard AS 1379
sets down a number of ways of specifying and ordering concrete to
promote uniformity, efficiency and economy in production and delivery. It
refers to two classes of concrete: normal-class and special-class.
Further information can be found at https://www.piave.com.au/.
PRODUCT RAW MATERIAL COMPOSITION
Material Proportion (%
m/m)
Post-consumer
material, weight
(%)
Renewable
material,
weight (%)
Sand 0-85% 0% 0%
Aggregate 0-91% 0% 0%
GP Cement 2-18% 0% 0%
Ground Blast Furnace Slag 0-11% 0% 0%
Silica Fume 0-1% 0% 0%
Water 3-11% 0% 0%
Admixtures <0.4% 0% 0%
The product mass and design mix details are provided in “Piave Premix
Concrete Mix Designs-Final.xlsx” (2025-03-21).
SUBSTANCES, REACH - VERY HIGH CONCERN
removalMarker-svhc1
The product does not contain substances in the Candidate List of
Substances of Very High Concern (SVHC) which exceeds the limits for
registration with the European Chemicals Agency (i.e., if the substance
constitute more than 0.1% of the weight of the product).-svhc3

-- 5 of 16 --

6
Premix Concrete – S32MPa GreenCrete 70
PRODUCT LIFE-CYCLE
MANUFACTURING AND PACKAGING (A1-A3)
The environmental impacts considered for the product stage cover the
manufacturing of raw materials used in the production as well as packaging
materials and other ancillary materials. Also, fuels used by machines, and
handling of waste formed in the production processes at the
manufacturing facilities are included in this stage. The study also considers
the material losses occurring during the manufacturing processes as well
as losses during electricity transmission.
Concrete production is the process of combining water, aggregates,
cementitious binders and additives. These different ‘ingredients’ are
transported from our suppliers to our specialised batching plant. Our
batching plant stores the ingredients in cement silos, aggregate bins and
admixture tanks. The plants use weigh scales and flow meters to accurately
weigh the ingredients which are then mixed in an agitator truck.
PRODUCT END OF LIFE (C1-C4, D)
BS EN 16757:2017 presents four end of life scenarios for concrete:
1. Disposal of concrete at a landfill site,
2. Reuse of recovered concrete elements in new construction works,
3. Use of concrete debris, e.g. In land restoration, or
4. Crushing/recycling of concrete:
a. Crushed concrete substitutes primary material without further
processing, or
Scenarios 2, 3 and 4 can all result in benefits and loads outside the
system boundary and thus should be considered in a whole-of-life
building study or when comparing concrete products on a functional
basis in line with BS EN 16757:2017.
END OF LIFE SCENARIO DETAILS
Scenario parameter Value
Collection process – kg collected separately 2400kg
Collection process – kg collected with mixed waste 0kg
Recovery process – kg for re-use 0kg
Recovery process – kg for recycling 2033kg
Recovery process – kg for energy recovery 0kg
Disposal (total) – kg for final deposition 367kg
Scenario assumptions e.g. transportation 50km
For concrete produced in Victoria, we have used the end-of-life scenario
representative for Victorian building & demolition materials products
based on the National Waste Report 2022 (NWR 2022). This scenario
implies that 84.7% of the concrete is recycled and the remaining 15.3% of
the concrete is sent to landfill.
We have modelled a single scenario for concrete with a density of 2 400
kg/m3. This is a conservative value for the concrete mixes covered by our
EPDs. The impact of this simplification is much smaller than the impact of
the scenario and data assumptions applied to the end-of-life modules.
The concrete collected for recycling reaches end-of-waste status when it
is crushed and stockpiled as “recycled crushed concrete” (RCC)
aggregates. Crushed concrete is assumed to substitute primary (quarried)
material without needing further processing.

-- 6 of 16 --

7
Premix Concrete – S32MPa GreenCrete 70
MANUFACTURING PROCESS

-- 7 of 16 --

8
Premix Concrete – S32MPa GreenCrete 70
LIFE-CYCLE ASSESSMENT
LIFE-CYCLE ASSESSMENT INFORMATION
Period for data 2022-01-01 to 2022-12-31
DECLARED AND FUNCTIONAL UNIT
Declared unit 1m3 of Premix Concrete supplied to the
client
Mass per declared unit 2373 kg
BIOGENIC CARBON CONTENT
The product contains no biogenic carbon and is delivered in bulk without packaging.
SYSTEM BOUNDARY Product stage Assembly
stage
Use stage End of life stage Beyond the
system
boundaries
A1 A2 A3 A4 A5 B1 B2 B3 B4 B5 B6 B7 C1 C2 C3 C
4
D D D
x x x ND ND ND ND ND ND ND ND ND x x x x x x x
Raw materials	
Transport	
Manufacturing	
Transport	
Assembly
Use	
Maintenance	
Repair
Replacement	
Refurbishment	
Operational	
energy use
Operational	
water use	
Deconstruction	
/demolition
Transport
Waste	
processing	
Disposal
Reuse
Recovery
Recycling
Geography AU AU AU - - - - - - - - - - - - - - - -
Share of Specific Data >90%
Variation - products NR
Variation - Sites NR
Included in this study = X. Modules not declared = ND. Modules not relevant = NR

-- 8 of 16 --

9
Premix Concrete – S32MPa GreenCrete 70
CUT-OFF CRITERIA
The study does not exclude any modules or processes which are stated
mandatory in the EN 15804:2012+A2:2019 and the applied PCR. The study
does not exclude any hazardous materials or substances. The study
includes all major raw material and energy consumption. All inputs and
outputs of the unit processes, for which data is available for, are included
in the calculation. There is no neglected unit process more than 1% of total
mass or energy flows. The module specific total neglected input and output
flows also do not exceed 5% of energy usage or mass.
The contribution of capital goods (production equipment and
infrastructure) and personnel is excluded, as these processes are non-
attributable and they contribute less than 10% to GWP‑GHG.
The contribution of the back ground processes have been included.
No flows were excluded on the basis of cut-off criteria.
ALLOCATION, ESTIMATES AND ASSUMPTIONS
Allocation is required if some material, energy, and waste data cannot be
measured separately for the product under investigation.
In this study, as per EN 15804, allocation is conducted in the following
order;
1. Allocation should be avoided.
2. Allocation should be based on physical properties (e.g. mass, volume)
when the difference in revenue is small.
3. Allocation should be based on economic values.
The key processes that require allocation are:
- Production of concrete mixes: All shared processes are attributed
to concrete products based on their volume.
- With regards to inputs, it was assumed that silica fume is a waste
product and therefore burden-free.
- Ground granulated blast furnace slag from steel blast furnace
production was allocated economically.
- Electricity and diesel use at the plant are allocated to concrete on
Volume (1m3) basis.
Electricity
Electricity has been modelled for processes that Piave Premix controls
using adjusted data to represent the estimated residual electricity grid mix
in Victoria. This is done by removing renewables from the Australian
Energy Statistics 2022 data (Table O3.2). The residual grid mix is made up
of Coal (92.1%), natural gas (7.3%) and oil products (0.6%).
The reference year for the electricity dataset documented is 2022.
The allocations in the Ecoinvent 3.10 datasets used in this study follow the
Ecoinvent system model ‘Allocation, cut-off, EN15804’.

-- 9 of 16 --

10
Premix Concrete – S32MPa GreenCrete 70
AVERAGES AND VARIABILITY
The results of the LCA are based on data from a single plant based in port
Melbourne Victoria. There are no other plants that the environmental
profiles of the concrete in this report relate to. Therefore the mandatory
indicators stay well within the ±10% range as required by the PCR as they
only relate to this one plant.

-- 10 of 16 --

11
Premix Concrete – S32MPa GreenCrete 70
ENVIRONMENTAL IMPACT DATA
Please consider the following mandatory statements when interpreting the results:
The estimated impact results are only relative statements, which do not indicate the endpoints of the impact categories, exceeding threshold values, safety margins
and/or risks. EN 15804 reference package based on EF 3.1 version has been used.
The use of the results of modules A1-A3 (A1-A5 for services) without considering the results of module C is discouraged.
Note: The results of the impact categories abiotic depletion of minerals and metals, land use, human toxicity (cancer), human toxicity, non-cancer and ecotoxicity
(freshwater) may be highly uncertain in LCAs that include capital goods/infrastructure in generic datasets, in case infrastructure/capital goods contribute greatly to
the total results. This is because the LCI data of infrastructure/capital goods used to quantify these indicators in currently available generic datasets sometimes lack
temporal, technological and geographical representativeness. Caution should be exercised when using the results of these indicators for decision-making purposes.
CORE ENVIRONMENTAL IMPACT INDICATORS – EN 15804+A2, PEF
Impact category Unit A1-A3 C1 C2 C3 C4 D
GWP – total1) kg CO2 eq 1.34E+02 5.67E+00 2.16E+01 1.25E+01 2.29E+00 ‐1.61E+00
GWP – fossil kg CO2 eq 1.34E+02 5.67E+00 2.16E+01 1.25E+01 2.29E+00 ‐1.61E+00
GWP – biogenic kg CO2 eq 0.00E+00 0.00E+00 4.34E‐19 0.00E+00 0.00E+00 0.00E+00
GWP – LULUC kg CO2 eq 2.28E‐02 5.65E‐04 7.69E‐03 1.28E‐03 1.31E‐03 ‐1.72E‐04
Ozone depletion pot. kg CFC-11 eq 7.54E‐06 1.21E‐06 4.31E‐07 1.91E‐07 6.64E‐08 ‐7.58E‐16
Acidification potential mol H+eq 1.38E+00 5.89E‐02 6.78E‐02 1.12E‐01 1.62E‐02 ‐2.87E‐03
EP-freshwater2) kg P eq 8.34E‐03 1.88E‐05 1.44E‐03 3.60E‐04 1.88E‐04 ‐5.33E‐05
EP-marine kg N eq 4.42E‐01 2.61E‐02 2.29E‐02 5.22E‐02 6.19E‐03 ‐1.38E‐03
EP-terrestrial mol N eq 4.88E+00 2.86E‐01 2.49E‐01 5.71E‐01 6.76E‐02 ‐1.29E‐02
POCP (“smog”)3) kg NMVOC eq 1.31E+00 7.87E‐02 1.07E‐01 1.70E‐01 2.42E‐02 ‐3.80E‐03
ADP-minerals & metals4) kg Sb eq 3.34E‐04 2.88E‐06 6.97E‐05 4.47E‐06 3.64E‐06 ‐3.92E‐08
ADP-fossil resources MJ 1.62E+03 7.63E+01 3.05E+02 1.63E+02 5.62E+01 ‐2.15E+01
Water use5) m3 eq depr. 6.84E+02 2.05E‐01 1.50E+00 4.07E‐01 1.62E‐01 ‐2.66E+00
1) GWP = Global Warming Potential; 2) EP = Eutrophication potential. Required characterisation method and data are in kg P-eq. Multiply by 3,07 to get PO4e; 3) POCP = Photochemical ozone formation; 4) ADP = Abiotic
depletion potential; 5) EN 15804+A2 disclaimer for Abiotic depletion and Water use and optional indicators except Particulate matter and Ionizing radiation, human health. The results of these environmental impact
indicators shall be used with care as the uncertainties on these results are high or as there is limited experience with the indicator.
2) The OneClickLCA tool uses global characterisation factors for WDP and does not use the regionalised Australian catchment level data.

-- 11 of 16 --

12
Premix Concrete – S32MPa GreenCrete 70
ADDITIONAL (OPTIONAL) ENVIRONMENTAL IMPACT INDICATORS – EN 15804+A2, PEF
Impact category Unit A1-A3 C1 C2 C3 C4 D
Particulate matter Incidence 8.99E‐06 1.58E‐06 1.74E‐06 1.83E‐05 3,70E‐07 ‐1,77E‐08
Ionizing radiation6) kBq U235
eq
4.79E‐01 3.51E‐01 3.86E‐01 7.22E‐02 3,53E‐02 0,00E+00
Ecotoxicity (freshwater) CTUe 6.94E+02 4.59E+01 3.96E+01 8.97E+00 4,72E+00 ‐1,70E+01
Human toxicity, cancer CTUh 4.95E‐08 1.76E‐09 3.67E‐09 1.28E‐09 4,22E‐10 ‐2,44E‐10
Human tox. non-cancer CTUh 1.31E‐06 3.32E‐08 1.92E‐07 2.03E‐08 9,70E‐09 ‐1,05E‐08
SQP7) - 8.61E+02 9.92E+00 1.93E+02 1.14E+01 1,11E+02 ‐6,46E+02
6) EN 15804+A2 disclaimer for Ionizing radiation, human health. This impact category deals mainly with the eventual impact of low dose ionizing radiation on human health of the nuclear fuel cycle. It does not consider effects due
to possible nuclear accidents, occupational exposure nor due to radioactive waste disposal in underground facilities. Potential ionizing radiation from the soil, from radon and from some construction materials is also not measured
by this indicator; 7) SQP = Land use related impacts/soil quality.
END OF LIFE – WASTE
Impact category Unit A1-A3 C1 C2 C3 C4 D
Renew. PER as energy8) MJ 4.04E+01 4.36E‐01 5.24E+00 1.03E+00 5.43E‐01 ‐2.87E+00
Renew. PER as material MJ 0.00E+00 0.00E+00 0.00E+00 0.00E+00 0.00E+00 0.00E+00
Total use of renew. PER MJ 4.04E+01 4.36E‐01 5.24E+00 1.03E+00 5.43E‐01 ‐2.87E+00
Non-re. PER as energy MJ 1.67E+03 7.63E+01 3.05E+02 1.63E+02 5.62E+01 ‐2.15E+01
Non-re. PER as material MJ 0.00E+00 0.00E+00 0.00E+00 0.00E+00 0.00E+00 0.00E+00
Total use of non-re. PER MJ 1.67E+03 7.63E+01 3.05E+02 1.63E+02 5.62E+01 ‐2.15E+01
Secondary materials kg 2.10E+02 2.99E‐02 1.39E‐01 6.77E‐02 1.41E‐02 ‐2.03E+00
Renew. secondary fuels MJ 1.13E‐03 9.76E‐05 1.75E‐03 1.77E‐04 2.93E‐04 0.00E+00
Non-ren. secondary fuels MJ 0.00E+00 0.00E+00 0.00E+00 0.00E+00 0.00E+00 0.00E+00
Use of net fresh water m3 2.96E+00 4.63E‐03 4.14E‐02 1.08E‐02 5.85E‐02 ‐6.65E‐02
8) PER = Primary energy resources

-- 12 of 16 --

13
Premix Concrete – S32MPa GreenCrete 70
ENVIRONMENTAL INFORMATION DESCRIBING WASTE CATEGORIES
Impact category Unit A1-A3 C1 C2 C3 C4 D
Hazardous waste kg 1.23E+00 1.02E‐01 4.37E‐01 1.81E‐01 6.21E‐02 ‐3.66E‐10
Non-hazardous waste kg 2.32E+03 7.18E‐01 9.18E+00 2.47E+00 3.67E+02 ‐1.16E‐01
Radioactive waste kg 2.34E‐03 5.37E‐04 9.60E‐05 1.77E‐05 8.62E‐06 ‐1.73E‐05
END OF LIFE – OUTPUT FLOWS
Impact category Unit A1-A3 C1 C2 C3 C4 D
Components for re-use kg 0.00E+00 0.00E+00 0.00E+00 0.00E+00 0.00E+00 0.00E+00
Materials for recycling kg 2.58E‐02 0.00E+00 0.00E+00 2.03E+03 0.00E+00 0.00E+00
Materials for energy rec kg 6.66E‐06 0.00E+00 0.00E+00 0.00E+00 0.00E+00 0.00E+00
Exported energy MJ 3.15E‐02 0.00E+00 0.00E+00 0.00E+00 0.00E+00 0.00E+00
ENVIRONMENTAL IMPACTS – GWP-GHG - THE INTERNATIONAL EPD SYSTEM
Impact category Unit A1-A3 C1 C2 C3 C4 D
GWP-GHG10) kg CO2 eq 1.34E+02 5.67E+00 2.16E+01 1.25E+01 2.29E+00 ‐1.61E+00
10) This indicator includes all greenhouse gases excluding biogenic carbon dioxide uptake and emissions and biogenic carbon stored in the product as defined by IPCC AR 5 (IPCC 2013). In addition, the characterisation factors for
the flows - CH4 fossil, CH4 biogenic and Dinitrogen monoxide - were updated in line with the guidance of IES PCR 1.3.4 Annex 1. This indicator is identical to the GWP-total of EN 15804:2012+A2:2019 except that the
characterization factor for biogenic CO2 is set to zero.
CLASSIFICATION OF DISCLAIMERS TO THE DECLARATION OF CORE AND ADDITIONAL ENVIRONMENTAL IMPACT INDICATORS
ILCD Classification Indicator Disclaimer
ILCD Type 1
GWP None
ODP None
PM None
ILCD Type 2
AP None
EP-Freshwater None
EP-Marine None
EP-Terrestrial None
POCP None
IRP 1

-- 13 of 16 --

14
Premix Concrete – S32MPa GreenCrete 70
ILCD Type 3
ADP-Minerals&Metals 2
ADP-Fossil 2
WDP 2
ETP-fw 2
HTP-c 2
HTP-nc 2
SQP 2
Disclaimer 1 – This impact category deals mainly with the eventful impact of low dose ionizing radiation on human health of the nuclear
fuel cycle. It does not consider effects due to possible nuclear accidents, occupational exposure nor due to radioactive waste disposal in
underground facilities. Potential ionizing radiation from the soil, from radon and from some construction materials is also not measured by
this indicator.
Disclaimer 2 – The results of this environmental impact indicator shall be used with care as the uncertainties on these results are high or as
there is limited experience with this indicator.

-- 14 of 16 --

15
Premix Concrete – S32MPa GreenCrete 70
SCENARIO DOCUMENTATION
Manufacturing energy scenario documentation
Scenario parameter Value
Electricity data source and quality Sourced from retail bill and on
site meter readings
Electricity CO2e / kWh 1.08 kg CO2e / kWh
REFERENCES
ISO 14025:2010 Environmental labels and declarations – Type III
environmental declarations. Principles and procedures.
ISO 14040:2006 Environmental management. Life cycle assessment.
Principles and frameworks.
ISO 14044:2006 Environmental management. Life cycle assessment.
Requirements and guidelines.
ecoinvent Centre. (2023). ecoinvent Database Version 3.10. Retrieved
from https://ecoinvent.org/ecoinvent-v3-10/
One Click LCA. (n.d.). One Click LCA database. One Click LCA. Retrieved
March 6, 2025, from https://www.oneclicklca.com/
EN 15804:2012+A2:2019/AC:2021, Sustainability of construction works –
Environmental product declarations – Core rules for the product
category of construction products, European Committee for
Standardization (CEN), Brussels, August 2021.
UN CPC 375 (Articles of concrete, cement and plaster)
United Nations Statistical Commission. 2008. ‘Central Product
Classification (CPC) Version 2.1’. version 2.1. United Nations.
https://unstats.un.org/unsd/classifications/unsdclassifications.
c-PCR-003 Concrete and concrete elements (EN 16757:2022), Product
category rules for concrete and concrete elements, version 2023-01-02
EPD International (2021). General Programme Instructions of the
international EPD® system. Version 4.0. www.environdec.com.
ABS and Statistics New Zealand. 2006. ‘Australian and New Zealand
Standard Industrial Classification (ANZSIC) 2006’.
https://www.abs.gov.au/AUSSTATS/abs@.nsf/DetailsPage/1292.02006%
20(Revision%202.0)?OpenDocument.
The LCA and EPD have been created using the One Click LCA Pre-verified
EPD Generator, tool version 0.22.12, One Click LCA Ltd, approved 2024-
01-05
Piave Premix Concrete Products LCA Background Report
IEPDS. 2024. ‘PCR 2019:14 Construction Products (EN 15804+A2)
(v1.3.4)’. version 1.3.4. Sweden: The International EPD System.
https://environdec.com/pcr-library/with-documents
Standards Australia. (2007). AS 1379: Specification and manufacture of
concrete. Standards Australia.

-- 15 of 16 --

16
Premix Concrete – S32MPa GreenCrete 70
Data references:
Adbri. (2022). Environmental Product Declaration: Cement Products.
EPD Australasia. Retrieved from https://www.adbri.com.au/wp-
content/uploads/2022/11/Adbri-Cement-EPD-2022_Press.pdf
Independent Cement and Lime Pty Ltd. (2023). Environmental Product
Declaration: Ground Granulated Blast-Furnace Slag (GGBFS). EPD
Australasia. Retrieved from
https://www.environdec.com/library/epd10955
Boral. (2024). Environmental Product Declaration: Victoria Region
Quarries and Recycling Products. EPD Australasia. Retrieved from
https://epd-australasia.com/wp-content/uploads/2024/02/SP10222-
Boral-EPD_Vic-Quarries-Recycling_Feb24.pdf
European Federation of Concrete Admixtures Associations a.i.s.b.l.
(EFCA). (2021). Environmental Product Declaration – Concrete
Admixtures: Plasticizers and Superplasticizers (EPD No. EPD-EFC-
20210198-IBG1-EN). Institut Bauen und Umwelt e.V. (IBU). Retrieved
from https://dnk.sika.com/dms/getdocument.get/27b4cc84-6112-4770-
8dda-2fcb6d61ddb9/Sika_Plastiment_LA-55_en_EPD.pdf
Department of Climate Change, Energy, the Environment and Water.
(2022). National Waste Report 2022. Retrieved from
https://www.dcceew.gov.au/sites/default/files/documents/national-
waste-report-2022.pdf
Australian Government Department of Industry, Science, Energy and
Resources. (2022). Australian Energy Statistics 2022: Table O3.2 –
Electricity generation in Victoria, by fuel type, physical units, calendar
year. Australian Energy Statistics. Retrieved from
https://www.energy.gov.au/sites/default/files/2022-
04/Australian%20Energy%20Statistics%202022%20Table%20O%20-
%20Publication%20version.pdf

-- 16 of 16 --

