Hymix EPD 1
An EPD should provide current information and may be updated or depublished if conditions change. To find
the latest version of the EPD and to confirm its validity, see www.environdec.com.
EPD Registration Number:
Date of Publication:
Valid Until:
Date of Version:
Environmental Product Declaration
In Accordance with Environdec c-PCR-003 Concrete, concrete elements (EN 16757:2023), ISO 14025 and
EN15804:A2
Programme Operator: EPD International AB
Regional Programme: EPD Australasia
QUEENSLAND - GOLD COAST
Generic EPD - Gold Coast Region
HyLo-50 Normal-Class 25 MPa
v.1 2024-11-19
2029-11-19
2024-11-19
EPD-IES-0014958:001

-- 1 of 29 --

Hymix EPD 2
Hymix & Sustainability 5
Life Cycle & Processes 8
Product Environmental Performance 15
References 25
Contents
hymix.com.au | 1300 049 649

-- 2 of 29 --

Hymix EPD 3
For over 50 years, Hymix has lead the industry in innovative concrete solutions.
From domestic pool surrounds and driveways, to residential, commercial and large
infrastructure developments Hymix supports projects of all scales.
Our promise
At Hymix, we want to be the most trusted concrete supplier in Australia; earning that
trust means that we need to do a few things, really well. So these are our promises to
you and the foundation for us to build trusting and long term partnerships.
1. Prior to and during pours we’ll put the effort in to get to know you and the nuances
of your particular project. Where required, we’ll offer the benefit of our 50 plus years
of experience.
2. We’ll supply high quality concrete alongside inspiring decorative concrete products
that you and your customers can rely on to perform, now, and into the future.
3. Through continuous training, we’ll ensure that our employees can take the time to
do the job right. And that means doing it safely. And we’ll remember that time is
money, so we’ll do everything within our power to keep your projects moving. That
means being realistic with our delivery times from the outset and making sure that
you get total visibility of your orders progress, where and when you need it.
About Hymix
hymix.com.au | 1300 049 649

-- 3 of 29 --

4
Hymix
We want to be the most
trusted concrete supplier
in Australia
For over 50 years, Hymix has led the industry in
innovative concrete solutions. From domestic pool
surrounds and driveways to residential, commercial
and large infrastructure developments Hymix
supports projects of all scales.
We're passionate about creating sustainable
concrete products for a better world. Our company
is united by the belief that for an organisation to
flourish long into the future, it must focus its energy
and resources on innovation, people, environment,
and ethical governance. We are driven by long-term
benefits, not quick wins.

-- 4 of 29 --

5
Hymix & Sustainability

-- 5 of 29 --

6
Our Sustainability Charter
To realise these sustainability goals, individual
plans will be developed for our operations,
addressing their unique sustainability challenges.
We will also build sustainability targets into
everyone’s roles, recruit sustainability champions
and invest in resources and projects that
support our sustainability plans. Our plans and
commitments align directly with each of our
core values: Care, Collaboration and Ownership.
Committing to these goals as a team is an
important part of being a truly sustainable
business.
I look forward to working together to
realise better outcomes for our people,
our communities and our planet.
“Driven by excellence and high performance, together we will
shape Australia’s construction materials industry, building a
legacy for generations to come”
Phil Schacht
Chief Executive
Heidelberg Materials Australia
The Heidelberg Materials Australia group of
companies are leaders in the heavy construction
materials industry. However, we never take it for
granted. We help to build the infrastructure of
communities by working with them and being a
part of them. While we are known for our “we’ll
make it happen” attitude, we are conscious of
our socio-economic and environmental impacts.
One of our strategic goals is to drive operational
excellence and innovation, which means we are
always looking for new ways of working to help
preserve and protect our planet’s natural
resources.
Heidelberg Materials sustainability commitments
2030 serve as a guiding principle for our
sustainability strategy.
The strategy is comprised of four strategic
pillars and supports initiatives that focus on C02
Emissions, Sustainable Products, Biodiversity,
Water and Corporate Social Responsibility.

-- 6 of 29 --

7
To be the most trusted concrete supplier in Australia
goes beyond people and products – we need to
manage our business sustainably.
We believe companies that succeed in the future will be
those that continuously invest in people, innovation,
environment and ethical governance – and focus on
delivering long-term benefits, not just immediate goals.
Every day we engage with employees, local
communities and stakeholders to drive sustainable work
practices. Our Sustainability policy (right) is embedded
into our company strategy and drives action on the
ground.
Leveraging the UN Sustainable Development Goals,
our commitment to sustainability is encapsulated in the
six policy topics, outlined to the right.
In Accordance with Environdec c-PCR-003 Concrete, concrete elements (EN 16757), ISO 14025 and EN15804:A2
Sustainability Policy
hymix.com.au | 1300 049 649

-- 7 of 29 --

8
Life Cycles & Processes

-- 8 of 29 --

Hymix EPD 9
Product EPD Process
hymix.com.au | 1300 049 649
Declared Unit is 1m3 of Concrete
The process is used to produce an accurate estimation at all stages of the product life cycle from cradle to grave.
Estimation at each stage is based on actual data which is a combination of both current and prior year average
consumption per declared unit.
Life Cycle Assessment Tool
For the purposes of creating this Environmental Product Declaration (EPD), the Global Cement & Concrete
Association (GCCA) concrete EPD tool v. 5.0 (short: GCCA tool) has been employed.
EPDs are created under either of 2 streams:
▪ Generic Stream - The class of product modelled is used for a particular geographical region using averaged data
across operations.
▪ Project-specific stream – Models the manufacture of specific products required for a particular project being
delivered from specific plant(s) using weighted average data where relevant and possible. Reports created after
the completion of a project offer the highest accuracy, including all mix variations for each delivery.
The main data categories include:
▪ The average bill of materials (BOM) for the concrete mix selected in the range of concrete plants specified
including their average raw material travel distance, or the calculated BOM based on actual delivered materials
incl. travel distances (average or specific) for the producing plants.
▪ The average fuel, water and energy consumption per declared unit between those plants;
▪ Plant production waste based on a nationally calculated figure;
▪ Recarbonation of concrete is determined through pre-defined values within GCCA tool for the type of
construction project (-3.28 kg CO2 eq./ m³ at Stage B, -1.11 kg CO2 eq./ m³ at Stage C3, and -2.82 kg CO2 eq./
m³ at Stage C4), where known; and,
▪ End of life recycling is based upon industry data.
▪ This EPD Process is certified using GCCA international modelling of energy use and environmental impact to
obtain a suitable estimation for products manufactured.
▪ Pre-defined cement and clinker data provided by the GCCA tool are used only where no better (supplier/source
specific) information is available.
Assumptions & Limitations
▪ This is a generic EPD.
▪ All modelling assumptions adopted from the GCCA Tool.
▪ The geographical scope involves QUEENSLAND - GOLD COAST.
▪ Raw material (inbound) transport distances is the previous year’s travel distance average weighted according to
deliveries across operations.
▪ For generic EPDs travel for diesel truck from concrete production site to customer site was set to 20 km default.
Longer or shorter travel distances will have minor effects on the overall CO2 values. Concrete plants in the study
include: Labrador, Stapylton, and Burleigh, Truck type of >32 tonne was assumed to be fully utilized travelling to
construction site with empty returns.
▪ Travel distance for fuel from depots to operations was set to 78 km.
▪ Concrete mixes are assumed to use an equal amount of site fuel and energy and responsible for an equal
amount of waste flows.
▪ Production is assumed to be equal across all plants included in the study for the calculation of the bill of
materials.
▪ Water usage in operations is averaged over the entire state.
▪ Grid purchased electricity mixes is based on the specific state’s energy mix from OpenNEM. For this project,
energy mix was sourced from coal and peat (66%), gas (7%), solar (21%), wind (4%), hydro (2%), and biomass
(<1%). The electricity emission (GWP-GHG) is 0.85 kg CO2e/kWh.
▪ Travel for materials sources internationally included from shipping origin.
▪ Reference Service Life (RSL) is set to 50 years as per default. It's based on the lowest exposure class A1 & A2
(AS 3600:2018 "Concrete Structures") in relatively benign environments.

-- 9 of 29 --

Hymix EPD 10
The materials (by mass%) contained in Generic EPD - Gold Coast Region mixes are
summarized in the table below.
By-Products, Recycled Materials & Allocations
Co-products would be allocated via economic allocations and then normalized based on BOM.
The following materials are the product of waste streams of other industrial processes:
Fly ash
• A by-product of coal-fired power stations, fly ash is considered to carry no environmental
impact for the purposes of this EPD, hence an economic allocation of $0 has been applied to
fly ash. The only burdens are of transport to manufacturing sites.
Ground Granulated Blast Furnace Slag (GGBFS)
• Blast furnace slag is a by-product of steel production that is dried and ground
for use in concrete production. To duly allocate the environmental impacts, economic
allocation has been employed.
Silica fume
• As a by-product of silicon production, silica fume is considered to carry
no environmental burden for the purposes of this EPD.
Recycled concrete aggregate
• A component of the boarder category of construction and demolition waste, environmental
impacts are allocated on the basis of reprocessing the material following delivery to the
recycling facility.
Manufactured Sand
• A by-product of processing coarse aggregate. This manufactured sand is a direct
replacement for natural sand and prevents the need to extract natural resources.
Packaging
This concrete is not produced with any packaging, instead delivered directly to site immediately
following production.
Hazard information related to concrete placement
GHS classifications
▪ Skin Corrosion Category 1
▪ Serious Eye Damage –Category 1
▪ Skin Sensitisation Category 1
▪ Specific Target Organ Toxicity (Repeated Exposure) Category 2
Hazard Statement(s)
▪ H302 –Harmful if swallowed
▪ P280 –Wear protective gloves/clothing/eye protection.
▪ H314 –Causes severe skin burns and eye damage
▪ H317 –May cause an allergic skin reaction
▪ H318 -Causes serious eye damage
▪ H373 –May cause damage to lungs by inhalation (dust from dried product)
Bill of Materials Low Level [%] High Level [%]
Cement 4 18
Supplementary Cementitious Materials 0 12
Aggregates 61 87
Water 3 12
Admixtures 0 <1
Reinforcements 0 <1
hymix.com.au | 1300 049 649
Product Content Declaration

-- 10 of 29 --

Hymix EPD 11
Product Life Cycle Stages
hymix.com.au | 1300 049 649
All stages of the product lifecycle have been
considered for this EPD – cradle to grave.
By its nature, there are some stages of the
lifecycle that are not applicable to the
concrete product.
The scenario applied for the use stage
assumes that under normal use, no
maintenance repair or replacement of the
product during its service life
is required. As a result, the values are
displayed as zero.
Those stages that, due to practicality,
cannot
be assessed accurately draw on default
values
of the underlying GCCA tool.
For Project-specific EPDs, allocation is
determined by the supplying plants with
estimates as to the likely volume to be
delivered from each. Where existing and
sufficient data exists, historical data will be
used to make this determination.
Product Stage Construction
Stage Use Stage End of Life Stage
Benefits &
loads for
the next
product
system
Raw Material Supply
Transport
Manufacturing
Transport
Construction/installation process
Use
Maintenance incl. transport
Repair incl. transport
Replacement incl. transport	
Refurbishment incl. transport
Operational Energy Use	
Operational Water Use
De
-construction & demolition
Transport
Re
-use recycling
Final Disposal
Reuse, Recovery Recycling
Module A1 A2 A3 A4 A5 B1 B2 B3 B4 B5 B6 B7 C1 C2 C3 C4 D
Modules
declared X X X X X X X X X X X X X X X X X
Geography GLO GLO AU AU AU AU AU AU AU AU AU AU AU AU AU AU AU
Specific
data 81%
Variation
products <10%
Variation
sites <10%

-- 11 of 29 --

Hymix EPD 12
• The lifecycle model and system
boundary is the same for both Generic
and Project-specific concrete EPDs, as
detailed in the graphic.
• All stages of the lifecycle, from quarry
to recycling are covered by the EPD.
Cut-off rules
• The cut-off threshold for the LCA study
was flows contributing less than 1% for
any individual input included in the LCA.
No flows were deliberately excluded
due to this threshold, however
particularly minor impacts (e. g.
packaging of chemical admixtures) were
not considered. Cut off will occur only
when data, or reliable estimates, are
not practical to source. The
contribution of capital goods
(production equipment and
infrastructure) and personnel are non-
attributable and excluded for the
system boundary.
Product LCA & System Boundary
hymix.com.au | 1300 049 649

-- 12 of 29 --

Hymix EPD 13
Product LCA & System Boundary
LCA Stage Item Source Timing Data Quality
Product Description Product description and density ERP report Bill of Materials and material specific data Upon EPD creation High, Primary
A1-3 Materials Raw Materials ERP report BOM and Mix design compilation used in conjunction with material template
Note. Upstream process for raw materials utilise data from ecoinvent 3.5. Cement and Clinker details to be provided by cement producer or, where
not available, GCCA Tool default data used in conjunction with ecoinvent 3.5.
Upon EPD creation High, Secondary
A1-3 Materials Inbound travel (raw materials) ERP report 2. Inbound Travel drawing from actual deliveries from sources to operations.
Where delivery data not available, travel calculated based on Google Maps.
Train travel (only for operations around Melbourne) calculated by actual Google Maps distance.
Full prior year data, average per delivery
Actual travel distances between source and
operation.
High, Primary
A1-3 Materials Allocation Factor (for secondary co products): Slag: AusLCI
Fly Ash & Silica fume: no allocation as they are industrial by-products.
Upon EPD creation Secondary, Medium
A1-3 Manufacturing Plant Energy and Fuel Consumption ERP Report 3. Concrete Energy Use, drawing on actual invoiced usage. Full prior year data, average per metre Primary, High
A1-3 Manufacturing Electricity Energy Sources Sourced from OpenNEM
https://opennem.org.au; Australian Energy Market Operator. Excludes imports.
Full year prior data, state-based, percentages Secondary, High
A1-3 Waste Management Waste and waste water Waste water volume set to 9L per 1 m3 Static Secondary, Medium
A4-5 Construction Outbound Travel For generic EPDs: ERP report 5. Outbound travel drawing from actual deliveries from operations to customer sites. Where data not available, travel
calculated based on Google Maps.
For project-specific EPDs: The project-specific travel distances from the main plant to the construction site was applied.
Generic EPD: Full prior year data, average per
delivery.
Project-specific EPD: Actual travel distances
between plant and construction site.
Primary, High
B. Use Re-carbonation Default GCCA Tool settings NA Proxy, Medium
C. End of Life Demolition Demolition Default GCCA Tool settings NA Proxy, Medium
C. End of Life Transport Transport Default GCCA Tool settings NA Proxy, Medium
C. End of Life
Waste Processing
Recycling Rate at EOL Masonry materials recycling rate obtained from annual National Waste Report published (e. g. for National Waste Report 2022, page 41, figure 29)
National Waste Reports
Prior year National Waste Report if available.
If not, then latest available
Proxy, Medium
C. End of Life
Disposal
Disposal Rate at EOL Disposal rate inverse of masonry materials recycling rate obtained from annual National Waste Report published
National Waste Reports
Prior year National Waste Report if available.
If not, then latest available
Proxy, Medium
D Benefits and Loads Default GCCA Tool settings NA NA
General General EcoInvent database used by the GCCA tool
Note: This covers environmental information for all raw materials and energy sources. Cement, where data is available, employs specific raw
material and energy data for the product manufacture and for each component draws on Eco Invent Data.
NA Secondary, High
Product Description Product description and density ERP report Bill of Materials and material specific data Upon EPD creation High, Primary
A1-3 Materials Raw Materials ERP report BOM and Mix design compilation used in conjunction with material template
Note. Upstream process for raw materials utilise data from ecoinvent 3.5. Cement and Clinker details to be provided by cement producer or, where
not available, GCCA Tool default data used in conjunction with ecoinvent 3.5.
Upon EPD creation High, Secondary
A1-3 Materials Inbound travel (raw materials) ERP report 2. Inbound Travel drawing from actual deliveries from sources to operations.
Where delivery data not available, travel calculated based on Google Maps.
Train travel (only for operations around Melbourne) calculated by actual Google Maps distance.
Full prior year data, average per delivery
Actual travel distances between source and
operation.
High, Primary
A1-3 Materials Allocation Factor (for secondary co products): Slag: AusLCI
Fly Ash & Silica fume: no allocation as they are industrial by-products.
Upon EPD creation Secondary, Medium
A1-3 Manufacturing Plant Energy and Fuel Consumption ERP Report 3. Concrete Energy Use, drawing on actual invoiced usage. Full prior year data, average per metre Primary, High
A1-3 Manufacturing Electricity Energy Sources Sourced from OpenNEM
https://opennem.org.au; Australian Energy Market Operator.
Full year prior data, state-based, percentages Secondary, High
A1-3 Waste Management Waste and waste water Waste water volume set to 9L per 1 m3 Static Secondary, Medium
hymix.com.au | 1300 049 649
LCA Stage Item Source Timing Data
Source
Data Quality
Geographical Technical Time
Product
Description
Product description and
density
ERP report Bill of Materials and material specific data Upon EPD creation Primary Very good Very good Very good
A1-3 Materials Raw Materials ERP report BOM and Mix design compilation used in conjunction with material template
Note. Upstream process for raw materials utilise data from ecoinvent 3.10. Specific cement EPD data by the
cement manufacturer was used if available. Published cement EPDs were used to create concrete EPDs.
In the rare case that specific cement data was not possible, region-specific default cement and clinker values
(default values provided by the GCCA tool) would have been used. This would be reflected in “Specific data.”
Upon EPD creation Secondary Very good Good Very good
A1-3 Materials Inbound travel (raw
materials)
ERP report 2. Inbound Travel drawing from actual deliveries from sources to operations.
Where delivery data not available, travel calculated based on Google Maps.
Train travel (only for operations around Melbourne) calculated by actual Google Maps distance.
Full prior year data,
average per delivery
Actual travel distances
between source and
operation.
Primary Very good Good Very good
A1-3 Materials Allocation Factor (for
secondary co
products):
Slag: AusLCI
Fly Ash & Silica fume: no allocation as they are industrial by-products.
Upon EPD creation Secondary Very good Good Very good
A1-3
Manufacturing
Plant Energy and Fuel
Consumption
ERP Report 3. Concrete Energy Use, drawing on actual invoiced usage. Full prior year data,
average per cubic metre
Primary Very good Very good Very good
A1-3
Manufacturing
Electricity Energy
Sources
Sourced from OpenNEM
https://opennem.org.au; Australian Energy Market Operator. Excludes imports.
Full year prior data, state-
based, percentages
Secondary Very good Very good Very good
A1-3 Waste
Management
Waste and wastewater Wastewater volume set to 9L per 1 m3 Static Secondary Very good Good Very good
A4-5 Construction Outbound Travel For generic EPDs: ERP report 5. Outbound travel drawing from actual deliveries from operations to customer
sites. Where data not available, travel calculated based on Google Maps.
For project-specific EPDs: The project-specific travel distances from the main plant to the construction site was
applied.
For both scenarios, diesel truck is used to transport deliveries to customer site/s. A5 uses default GCCA Tool
settings for: 2.8 kWh electricity, 1.7 L diesel in building machine, 669 kg water, and 0.7 m3 wastewater. Note that
internal concrete losses are at ~1% (based on internal reports)
Generic EPD: Full prior year
data, average per
delivery.
Project-specific EPD:
Actual travel distances
between plant and
construction site.
Primary Very good Good Very good
B. Use Re-carbonation Default GCCA Tool settings NA Proxy Good Good Very good,

-- 13 of 29 --

Hymix EPD 14
Product LCA & System Boundary
hymix.com.au | 1300 049 649
LCA Stage Item Source Timing Data
Source
Data Quality
Geographical Technical Time
C. End of Life
Demolition
Demolition Default GCCA Tool settings (2.674 L diesel in building machine, 0.0365 mg PM2.5, 0.184 mg PM10, 0.139 mg
PM>10). PM refers to particulate matter.
NA Proxy Good Good Very good,
C. End of Life
Transport
Transport Default GCCA Tool settings NA Proxy Good Good Very good
C. End of Life
Waste Processing
Recycling Rate at EOL Masonry materials recycling rate obtained from annual National Waste Report published (e. g. for National
Waste Report 2022, page 41, figure 29). Referenced recycling rate is used in industry as closest to concrete-
specific value.
National Waste Reports
Prior year National Waste
Report if available. If not,
then latest available
Proxy Good Good Very good
C. End of Life
Disposal
Disposal Rate at EOL Disposal rate inverse of masonry materials recycling rate obtained from annual National Waste Report
published
National Waste Reports
Prior year National Waste
Report if available. If not,
then latest available
Proxy Good Good Very good
D Benefits and
Loads
Default GCCA Tool settings NA NA NA NA NA
General General Ecoinvent database used by the GCCA tool
Note: This covers environmental information for all raw materials and energy sources. Cement, where data is
available, employs specific raw material and energy data for the product manufacture and for each
component draws on Eco Invent Data.
NA Secondary Very good Good Very good

-- 14 of 29 --

Product Environmental
Performance

-- 15 of 29 --

Hymix EPD 16
Comment All information about goal and scope necessary for results interpretation are present in the latest version of the “LCA Model” report,
available in GCCA’s Industry EPD Tool.
Declared GWP-GHG results for modules A1-A3 are <10%.
The estimated impact results are only relative statements, which do not indicate the endpoints of the impact categories, exceeding
threshold values, safety margins and/or risks. Since Module C is included in the EPD, the use of Module A1-A3 results without
considering the results of Module C is discouraged.
EF3.0 based EN15804+A2 impact assessment methodology has been is used for the GWP indicators.
The removals and emissions associated with biogenic carbon content of i) the product and ii) the packaging are not significant or even
not relevant in the sector. The only limitation is the uptake of CO2 in A1-A3 (e.g. biobased insulation materials in precast elements or
bio based packaging materials) and reemission in A5 (packaging end-of-life) or C3-C4 (product end-of-life). This does not affect the
GWP-tot indicator.
The tool does not calculate the ‘Radioactive waste disposed’ indicator, it is considered not to be significant for the sector.
Core
environmental
impact
indicators
GWP-GHG (Global Warming Potential, GHG) • GWP-tot (Global Warming Potential total) • GWP-fos (Global Warming Potential fossil
fuels) • GWP-bio (Global Warming Potential biogenic) • GWP-luc (Global Warming Potential land use and land use change) • ODP
(Depletion potential of the stratospheric ozone layer) • AP (Acidification potential, Accumulated Exceedance) • EP-fw (Eutrophication
potential, freshwater) • EP-mar (Eutrophication potential, fraction of nutrients reaching marine end compartment) • EP-ter
(Eutrophication potential, Accumulated Exceedance) • POCP (Formation potential of tropospheric ozone) • ADPE (Abiotic depletion
potential for non- fossil resources) • ADPF (Abiotic depletion for fossil resources potential) • WDP (Water (user) deprivation potential,
deprivation-weighted water consumption)
Product Environmental Performance
hymix.com.au | 1300 049 649
1 The results of this environmental impact indicator shall be used with care as the uncertainties of the results are high and as there is limited experience with the indicator.

-- 16 of 29 --

Hymix EPD 17
Additional environmental impact indicators
PM (Potential incidence of disease due to PM emissions) • IRP2 (Potential Human exposure efficiency relative to U235) •
ETP1 (Potential Comparative Toxic Unit for ecosystems) • HTPC1 (Potential Comparative Toxic Unit for humans - cancer) •
HTPNC1 (Potential Comparative Toxic Unit for humans - non-cancer) • SQP1 (Potential soil quality index)
Parameters describing resource use
PERE (Use of renewable primary energy excluding renewable primary energy resources used as raw materials) • PERM
(Use of renewable primary energy resources used as raw materials) • PERT (Total use of renewable primary energy
resources) • PENRE (Use of non renewable primary energy excluding non-renewable primary energy resources used as
raw materials) • PENRM (Use of non-renewable primary energy resources used as raw materials) • PENRT (Total use of
non-renewable primary energy resources) • SM (Use of secondary materials) • RSF (Use of renewable secondary fuels) •
NRSF (Use of non-renewable secondary fuels) • NFW (Net use of fresh water)
Waste categories
HWD (Hazardous waste disposed) • NHWD (Non-hazardous waste disposed) • RWD (Radioactive waste disposed)
Output flows
CRU (Components for re-use) • MFR (Materials for recycling) • MER (Materials for energy recovery) • EE (Exported energy)
Extra indicators
CC1 (Emissions from calcination and removals from carbonation) • CWRS (Emissions from combustion of waste from
renewable sources used in production processes) • CWNRS (Emissions from combustion of waste from non-renewable
sources used in production processes) • GWP-prod (Removals and emissions associated with biogenic carbon content of
the bio-based product) • GWP-pack (Removals and emissions associated with biogenic carbon content of the bio-based
packaging)
Product Environmental Performance
hymix.com.au | 1300 049 649
1 The results of this environmental impact indicator shall be used with care as the uncertainties of the results are high and as there is limited experience with the indicator.
2 This impact category deals mainly with the eventual impact of low dose ionizing radiation on human health of the nuclear fuel cycle. It does not consider effects due to possible nuclear accidents, occupational
exposure nor due to radioactive waste disposal in underground facilities. Potential ionizing radiation from the soil, from radon and from some construction materials is also not measured by this indicator.

-- 17 of 29 --

Hymix EPD 18
Product Environmental Performance
hymix.com.au | 1300 049 649
[hymix_slide1]
Product identification 	HyLo-50 Normal-Class 25 MPa
EPD Registration Number 	EPD-IES-0014958:001
Production site(s) 	Gold Coast
Compressive strength 	25
Density 	2315 kg/m³
Reference service life 	50 Years
Recycling Rate At EoL 	78%
Declared unit 	1 m3
Scope 	A1-A3 + A4-A5 + B1-B7 + C1-C4 + D, cradle-to-grave
Methodology 	GCCA’s Industry EPD Tool for Cement and Concrete (V5.0), International version
Reference Year 	2023

-- 18 of 29 --

Hymix EPD 19
Product Environmental Performance
hymix.com.au | 1300 049 649
[hymix_slide2]
EPD Registration Number 	EPD-IES-0014958:001
Core environmental impact indicators 	C1-C4Recarbonation at waste processing	C1-C4Recarbonation at disposal
A1-A3 A4 A5 B1 B2 B3 B4 B5 B6 B7 C1 C2 C3 C4 D
GWP-GHG kg CO₂ eq. 	1.41E+02 4.95E+00 1.07E+01 -3.28E+00 0.00E+00 0.00E+00 0.00E+00 0.00E+00 0.00E+00 0.00E+00 9.64E+00 1.01E+01 4.44E+00 3.19E+00 -1.31E+01
GWP-tot kg CO₂ eq. 	1.41E+02 4.95E+00 1.07E+01 -3.28E+00 0.00E+00 0.00E+00 0.00E+00 0.00E+00 0.00E+00 0.00E+00 9.64E+00 1.01E+01 4.44E+00 3.19E+00 -1.31E+01
GWP-fos kg CO₂ eq. 	1.41E+02 4.95E+00 1.07E+01 -3.28E+00 0.00E+00 0.00E+00 0.00E+00 0.00E+00 0.00E+00 0.00E+00 9.63E+00 1.00E+01 4.42E+00 3.19E+00 -1.30E+01
GWP-bio kg CO₂ eq. 	2.70E-02 8.93E-04 6.78E-03 0.00E+00 0.00E+00 0.00E+00 0.00E+00 0.00E+00 0.00E+00 0.00E+00 8.57E-04 2.15E-03 3.49E-03 8.61E-04 -1.60E-02
GWP-luc kg CO₂ eq. 	2.17E-02 2.01E-03 2.59E-03 0.00E+00 0.00E+00 0.00E+00 0.00E+00 0.00E+00 0.00E+00 0.00E+00 8.36E-04 4.83E-03 6.79E-03 1.64E-03 -1.03E-02
ODP kg CFC 11 eq. 	1.63E-06 7.72E-08 2.14E-07 0.00E+00 0.00E+00 0.00E+00 0.00E+00 0.00E+00 0.00E+00 0.00E+00 1.47E-07 1.46E-07 4.22E-08 9.21E-08 -1.06E-07
AP mol H+ eq. 	6.12E-01 2.06E-02 8.65E-02 0.00E+00 0.00E+00 0.00E+00 0.00E+00 0.00E+00 0.00E+00 0.00E+00 8.69E-02 5.23E-02 3.05E-02 2.26E-02 -8.23E-02
EP-fw kg P eq. 	2.25E-02 1.27E-04 6.69E-04 0.00E+00 0.00E+00 0.00E+00 0.00E+00 0.00E+00 0.00E+00 0.00E+00 9.17E-05 3.37E-04 7.49E-04 8.63E-05 -1.18E-03
EP-mar kg N eq. 	5.25E-02 7.51E-03 3.03E-02 0.00E+00 0.00E+00 0.00E+00 0.00E+00 0.00E+00 0.00E+00 0.00E+00 4.03E-02 1.96E-02 7.07E-03 8.60E-03 -1.95E-02
EP-ter mol N eq. 	1.42E+00 8.18E-02 3.32E-01 0.00E+00 0.00E+00 0.00E+00 0.00E+00 0.00E+00 0.00E+00 0.00E+00 4.41E-01 2.13E-01 7.34E-02 9.40E-02 -2.47E-01
POCP kg NMVOC eq. 	3.94E-01 2.99E-02 9.92E-02 0.00E+00 0.00E+00 0.00E+00 0.00E+00 0.00E+00 0.00E+00 0.00E+00 1.32E-01 7.14E-02 2.20E-02 3.37E-02 -6.70E-02
ADPE kg Sb eq. 	1.63E-04 1.39E-05 1.95E-05 0.00E+00 0.00E+00 0.00E+00 0.00E+00 0.00E+00 0.00E+00 0.00E+00 3.53E-06 2.75E-05 2.90E-05 5.08E-06 -6.91E-05
ADPF MJ, net calorific value 9.82E+02 7.23E+01 1.28E+02 0.00E+00 0.00E+00 0.00E+00 0.00E+00 0.00E+00 0.00E+00 0.00E+00 1.26E+02 1.42E+02 7.14E+01 7.81E+01 -1.56E+02
WDP m³ world eq. deprived 2.62E+01 3.47E-01 9.66E-01 0.00E+00 0.00E+00 0.00E+00 0.00E+00 0.00E+00 0.00E+00 0.00E+00 3.09E-01 8.27E-01 1.14E+00 2.19E-01 -2.62E+01
Parameters describing resource use
A1-A3 A4 A5 B1 B2 B3 B4 B5 B6 B7 C1 C2 C3 C4 D
PERE MJ, net calorific value 2.66E+01 1.92E+00 5.30E+00 0.00E+00 0.00E+00 0.00E+00 0.00E+00 0.00E+00 0.00E+00 0.00E+00 7.59E-01 4.83E+00 8.19E+00 2.02E+00 -1.30E+01
PERM MJ, net calorific value 0.00E+00 0.00E+00 0.00E+00 0.00E+00 0.00E+00 0.00E+00 0.00E+00 0.00E+00 0.00E+00 0.00E+00 0.00E+00 0.00E+00 0.00E+00 0.00E+00 0.00E+00
PERT MJ, net calorific value 2.66E+01 1.92E+00 5.30E+00 0.00E+00 0.00E+00 0.00E+00 0.00E+00 0.00E+00 0.00E+00 0.00E+00 7.59E-01 4.83E+00 8.19E+00 2.02E+00 -1.30E+01
PENRE MJ, net calorific value 4.69E+02 7.23E+01 1.23E+02 0.00E+00 0.00E+00 0.00E+00 0.00E+00 0.00E+00 0.00E+00 0.00E+00 1.26E+02 1.42E+02 7.14E+01 7.81E+01 -1.56E+02
PENRM MJ, net calorific value 0.00E+00 0.00E+00 0.00E+00 0.00E+00 0.00E+00 0.00E+00 0.00E+00 0.00E+00 0.00E+00 0.00E+00 0.00E+00 0.00E+00 0.00E+00 0.00E+00 0.00E+00
PENRT MJ, net calorific value 4.69E+02 7.23E+01 1.23E+02 0.00E+00 0.00E+00 0.00E+00 0.00E+00 0.00E+00 0.00E+00 0.00E+00 1.26E+02 1.42E+02 7.14E+01 7.81E+01 -1.56E+02
SM kg 	1.68E+02 0.00E+00 1.68E+00 0.00E+00 0.00E+00 0.00E+00 0.00E+00 0.00E+00 0.00E+00 0.00E+00 0.00E+00 0.00E+00 0.00E+00 0.00E+00 0.00E+00
RSF MJ, net calorific value 2.37E+00 0.00E+00 2.37E-02 0.00E+00 0.00E+00 0.00E+00 0.00E+00 0.00E+00 0.00E+00 0.00E+00 0.00E+00 0.00E+00 0.00E+00 0.00E+00 0.00E+00
NRSF MJ, net calorific value 3.94E+01 0.00E+00 3.94E-01 0.00E+00 0.00E+00 0.00E+00 0.00E+00 0.00E+00 0.00E+00 0.00E+00 0.00E+00 0.00E+00 0.00E+00 0.00E+00 0.00E+00
NFW m³ 	1.78E+00 1.46E-02 1.14E-01 0.00E+00 0.00E+00 0.00E+00 0.00E+00 0.00E+00 0.00E+00 0.00E+00 1.99E-02 3.53E-02 4.26E-02 8.76E-02 -6.41E-01

-- 19 of 29 --

Hymix EPD 20
Product Environmental Performance
hymix.com.au | 1300 049 649
[hymix_slide3]
EPD Registration Number 	EPD-IES-0014958:001
Additional environmental impact indicators
A1-A3 A4 A5 B1 B2 B3 B4 B5 B6 B7 C1 C2 C3 C4 D
PM 	Disease incidence 	5.56E-06 5.07E-07 1.71E-06 0.00E+00 0.00E+00 0.00E+00 0.00E+00 0.00E+00 0.00E+00 0.00E+00 2.47E-06 1.10E-06 3.54E-07 5.13E-07 -1.34E-06
IRP 	kBq U235 eq. 	4.50E+02 6.38E-02 4.69E+00 0.00E+00 0.00E+00 0.00E+00 0.00E+00 0.00E+00 0.00E+00 0.00E+00 5.65E-02 1.82E-01 6.81E-01 4.98E-02 -1.12E+00
ETP 	CTUe 	1.19E+03 1.74E+01 1.77E+02 0.00E+00 0.00E+00 0.00E+00 0.00E+00 0.00E+00 0.00E+00 0.00E+00 1.79E+01 4.09E+01 1.76E+01 1.07E+01 -8.35E+01
HTPC CTUh 	3.00E-06 2.48E-08 6.95E-08 0.00E+00 0.00E+00 0.00E+00 0.00E+00 0.00E+00 0.00E+00 0.00E+00 3.77E-08 6.45E-08 1.37E-08 1.44E-08 -1.54E-07
HTPNC CTUh 	6.15E-06 4.78E-08 1.17E-07 0.00E+00 0.00E+00 0.00E+00 0.00E+00 0.00E+00 0.00E+00 0.00E+00 1.72E-08 9.09E-08 4.98E-08 1.41E-08 -1.05E-07
SQP dimensionless 	7.66E+02 7.28E+01 2.99E+01 0.00E+00 0.00E+00 0.00E+00 0.00E+00 0.00E+00 0.00E+00 0.00E+00 8.86E+00 1.32E+02 3.89E+01 1.54E+02 -1.66E+02
Other environmental information describing waste categories
A1-A3 A4 A5 B1 B2 B3 B4 B5 B6 B7 C1 C2 C3 C4 D
HWD kg 	0.00E+00 0.00E+00 0.00E+00 0.00E+00 0.00E+00 0.00E+00 0.00E+00 0.00E+00 0.00E+00 0.00E+00 0.00E+00 0.00E+00 0.00E+00 0.00E+00 0.00E+00
NHWD kg 	5.03E-02 0.00E+00 5.08E+00 0.00E+00 0.00E+00 0.00E+00 0.00E+00 0.00E+00 0.00E+00 0.00E+00 0.00E+00 0.00E+00 0.00E+00 5.08E+02 0.00E+00
RWD kg 	3.21E-04 1.56E-05 4.77E-05 0.00E+00 0.00E+00 0.00E+00 0.00E+00 0.00E+00 0.00E+00 0.00E+00 1.38E-05 4.49E-05 1.66E-04 1.22E-05 -2.73E-04
Environmental information describing output flows
A1-A3 A4 A5 B1 B2 B3 B4 B5 B6 B7 C1 C2 C3 C4 D
CRU kg 	0.00E+00 0.00E+00 0.00E+00 0.00E+00 0.00E+00 0.00E+00 0.00E+00 0.00E+00 0.00E+00 0.00E+00 0.00E+00 0.00E+00 0.00E+00 0.00E+00 0.00E+00
MFR kg 	0.00E+00 0.00E+00 1.81E+01 0.00E+00 0.00E+00 0.00E+00 0.00E+00 0.00E+00 0.00E+00 0.00E+00 0.00E+00 0.00E+00 1.81E+03 0.00E+00 0.00E+00
MER kg 	0.00E+00 0.00E+00 0.00E+00 0.00E+00 0.00E+00 0.00E+00 0.00E+00 0.00E+00 0.00E+00 0.00E+00 0.00E+00 0.00E+00 0.00E+00 0.00E+00 0.00E+00
EE 	kg 	0.00E+00 0.00E+00 0.00E+00 0.00E+00 0.00E+00 0.00E+00 0.00E+00 0.00E+00 0.00E+00 0.00E+00 0.00E+00 0.00E+00 0.00E+00 0.00E+00 0.00E+00
Extra indicators
A1-A3 A4 A5 B1 B2 B3 B4 B5 B6 B7 C1 C2 C3 C4 D
CC 	kg CO₂ eq. 	5.71E+01 0.00E+00 4.99E-01 -3.28E+00 0.00E+00 0.00E+00 0.00E+00 0.00E+00 0.00E+00 0.00E+00 0.00E+00 0.00E+00 -1.11E+00 0.00E+00 0.00E+00
CWRS kg CO₂ eq. 	2.96E-03 0.00E+00 2.96E-05 0.00E+00 0.00E+00 0.00E+00 0.00E+00 0.00E+00 0.00E+00 0.00E+00 0.00E+00 0.00E+00 0.00E+00 0.00E+00 0.00E+00
CWNRS kg CO₂ eq. 	3.34E+00 0.00E+00 3.34E-02 0.00E+00 0.00E+00 0.00E+00 0.00E+00 0.00E+00 0.00E+00 0.00E+00 0.00E+00 0.00E+00 0.00E+00 0.00E+00 0.00E+00
GWP-prod kg CO₂ 	0.00E+00 0.00E+00 0.00E+00 0.00E+00 0.00E+00 0.00E+00 0.00E+00 0.00E+00 0.00E+00 0.00E+00 0.00E+00 0.00E+00 0.00E+00 0.00E+00 0.00E+00
GWP-pack kg CO₂ 	0.00E+00 0.00E+00 0.00E+00 0.00E+00 0.00E+00 0.00E+00 0.00E+00 0.00E+00 0.00E+00 0.00E+00 0.00E+00 0.00E+00 0.00E+00 0.00E+00 0.00E+00

-- 20 of 29 --

Hymix EPD 21
Product Environmental Performance
• The EPD values presented are indicative of local material performance at the time of publishing and are subject to
change based on material availability and seasonal factors.
hymix.com.au | 1300 049 649
1More detailed information is provided in the mix-specific tables and assumptions covered in Life Cycles & Processes section
A1-A3 GWP-tot1
[kg CO2 eq./m3]
Full Lifecycle GWP-tot1
[kg CO2 eq./m3]Product Identification EPD Registration
Number
Compressive strength
[MPa]
A1-A3 GWP-tot1
[kg CO2 eq./m3]
Full Lifecycle GWP-tot1
[kg CO2 eq./m3] Application
25 MPa with 4.6 kg/m3 Blended Polyfibre 	EPD-IES-0014957:001 	25 	211 	247 	Footpath
32 MPa with 4.6 kg/m3 Blended Polyfibre 	EPD-IES-0014960:001 	32 	241 	276 	Footpath
Burnish 40 MPa 	EPD-IES-0014950:001 	40 	296 	321 	Burnish
Blockfill 20 MPa 	EPD-IES-0014951:001 	20 	145 	171 	Blockfill
Blockfill 25 MPa 	EPD-IES-0014952:001 	25 	159 	184 	Blockfill
Blockfill 32 MPa 	EPD-IES-0014953:001 	32 	180 	205 	Blockfill
Blockfill 40 MPa 	EPD-IES-0014954:001 	40 	213 	240 	Blockfill
High Workability 40 MPa 	EPD-IES-0014982:001 	40 	260 	286 	Column & Wall
High Workability 50 MPa 	EPD-IES-0014983:001 	50 	281 	307 	Column & Wall
High Workability 65 MPa 	EPD-IES-0014984:001 	65 	330 	354 	Column & Wall
High Workability 70 MPa 	EPD-IES-0014985:001 	70 	347 	371 	Column & Wall
High Workability 80 MPa 	EPD-IES-0014986:001 	80 	391 	415 	Column & Wall
High Workability 90 MPa 	EPD-IES-0014987:001 	90 	413 	436 	Column & Wall
High Workability 100 MPa 	EPD-IES-0014981:001 	100 	408 	431 	Column & Wall
HyColour 25 MPa 	EPD-IES-0014971:001 	25 	177 	202 	Decorative
HyColour 32 MPa 	EPD-IES-0014972:001 	32 	208 	232 	Decorative
HyColour 40 MPa 	EPD-IES-0014973:001 	40 	251 	277 	Decorative
HyGrade 20 MPa 	EPD-IES-0015002:001 	20 	168 	193 	Slab
HyGrade 25 MPa 	EPD-IES-0015003:001 	25 	185 	209 	Slab
HyGrade 32 MPa 	EPD-IES-0015004:001 	32 	214 	238 	Slab

-- 21 of 29 --

Hymix EPD 22
Product Environmental Performance
• The EPD values presented are indicative of local material performance at the time of publishing and are subject to
change based on material availability and seasonal factors.
hymix.com.au | 1300 049 649
1More detailed information is provided in the mix-specific tables and assumptions covered in Life Cycles & Processes section
A1-A3 GWP-tot1
[kg CO2 eq./m3]
Full Lifecycle GWP-tot1
[kg CO2 eq./m3]Product Identification EPD Registration
Number
Compressive strength
[MPa]
A1-A3 GWP-tot1
[kg CO2 eq./m3]
Full Lifecycle GWP-tot1
[kg CO2 eq./m3] Application
HyGrade 40 MPa 	EPD-IES-0015005:001 	40 	258 	284 	Slab
HyGrade 50 MPa 	EPD-IES-0015006:001 	50 	320 	344 	Slab
HyLite 25 MPa 	EPD-IES-0014974:001 	25 	196 	220 	Decorative
HyLite 32 MPa 	EPD-IES-0014975:001 	32 	214 	238 	Decorative
HyShine 32 MPa 	EPD-IES-0014976:001 	32 	220 	244 	Decorative
HyShine 40 MPa 	EPD-IES-0014977:001 	40 	261 	286 	Decorative
HySpray 25 MPa 	EPD-IES-0015007:001 	25 	254 	277 	Shotcrete
HySpray 32 MPa 	EPD-IES-0015008:001 	32 	260 	282 	Shotcrete
HySpray 40 MPa 	EPD-IES-0015009:001 	40 	303 	327 	Shotcrete
HyLo-40 Normal-Class 20MPa 	EPD-IES-0014955:001 	20 	160 	185 	General
HyLo-40 Normal-Class 25MPa 	EPD-IES-0014959:001 	25 	183 	207 	General
HyLo-40 Normal-Class 32MPa 	EPD-IES-0014961:001 	32 	211 	235 	General
HyLo-40 Normal-Class 40MPa 	EPD-IES-0014968:001 	40 	257 	283 	General
HyLo-40 Normal-Class 50MPa 	EPD-IES-0014969:001 	50 	329 	353 	General
HyLo-50 Normal-Class 20 MPa 	EPD-IES-0014956:001 	20 	128 	155 	General
HyLo-50 Normal-Class 25 MPa 	EPD-IES-0014958:001 	25 	141 	167 	General
HyLo-50 Normal-Class 32 MPa 	EPD-IES-0014962:001 	32 	166 	192 	General
HyLo-50 Normal-Class 40 MPa 	EPD-IES-0014967:001 	40 	200 	227 	General
HyLo-50 Normal-Class 50 MPa 	EPD-IES-0014970:001 	50 	234 	260 	General
Kerb Machine-placed Minimum 280 kg/m3 Cementitious 	EPD-IES-0014978:001 	No strength grade 	157 	172 	Kerb

-- 22 of 29 --

Hymix EPD 23
Product Environmental Performance
• The EPD values presented are indicative of local material performance at the time of publishing and are subject to
change based on material availability and seasonal factors.
hymix.com.au | 1300 049 649
1More detailed information is provided in the mix-specific tables and assumptions covered in Life Cycles & Processes section
A1-A3 GWP-tot1
[kg CO2 eq./m3]
Full Lifecycle GWP-tot1
[kg CO2 eq./m3]Product Identification EPD Registration
Number
Compressive strength
[MPa]
A1-A3 GWP-tot1
[kg CO2 eq./m3]
Full Lifecycle GWP-tot1
[kg CO2 eq./m3] Application
Kerb Machine-placed Minimum 320 kg/m3 Cementitious 	EPD-IES-0014979:001 	No strength grade 	176 	188 	Kerb
Lean Mix 10:1 (Mass) 	EPD-IES-0014980:001 	No strength grade 	122 	141 	Lean Mix
Piling 32 MPa HyLo-50 	EPD-IES-0014988:001 	32 	176 	202 	Piling
Piling 40 MPa HyLo-50 	EPD-IES-0014989:001 	40 	210 	236 	Piling
Piling 50 MPa HyLo-50 	EPD-IES-0014990:001 	50 	258 	283 	Piling
Post-tensioned 40 MPa (22 MPa @ 3 days) 	EPD-IES-0014963:001 	40 	268 	294 	Post-Tensioned Slab
Post-tensioned 40 MPa (22 MPa @ 4 days) 	EPD-IES-0014964:001 	40 	258 	283 	Post-Tensioned Slab
Post-tensioned 40 MPa (25 MPa @ 3 days) 	EPD-IES-0014966:001 	40 	298 	322 	Post-Tensioned Slab
Post-tensioned 40 MPa (25 MPa @ 4 days) 	EPD-IES-0014965:001 	40 	275 	300 	Post-Tensioned Slab
Stabilised Sand 12:1 (Volume) 	EPD-IES-0015010:001 	No strength grade 	120 	136 	Stabilised Sand
TMR MRTS14 Barrier Wall - 32 MPa with 0.9 kg/m3 Polyfibre EPD-IES-0014993:001 	32 	244 	269 	TMR Barrier Kerb
TMR MRTS70 Cast-in-place piles - 32 MPa (Exp B1) 	EPD-IES-0014994:001 	32 	204 	228 	TMR Piling
TMR MRTS70 Cast-in-place piles - 40 MPa (Exp B2) 	EPD-IES-0014997:001 	40 	224 	251 	TMR Piling
TMR MRTS70 Cast-in-place piles - 50 MPa (Exp B2) 	EPD-IES-0014998:001 	50 	254 	280 	TMR Piling
TMR MRTS70 Cast-in-place piles - 55 MPa (Exp B2) 	EPD-IES-0015001:001 	55 	287 	313 	TMR Piling
TMR MRTS70 Insitu - 32 MPa (Exp B1) 	EPD-IES-0014992:001 	32 	199 	224 	TMR Structural
TMR MRTS70 Insitu - 40 MPa (Exp B2) 	EPD-IES-0014996:001 	40 	222 	248 	TMR Structural
TMR MRTS70 Insitu - 50 MPa (Exp B2) 	EPD-IES-0014999:001 	50 	249 	275 	TMR Structural
TMR MRTS70 Insitu - 55 MPa (Exp B2) 	EPD-IES-0015000:001 	55 	280 	306 	TMR Structural
TMR MRTS70 No Fines Concrete 	EPD-IES-0015011:001 	No strength grade 	141 	153 	TMR No-Fines

-- 23 of 29 --

Hymix EPD 24
Product Environmental Performance
• The EPD values presented are indicative of local material performance at the time of publishing and are subject to
change based on material availability and seasonal factors.
hymix.com.au | 1300 049 649
1More detailed information is provided in the mix-specific tables and assumptions covered in Life Cycles & Processes section
A1-A3 GWP-tot1
[kg CO2 eq./m3]
Full Lifecycle GWP-tot1
[kg CO2 eq./m3]Product Identification EPD Registration
Number
Compressive strength
[MPa]
A1-A3 GWP-tot1
[kg CO2 eq./m3]
Full Lifecycle GWP-tot1
[kg CO2 eq./m3] Application
TMR MRTS70 Shotcrete - 32 MPa (Exp B1) 	EPD-IES-0014991:001 	32 	287 	308 	TMR Shotcrete
TMR MRTS70 Shotcrete - 40 MPa (Exp B2) 	EPD-IES-0014995:001 	40 	326 	350 	TMR Shotcrete

-- 24 of 29 --

References

-- 25 of 29 --

Hymix EPD 26
EPD OWNER
Hymix Australia Pty Ltd
L10, 35 Clarence St, Sydney NSW 2000
Phone: 1300 136 464
Online: hymix.com.au
PROGRAM OPERATOR
EPD International AB Box 210 60 SE-100 31 Stockholm Sweden
Online: www.environdec.com
Email: info@environdec.com
REGIONAL PROGRAMME
EPD Australasia, 315a Hardy St, Nelson 7010 New Zealand
Online: epd-australasia.com
Email: info@epd-Australasia.com
PROCESS EPD CERTIFIED BY
Megan Blizzard
Epsten Group, Inc.
101 Marietta St. NW, Suite 2600, Atlanta, Georgia 30303, USA
www.epstengroup.com
Accredited by: A2LA, Certificate #3142.03
PRODUCT CATEGORY RULES CEN standard EN 15804:A2 (PCR 2019:14 Construction Products, Version 1.3.4) served as the core PCR.
Environdec c-PCR-003 Concrete, concrete elements (EN 16757:2023) served as sub-PCR.
EN 15804 PCR REVIEW The Technical Committee of the International EPD®System. Chair: Claudia A. Peña.
The review panel may be contacted via info@environdec.com.
EPD REGISTRATION NUMBER EPD-IES-0014958:001
INDEPENDENT VERIFICATION OF THE
DECLARATION AND DATA, ACCCORDING
TO ISO 14025:
❑EPD process certification
❑EPD verification
VALID FROM 2024-11-19
VALID TO 2029-11-19
VERSION v.1 2024-11-19
DESCRIPTION OF VERSION DIFFERENCES (IF NOT
VERSION 1.0) N/A
GEOGRAPHICAL SCOPE QUEENSLAND - GOLD COAST
IMPORTANT NOTES
EPDs within the same product category but from different programmes may not be comparable. EPDs of construction products may not be comparable if they do not
comply with EN 15804.
The EPD Owner maintains full ownership, liability and responsibility for the EPD.
PRODUCT GROUP CLASSIFICATION UN CPC 88 - Concrete, cement and plaster article manufacturing services
ANZSIC CLASSIFICATION 2033 Ready Mix Concrete Manufacturing
Programme Information
hymix.com.au | 1300 049 649
x

-- 26 of 29 --

Hymix EPD 27
1) Australian Life Cycle Assessment Society. (2015). Australian Life Cycle Inventory Database Initiative. Retrieved from http://www.auslci.com.au
2) National Waste Report. (2022). https://www.dcceew.gov.au/environment/protection/waste/publications/national-waste-reports. Canberra: Department of
Climate Change, Energy, the Environment and Water.
3) Ecoinvent. (2023, Nov 23). ecoinvent 3.10 (database). Retrieved from https://ecoinvent.org/ecoinvent-v3-10/
4) EPD International. (2024). General Programme Instructions for the International EPD® System v5.0. Retrieved from envirodec.com
5) EPD Australasia Regional Annex (2024) – Version 4.2 Retrieved from epd-australasia.com
6) European Committee for Standardisation (CEN). (2022). EN 16757:2022: Sustainability of construction works - Environmental product declarations -
Product Category Rules for concrete and concrete elements.
7) European Committee for Standardisation (CEN). (2017, February). EN 16908:2017: Cement and building lime - Environmental Product Declarations -
Product Category Rules complementary to EN 15804. Brussels.
8) European Committee for Standardisation (CEN). (2019). EN 15804:2012+A2:2019: Sustainability of construction works - Environmental product
declarations - Core rules for the product category of construction products. Brussels.
9) Google. (n.d.). Google Maps. Retrieved from https://www.google.com.au/maps/
10) International Organization for Standardization. (2015). ISO14020 Environmental Labels and Declarations - General Principles.
11) International Organization for Standardization. (2017). ISO14025 Environmental Labels and Declarations - Type III Environmental Declarations -
Principles and Procedures.
12) International Organization for Standardization. (2020). ISO 14044 Environmental Management - Life Cycle Assessment - Requirements and
Guidelines.
13) McConnell, D., Holmes a Court, S., Tan, S., & Cubrilovic, N. (2022). OpenNEM. https://opennem.org.au/
14) Quantis. (2024). GCCA's Industry EPD Tool for Cement and Concrete. Retrieved from https://concrete-epd-tool.org/
15) Green Star Mat–4 Concrete Credit User Guide (2012). Retrieved from Mat-4 (gbca.org.au)
References
hymix.com.au | 1300 049 649

-- 27 of 29 --

4 Bailey Crescent
Southport QLD 4215
t: 1300 049 649
hymix.com.au
Thank you

-- 28 of 29 --

Hymix EPD 29
Appendix CO2 Service Offer
Pre-
Project
Running
Project
Post
Project
CO2 is set to become a crucial budgeting currency in the construction sector.
As such, it must be managed accordingly. Most provided embodied carbon
emission data out there is based on estimates and typically handed over to
the customer before a project starts.
At Heidelberg Materials Australia, we believe there’s a better way to
communicate carbon values, which also eliminates the current gap of carbon
monitoring options during
the construction phase in the market:
1) Pre-project: Predicting - We can provide you indicative CO2 values for your
specific project with our 3rd party verified CO2 calculator (targeted & fast
& reliable).
2) Running project: Monitoring - You get regular updates of your deliveries
and how you track towards your carbon targets (no more surprises).
3) Post-project: Verification - You’ll receive a final report and a project-specific
EPD based on actual deliveries (highest accuracy).

-- 29 of 29 --

