Environmental Product Declaration
In Accordance with Environdec c-PCR-003 ABC, ABC elements (EN 16757), ISO 14025 and EN15804:A2
Programme Operator: EPD International AB
Regional Programme: EPD Australasia
An EPD should provide current information and may be updated if conditions change. The stated validity is therefore
subject to the continued registration and publication at www.environdec.com.
EPD Registration Number:
Date of Publication:
Valid Until:
Date of Version: 1.0 2024-08-26
2029-08-26
2024-08-26
EPD-IES-0014769:001
Queensland - Brisbane
Hutchinson Builders - Aliro Warehouse
P252080

-- 1 of 28 --

Hanson & Sustainability 3
Life Cycle & Processes 9
Product Environmental Performance 15
References 23

-- 2 of 28 --

Hanson & Sustainability

-- 3 of 28 --

Global Expertise
Local Experience
Using world-class technologies and service platforms, we supply a
comprehensive range of high-quality concrete, aggregates and sand
products. We also produce road base, asphalt, and sustainable and
recycled materials.
We are backed by Heidelberg Materials - one of the world’s largest
building materials companies focused on developing materials to build
our future.
At the centre of our actions lies our responsibility for the environment.
Our Mission:
Leading change with our customers to build a sustainable future.
Silde 4

-- 4 of 28 --

Our 5 Sustainability Pillars
Silde 5

-- 5 of 28 --

Introducing the enrich - 30 / 40 / 50 Range
Slide 6 hanson.com.au | 1300 136 464
Our enrich-30/40/50 range has all the properties you expect of standard concrete,
with a guaranteed minimum of 30%, 40% or 50% carbon reduction.
And we can provide reporting based on the actual deliveries of the project.
Reporting options include:
• Pre-Project (simulated)
• During Project
• Post-Project
• EPD (project-specific)

-- 6 of 28 --

Introducing ECOTERA®
Slide 7 hanson.com.au | 1300 136 464
The Challenge with Low Carbon Concrete
The Solution
▪ A concrete that has:
• High Performance
• Low Carbon – 30% to 50% reduction
▪ Historically substituting materials in concrete mix design to lower the carbon content effects performance
• Slow early strength development
• Effect on Workability and Setting Time

-- 7 of 28 --

ECOTERA® - High Performance Low Carbon Concrete
Slide 8
A unique and innovative product:
▪ Low Carbon Concrete 30% to 50% reduction in CO2
▪ Early age strength equivalent to standard post-tensioned concrete
▪ Lower shrinkage than standard concrete – up to 50% improvement
▪ Improved Flexural Strength up to 50% improvement
Requires no additional safety requirements compared
to standard concrete - pump, place and finish within standard WHS
requirements.
The mix can be tailored to meet your specific requirements.
hanson.com.au | 1300 136 464

-- 8 of 28 --

Life Cycle & Processes

-- 9 of 28 --

Product EPD Process
Slide 10
Declared Unit is 1m3 of Concrete
▪ The process is used to produce an accurate estimation at all stages of the product life cycle
from cradle to grave. Estimation at each stage is based on actual data which is a combination
of both current and prior year average consumption per declared unit.
Life Cycle Assessment Tool
▪ For the purposes of creating this Environmental Product Declaration (EPD), the Global Cement
& Concrete Association (GCCA) concrete EPD tool v. 4.2 (short: GCCA tool) has been
employed.
EPDs are created under either of 2 streams:
▪ Generic Stream - The class of product modelled is used for a particular geographical region
using averaged data across operations.
▪ Project-specific stream – Models the manufacture of specific products required for a particular
project being delivered from specific plant(s) using weighted average data where relevant
and possible. Reports created after the completion of a project offer the highest accuracy,
including all mix variations for each delivery.
The main data categories include:
▪ The average bill of materials (BOM) for the concrete mix selected in the range of concrete
plants specified including their average raw material travel distance, or the calculated BOM
based on actual delivered materials incl. travel distances (average or specific) for the
producing plants.
▪ The average fuel, water and energy consumption per declared unit between those plants;
▪ Plant production waste based on a nationally calculated figure;
▪ Recarbonation of concrete is determined through pre-defined values within GCCA tool for the
type of construction project, where known; and,
▪ End of life recycling is based upon industry data.
▪ This EPD Process is certified using GCCA international modelling of energy use and
environmental impact to obtain a suitable estimation for products manufactured.
▪ Pre-defined cement and clinker data provided by the GCCA tool are used only where no
better (supplier/source specific) information is available.
▪ Assumptions & Limitations
▪ This is a project-specific EPD.
▪ All modelling assumptions adopted from the GCCA Tool.
▪ Raw material (inbound) transport distances is the previous year’s travel distance average
weighted according to deliveries across operations.
▪ Concrete mixes are assumed to use an equal amount of site fuel and energy and responsible
for an equal amount of waste flows.
▪ Agreed mixes are used to calculate the BOMs. Production is assumed to be equal across all
plants included in the study.
▪ The project-specific travel distances from the main plant to the construction site were applied.
▪ Water usage in operations is averaged over the full geographic region of study.
▪ Grid purchased electricity mixes is based on the specific state’s energy mix from OpenNEM. For
this project, energy mix was sourced from coal and peat (65.8%), gas (7.3%), solar (20.7%), wind
(4.0%), hydro (2.0%), and biomass (0.2%). The electricity emission (GWP-GHG) is 0.83 kg
CO2e/kWh.
▪ Travel for materials sources internationally included from shipping origin.
▪ Reference Service Life (RSL) is set to 50 years as per default. It's based on the lowest exposure
class A1 & A2 (AS 3600:2018 "Concrete Structures") in relatively benign environments.
In Accordance with Environdec c-PCR-003 Concrete, concrete elements (EN 16757), ISO 14025 and EN15804:A2
hanson.com.au | 1300 136 464

-- 10 of 28 --

Product EPD Process
Slide 11
The materials (by mass%) contained in the project mixes are summarized in the table
above.
Hazard information related to concrete placement
▪ GHS classifications
▪ Skin Corrosion Category 1
▪ Serious Eye Damage –Category 1
▪ Skin Sensitisation Category 1
▪ Specific Target Organ Toxicity (Repeated Exposure) Category 2
▪ Hazard Statement(s)
▪ H302 –Harmful if swallowed
▪ P280 –Wear protective gloves/clothing/eye protection.
▪ H314 –Causes severe skin burns and eye damage
▪ H317 –May cause an allergic skin reaction
▪ H318 – Causes serious eye damage
▪ H373 –May cause damage to lungs by inhalation (dust from dried product)
By-Products, Recycled Materials & Allocations
The following materials are the product of waste streams of other industrial processes:
Fly ash
▪ A by-product of coal-fired power stations, fly ash is considered to carry no environmental
impact for the purposes of this EPD.
Ground Granulated Blast Furnace Slag (GGBFS)
▪ Blast furnace slag is a by-product of steel production that is dried and ground for use in
concrete production. To duly allocate the environmental impacts, economic allocation
has been employed.
Silica fume
▪ As a by-product of silicon production, silica fume is considered to carry no environmental
burden for the purposes of this EPD.
Recycled concrete aggregate
▪ A component of the boarder category of construction and demolition waste,
environmental impacts are allocated on the basis of reprocessing the material following
delivery to the recycling facility.
Manufactured Sand
▪ A by-product of processing coarse aggregate. This manufactured sand is a direct
replacement for natural sand and prevents the need to extract natural resources.
Packaging
▪ This concrete is not produced with any packaging, instead delivered directly to site
immediately following production.
Bill of Materials Low Level [%] High Level [%]
Cement 4 15
Supplementary Cementitious Materials 2 7
Aggregates 73 84
Water 6 8
Admixtures 0 <1
Reinforcements 0 <2
In Accordance with Environdec c-PCR-003 Concrete, concrete elements (EN 16757), ISO 14025 and EN15804:A2
hanson.com.au | 1300 136 464

-- 11 of 28 --

Product Lifecycle Stages
Slide 12
▪ All stages of the product lifecycle have been
considered for this EPD – cradle to grave. By its
nature, there are some stages of the lifecycle
that are not applicable to the concrete product.
▪ The scenario applied for the use stage assumes
that under normal use, no maintenance repair or
replacement of the product during its service life
is required. As a result, the values are displayed as
zero.
▪ Those stages that, due to practicality, cannot be
assessed accurately draw on default values of
the underlying GCCA tool.
▪ For Project-specific EPDs, allocation is determined
by the supplying plants with estimates as to the
likely volume to be delivered from each. Where
existing and sufficient data exists, historical data
will be used to make this determination.
hanson.com.au | 1300 136 464
Product Stage Construction
Stage Use Stage End of Life Stage
Benefits & loads
for the next
product system
Raw Material Supply
Transport
Manufacturing
Transport
Construction/installation process
Use
Maintenance incl. transport
Repair incl. transport
Replacement incl. transport	
Refurbishment incl. transport
Operational Energy Use	
Operational Water Use
De
-construction & demolition
Transport
Re
-use recycling
Final Disposal
Reuse, Recovery Recycling
A1 A2 A3 A4 A5 B1 B2 B3 B4 B5 B6 B7 C1 C2 C3 C4 D1
✓ ✓ ✓ ✓ ✓ ✓ ✓ ✓ ✓ ✓ ✓ ✓ ✓ ✓ ✓ ✓ ✓

-- 12 of 28 --

Product Lifecycle Stages
Slide 13 hanson.com.au | 1300 136 464
▪ The lifecycle model and system boundary is the
same for both Generic and Project-specific
concrete EPDs, as detailed in the graphic.
▪ All stages of the lifecycle, from quarry to
recycling are covered by the EPD.
▪ Cut-off rules
The cut-off threshold for the LCA study was flows
contributing less than 1% for any individual input
included in the LCA. No flows were deliberately
excluded due to this threshold, however
particularly minor impacts (e. g. packaging of
chemical admixtures) were not considered. Cut
off will occur only when data, or reliable
estimates, are not practical to source. The
contribution of capital goods (production
equipment and infrastructure) and personnel are
non-attributable and excluded for the system
boundary.

-- 13 of 28 --

Product Data Sources
Slide 14
LCA Stage Item Source Timing Data Quality
Product Description Product description and density ERP report Bill of Materials and material specific data Upon EPD creation High, Primary
A1-3 Materials Raw Materials ERP report BOM and Mix design compilation used in conjunction with material
template
Note. Upstream process for raw materials utilise data from ecoinvent 3.5. Cement
and Clinker details to be provided by cement producer or, where not available,
GCCA Tool default data used in conjunction with ecoinvent 3.5.
Upon EPD creation High, Secondary
A1-3 Materials Inbound travel (raw materials) ERP report 2. Inbound Travel drawing from actual deliveries from sources to
operations.
Where delivery data not available, travel calculated based on Google Maps.
Train travel (only for operations around Melbourne) calculated by actual Google
Maps distance.
Full prior year data, average per delivery
Actual travel distances between source
and operation.
High, Primary
A1-3 Materials Allocation Factor (for secondary co products): Slag: AusLCI
Fly Ash & Silica fume: no allocation as they are industrial by-products.
Upon EPD creation Secondary, Medium
A1-3 Manufacturing Plant Energy and Fuel Consumption ERP Report 3. Concrete Energy Use, drawing on actual invoiced usage. Full prior year data, average per metre Primary, High
A1-3 Manufacturing Electricity Energy Sources Sourced from OpenNEM
https://opennem.org.au; Australian Energy Market Operator. Excludes imports.
Full year prior data, state-based,
percentages
Secondary, High
A1-3 Waste Management Waste and waste water Waste water volume set to 9L per 1 m3 Static Secondary, Medium
A4-5 Construction Outbound Travel For generic EPDs: ERP report 5. Outbound travel drawing from actual deliveries from
operations to customer sites. Where data not available, travel calculated based on
Google Maps.
For project-specific EPDs: The project-specific travel distances from the main plant
to the construction site was applied.
Generic EPD: Full prior year data, average
per delivery.
Project-specific EPD: Actual travel
distances between plant and
construction site.
Primary, High
B. Use Re-carbonation Default GCCA Tool settings NA Proxy, Medium
C. End of Life Demolition Demolition Default GCCA Tool settings NA Proxy, Medium
C. End of Life Transport Transport Default GCCA Tool settings NA Proxy, Medium
C. End of Life
Waste Processing
Recycling Rate at EOL Masonry materials recycling rate obtained from annual National Waste Report
published (e. g. for National Waste Report 2022, page 41, figure 29)
National Waste Reports
Prior year National Waste Report if
available. If not, then latest available
Proxy, Medium
C. End of Life
Disposal
Disposal Rate at EOL Disposal rate inverse of masonry materials recycling rate obtained from annual
National Waste Report published
National Waste Reports
Prior year National Waste Report if
available. If not, then latest available
Proxy, Medium
D Benefits and Loads Default GCCA Tool settings NA NA
General General EcoInvent database used by the GCCA tool
Note: This covers environmental information for all raw materials and energy
sources. Cement, where data is available, employs specific raw material and
energy data for the product manufacture and for each component draws on Eco
Invent Data.
NA Secondary, High
hanson.com.au | 1300 136 464

-- 14 of 28 --

Product Environmental
Performance

-- 15 of 28 --

Product Environmental Performance
Slide 16
Comment All information about goal and scope necessary for results interpretation are present in the latest version of the “LCA Model”
report, available in GCCA’s Industry EPD Tool.
The removals and emissions associated with biogenic carbon content of i) the product and ii) the packaging are not significant or
even not relevant in the sector. The only limitation is the uptake of CO2 in A1-A3 (e.g. biobased insulation materials in precast
elements or biobased packaging materials) and reemission in A5 (packaging end-of-life) or C3-C4 (product end-of-life). This does
not affect the GWP-tot indicator.
The tool does not calculate the ‘Radioactive waste disposed’ indicator, it is considered not to be significant for the sector.
Core Environmental Impact
Indicators
GWP-GHG (Global Warming Potential, GHG) • GWP-tot (Global Warming Potential total) • GWP-fos (Global Warming Potential
fossil fuels) • GWP-bio (Global Warming Potential biogenic) • GWP-luc (Global Warming Potential land use and land use change)
• ODP (Depletion potential of the stratospheric ozone layer) • AP (Acidification potential, Accumulated Exceedance) • EP-fw
(Eutrophication potential, freshwater) • EP-mar (Eutrophication potential, fraction of nutrients reaching marine end compartment)
• EP-ter (Eutrophication potential, Accumulated Exceedance) • POCP (Formation potential of tropospheric ozone) • ADPE
(Abiotic depletion potential for non- fossil resources) • ADPF (Abiotic depletion for fossil resources potential) • WDP (Water (user)
deprivation potential, deprivation-weighted water consumption)
hanson.com.au | 1300 136 464

-- 16 of 28 --

Product Environmental Performance
Slide 17
Additional Environmental Impact
Indicators
PM (Potential incidence of disease due to PM emissions) • IRP (Potential Human exposure efficiency relative to U235) • ETP
(Potential Comparative Toxic Unit for ecosystems) • HTPC (Potential Comparative Toxic Unit for humans - cancer) • HTPNC
(Potential Comparative Toxic Unit for humans - non-cancer) • SQP (Potential soil quality index)
Parameters Describing Resource Use PERE (Use of renewable primary energy excluding renewable primary energy resources used as raw materials) • PERM (Use of
renewable primary energy resources used as raw materials) • PERT (Total use of renewable primary energy resources) • PENRE
(Use of non renewable primary energy excluding non-renewable primary energy resources used as raw materials) • PENRM (Use
of non-renewable primary energy resources used as raw materials) • PENRT (Total use of non-renewable primary energy
resources) • SM (Use of secondary materials) • RSF (Use of renewable secondary fuels) • NRSF (Use of non-renewable secondary
fuels) • NFW (Net use of fresh water)
Waste Categories HWD (Hazardous waste disposed) • NHWD (Non-hazardous waste disposed) • RWD (Radioactive waste disposed)
Output Flows CRU (Components for re-use) • MFR (Materials for recycling) • MER (Materials for energy recovery) • EE (Exported energy)
Extra Indicators CC (Emissions from calcination and removals from carbonation) • CWRS (Emissions from combustion of waste from renewable
sources used in production processes) • CWNRS (Emissions from combustion of waste from non-renewable sources used in
production processes) • GWP-prod (Removals and emissions associated with biogenic carbon content of the bio-based product)
• GWP-pack (Removals and emissions associated with biogenic carbon content of the bio-based packaging)
hanson.com.au | 1300 136 464

-- 17 of 28 --

Product Environmental Performance
Slide 18
▪ The EPD values presented are indicative of local material
performance at the time of publishing and are subject to change
based on material availability and seasonal factors.
1GP = General Portland Cement, does not include SCMs.
2See Appendix for detailed explanation.
3Calculation: {1 - (GWP-tot - CO2 Reference)} / (CO2 reference).
4GWP-tot: Covers A1-A3 only. More detailed information is provided in the following mix-specific tables.
hanson.com.au | 1300 136 464
[Summary_Table]
Product
Identification EPD Registration Number Compressive strength
[MPa]
GP Content1
[kg/m3]
CO2
Reference2
[kg/m3]
CO2
Reduction3
[%]
GWP-tot4
[kg CO2
eq./m3]
Application
BN402BO31 	EPD-IES-0014761:001 	40 	337 	467 	19% 	378 	Slabs
BN402BS32 	EPD-IES-0014762:001 	40 	342 	467 	18% 	382 	Slabs
BN402DD36 	EPD-IES-0014763:001 	40 	340 	467 	19% 	380 	Slabs
GE322SM30 	EPD-IES-0014764:001 	32 	126 	390 	46% 	213 	Footings
GE322XI41 	EPD-IES-0014765:001 	32 	129 	390 	37% 	246 	Footings
GE402AA22 	EPD-IES-0014766:001 	40 	344 	467 	31% 	321 	Slabs
KM0G1AA22 	EPD-IES-0014767:001 No guaranteed
breaking strength 160 	N/A 	N/A 	179 	Kerb
P202080 	EPD-IES-0014768:001 	20 	97 	311 	61% 	124 	General use
P252080 	EPD-IES-0014769:001 	25 	98 	340 	63% 	127 	General use
P3220100 	EPD-IES-0014770:001 	32 	116 	390 	64% 	143 	General use
P322080 	EPD-IES-0014771:001 	32 	113 	390 	64% 	140 	General use
P402080 	EPD-IES-0014772:001 	40 	139 	467 	64% 	168 	General use
SAC322100 	EPD-IES-0014773:001 	32 	199 	390 	49% 	198 	Slabs
SAC32280 	EPD-IES-0014774:001 	32 	193 	390 	51% 	193 	Slabs
SAP252100 	EPD-IES-0014775:001 	25 	178 	340 	47% 	180 	Slabs
SAP25280 	EPD-IES-0014776:001 	25 	172 	340 	49% 	175 	Slabs
SAP322100 	EPD-IES-0014777:001 	32 	202 	390 	49% 	201 	Slabs
SAP32280 	EPD-IES-0014778:001 	32 	196 	390 	50% 	196 	Slabs
SAP40280 	EPD-IES-0014779:001 	40 	238 	467 	50% 	235 	Slabs

-- 18 of 28 --

Product Environmental Performance
Slide 19
▪ The EPD values presented are indicative of local material performance at the time of publishing and are subject to change based on material
availability and seasonal factors.
1GWP-tot: Covers A1-A3 only. More detailed information is provided in the following mix-specific tables.
2CO2 Baseline (simulated) is based on the Green Star Mat–4 Concrete Credit User Guide (2012). Detailed explanation is provided in the appendix.
3Plotting style: Scatter plot of values with smooth lines & markers.
hanson.com.au | 1300 136 464
[hanson_chart1]

-- 19 of 28 --

Product Environmental Performance
Slide 20 hanson.com.au | 1300 136 464
[hanson_slide1]
Product Identification 	P252080
EPD Registration Number 	EPD-IES-0014769:001
Production Site(S) 	Brisbane
Compressive Strength 	25
Density 	2480 kg/m³
Reference Service Life 	50 Years
Recycling Rate At Eol 	78%
Declared Unit 	1 m3
Scope 	A1-A3 + A4-A5 + B1-B7 + C1-C4 + D, cradle-to-grave
Methodology 	GCCA’s Industry EPD Tool for Cement and Concrete (V4.2), International version
Reference Year 	2023

-- 20 of 28 --

Product Environmental Performance
Slide 21 hanson.com.au | 1300 136 464
[hanson_slide2]
EPD Registration Number 	EPD-IES-0014769:001
Core Environmental Impact Indicators
A1-A3 	A4 	A5 	B1 	B2 	B3 	B4 	B5 	B6 	B7 	C1 	C2 	C3 	C4 	D
GWP-GHG 	kg CO₂ eq. 	1.27E+02 	2.45E+00 	9.95E+00 -2.65E+00 0.00E+00 	0.00E+00 	0.00E+00 	0.00E+00 	0.00E+00 	0.00E+00 	8.99E+00 	8.85E+00 	5.24E+00 	2.79E+00 	6.14E+00
GWP-tot 	kg CO₂ eq. 	1.27E+02 	2.45E+00 	9.95E+00 -2.65E+00 0.00E+00 	0.00E+00 	0.00E+00 	0.00E+00 	0.00E+00 	0.00E+00 	8.99E+00 	8.85E+00 	5.24E+00 	2.79E+00 	6.14E+00
GWP-fos 	kg CO₂ eq. 	1.26E+02 	2.45E+00 	9.94E+00 -2.65E+00 0.00E+00 	0.00E+00 	0.00E+00 	0.00E+00 	0.00E+00 	0.00E+00 	8.99E+00 	8.84E+00 	5.21E+00 	2.79E+00 	6.11E+00
GWP-bio 	kg CO₂ eq. 	4.62E-02 	9.59E-04 	4.35E-03 	0.00E+00 	0.00E+00 	0.00E+00 	0.00E+00 	0.00E+00 	0.00E+00 	0.00E+00 	1.60E-03 	6.32E-03 	1.89E-02 	1.84E-03 	1.89E-02
GWP-luc 	kg CO₂ eq. 	2.92E-02 	8.29E-04 	3.31E-03 	0.00E+00 	0.00E+00 	0.00E+00 	0.00E+00 	0.00E+00 	0.00E+00 	0.00E+00 	1.13E-03 	5.14E-03 	1.44E-02 	1.50E-03 	1.44E-02
ODP 	kg CFC 11 eq. 	6.34E-06 	4.67E-07 	1.30E-06 	0.00E+00 	0.00E+00 	0.00E+00 	0.00E+00 	0.00E+00 	0.00E+00 	0.00E+00 	1.62E-06 	1.49E-06 	3.64E-07 	9.09E-07 	3.64E-07
AP 	mol H+ eq. 	6.10E-01 	1.27E-02 	8.94E-02 	0.00E+00 	0.00E+00 	0.00E+00 	0.00E+00 	0.00E+00 	0.00E+00 	0.00E+00 	9.42E-02 	5.34E-02 	3.85E-02 	2.67E-02 	3.85E-02
EP-fw 	kg P eq. 	2.62E-02 	1.83E-04 	2.01E-03 	0.00E+00 	0.00E+00 	0.00E+00 	0.00E+00 	0.00E+00 	0.00E+00 	0.00E+00 	4.02E-04 	1.18E-03 	3.00E-03 	3.27E-04 	3.00E-03
EP-mar 	kg N eq. 	1.96E-03 	1.59E-05 	6.85E-04 	0.00E+00 	0.00E+00 	0.00E+00 	0.00E+00 	0.00E+00 	0.00E+00 	0.00E+00 	3.34E-05 	8.74E-05 	2.08E-04 	3.09E-05 	2.08E-04
EP-ter 	mol N eq. 	1.40E+00 	4.54E-02 	3.30E-01 	0.00E+00 	0.00E+00 	0.00E+00 	0.00E+00 	0.00E+00 	0.00E+00 	0.00E+00 	4.44E-01 	1.88E-01 	7.19E-02 	9.58E-02 	7.19E-02
POCP 	kg NMVOC eq. 	3.87E-01 	1.37E-02 	9.11E-02 	0.00E+00 	0.00E+00 	0.00E+00 	0.00E+00 	0.00E+00 	0.00E+00 	0.00E+00 	1.22E-01 	5.50E-02 	2.03E-02 	2.81E-02 	2.03E-02
ADPE 	kg Sb eq. 	1.78E-04 	4.57E-06 	7.27E-06 	0.00E+00 	0.00E+00 	0.00E+00 	0.00E+00 	0.00E+00 	0.00E+00 	0.00E+00 	2.66E-06 	1.56E-05 	4.48E-06 	3.04E-06 	4.48E-06
ADPF 	MJ, net calorific value 	9.99E+02 	3.86E+01 	1.28E+02 	0.00E+00 	0.00E+00 	0.00E+00 	0.00E+00 	0.00E+00 	0.00E+00 	0.00E+00 	1.30E+02 	1.32E+02 	7.48E+01 	7.77E+01 	7.48E+01
WDP 	m³ world eq. deprived 	7.59E+01 	2.84E-01 	-1.38E+00 0.00E+00 	0.00E+00 	0.00E+00 	0.00E+00 	0.00E+00 	0.00E+00 	0.00E+00 	7.67E-01 	1.14E+00 	1.05E+00 	3.75E+00 	1.05E+00
Parameters Describing Resource Use
A1-A3 	A4 	A5 	B1 	B2 	B3 	B4 	B5 	B6 	B7 	C1 	C2 	C3 	C4 	D
PERE 	MJ, net calorific value 	4.49E+01 	1.12E+00 	5.48E+00 	0.00E+00 	0.00E+00 	0.00E+00 	0.00E+00 	0.00E+00 	0.00E+00 	0.00E+00 	7.59E-01 	4.82E+00 	8.18E+00 	2.02E+00 	8.18E+00
PERM 	MJ, net calorific value 	0.00E+00 	0.00E+00 	0.00E+00 	0.00E+00 	0.00E+00 	0.00E+00 	0.00E+00 	0.00E+00 	0.00E+00 	0.00E+00 	0.00E+00 	0.00E+00 	0.00E+00 	0.00E+00 	0.00E+00
PERT 	MJ, net calorific value 	4.49E+01 	1.12E+00 	5.48E+00 	0.00E+00 	0.00E+00 	0.00E+00 	0.00E+00 	0.00E+00 	0.00E+00 	0.00E+00 	7.59E-01 	4.82E+00 	8.18E+00 	2.02E+00 	8.18E+00
PENRE 	MJ, net calorific value 	1.01E+03 	3.86E+01 	1.28E+02 	0.00E+00 	0.00E+00 	0.00E+00 	0.00E+00 	0.00E+00 	0.00E+00 	0.00E+00 	1.30E+02 	1.32E+02 	7.48E+01 	7.77E+01 	7.48E+01
PENRM 	MJ, net calorific value 	0.00E+00 	0.00E+00 	0.00E+00 	0.00E+00 	0.00E+00 	0.00E+00 	0.00E+00 	0.00E+00 	0.00E+00 	0.00E+00 	0.00E+00 	0.00E+00 	0.00E+00 	0.00E+00 	0.00E+00
PENRT 	MJ, net calorific value 	1.01E+03 	3.86E+01 	1.28E+02 	0.00E+00 	0.00E+00 	0.00E+00 	0.00E+00 	0.00E+00 	0.00E+00 	0.00E+00 	1.30E+02 	1.32E+02 	7.48E+01 	7.77E+01 	7.48E+01
SM 	kg 	1.37E+02 	0.00E+00 	1.37E+00 	0.00E+00 	0.00E+00 	0.00E+00 	0.00E+00 	0.00E+00 	0.00E+00 	0.00E+00 	0.00E+00 	0.00E+00 	0.00E+00 	0.00E+00 	0.00E+00
RSF 	MJ, net calorific value 	1.92E+00 	0.00E+00 	1.92E-02 	0.00E+00 	0.00E+00 	0.00E+00 	0.00E+00 	0.00E+00 	0.00E+00 	0.00E+00 	0.00E+00 	0.00E+00 	0.00E+00 	0.00E+00 	0.00E+00
NRSF 	MJ, net calorific value 	3.19E+01 	0.00E+00 	3.19E-01 	0.00E+00 	0.00E+00 	0.00E+00 	0.00E+00 	0.00E+00 	0.00E+00 	0.00E+00 	0.00E+00 	0.00E+00 	0.00E+00 	0.00E+00 	0.00E+00
NFW 	m³ 	2.19E+00 	8.51E-03 	1.18E-01 	0.00E+00 	0.00E+00 	0.00E+00 	0.00E+00 	0.00E+00 	0.00E+00 	0.00E+00 	1.99E-02 	3.53E-02 	4.25E-02 	8.74E-02 	4.25E-02

-- 21 of 28 --

Product Environmental Performance
Slide 22 hanson.com.au | 1300 136 464
[hanson_slide3]
EPD Registration Number 	EPD-IES-0014769:001
Additional Environmental Impact Indicators
A1-A3 	A4 	A5 	B1 	B2 	B3 	B4 	B5 	B6 	B7 	C1 	C2 	C3 	C4 	D
PM 	Disease incidence 	5.40E-06 	2.26E-07 1.67E-06 0.00E+00 0.00E+00 0.00E+00 0.00E+00 0.00E+00 0.00E+00 0.00E+00 2.45E-06 8.25E-07 3.44E-07 4.98E-07 3.44E-07
IRP 	kBq U235 eq. 	3.68E+02 	2.03E-01 4.23E+00 0.00E+00 0.00E+00 0.00E+00 0.00E+00 0.00E+00 0.00E+00 0.00E+00 6.08E-01 7.56E-01 8.03E-01 3.59E-01 8.03E-01
ETP 	CTUe 	3.66E+02 	8.15E+00 7.39E+00 0.00E+00 0.00E+00 0.00E+00 0.00E+00 0.00E+00 0.00E+00 0.00E+00 1.76E+00 2.31E+01 1.57E+00 1.47E+00 1.57E+00
HTPC 	CTUh 	6.96E-07 	1.57E-08 1.89E-07 0.00E+00 0.00E+00 0.00E+00 0.00E+00 0.00E+00 0.00E+00 0.00E+00 6.36E-08 1.00E-07 6.22E-08 2.44E-08 6.22E-08
HTPNC 	CTUh 	9.87E-06 	4.39E-07 8.87E-07 0.00E+00 0.00E+00 0.00E+00 0.00E+00 0.00E+00 0.00E+00 0.00E+00 2.46E-07 1.39E-06 2.87E-07 1.56E-07 2.87E-07
SQP 	dimensionless 	8.28E+02 	6.85E+01 3.77E+01 0.00E+00 0.00E+00 0.00E+00 0.00E+00 0.00E+00 0.00E+00 0.00E+00 7.71E+00 2.15E+02 6.11E+01 1.45E+02 6.11E+01
Other Environmental Information Describing Waste Categories
A1-A3 	A4 	A5 	B1 	B2 	B3 	B4 	B5 	B6 	B7 	C1 	C2 	C3 	C4 	D
HWD 	kg 	0.00E+00 	0.00E+00 0.00E+00 0.00E+00 0.00E+00 0.00E+00 0.00E+00 0.00E+00 0.00E+00 0.00E+00 0.00E+00 0.00E+00 0.00E+00 0.00E+00 0.00E+00
NHWD 	kg 	4.08E-02 	0.00E+00 6.78E+00 0.00E+00 0.00E+00 0.00E+00 0.00E+00 0.00E+00 0.00E+00 0.00E+00 0.00E+00 0.00E+00 0.00E+00 6.77E+02 0.00E+00
RWD 	kg 	0.00E+00 	0.00E+00 0.00E+00 0.00E+00 0.00E+00 0.00E+00 0.00E+00 0.00E+00 0.00E+00 0.00E+00 0.00E+00 0.00E+00 0.00E+00 0.00E+00 0.00E+00
Environmental Information Describing Output Flows
A1-A3 	A4 	A5 	B1 	B2 	B3 	B4 	B5 	B6 	B7 	C1 	C2 	C3 	C4 	D
CRU 	kg 	0.00E+00 	0.00E+00 0.00E+00 0.00E+00 0.00E+00 0.00E+00 0.00E+00 0.00E+00 0.00E+00 0.00E+00 0.00E+00 0.00E+00 0.00E+00 0.00E+00 0.00E+00
MFR 	kg 	0.00E+00 	0.00E+00 1.80E+01 0.00E+00 0.00E+00 0.00E+00 0.00E+00 0.00E+00 0.00E+00 0.00E+00 0.00E+00 0.00E+00 1.80E+03 0.00E+00 1.80E+03
MER 	kg 	0.00E+00 	0.00E+00 0.00E+00 0.00E+00 0.00E+00 0.00E+00 0.00E+00 0.00E+00 0.00E+00 0.00E+00 0.00E+00 0.00E+00 0.00E+00 0.00E+00 0.00E+00
EE 	kg 	0.00E+00 	0.00E+00 0.00E+00 0.00E+00 0.00E+00 0.00E+00 0.00E+00 0.00E+00 0.00E+00 0.00E+00 0.00E+00 0.00E+00 0.00E+00 0.00E+00 0.00E+00
Extra Indicators
A1-A3 	A4 	A5 	B1 	B2 	B3 	B4 	B5 	B6 	B7 	C1 	C2 	C3 	C4 	D
CC 	kg CO₂ eq. 	4.63E+01 	0.00E+00 4.04E-01 -2.65E+00 0.00E+00 0.00E+00 0.00E+00 0.00E+00 0.00E+00 0.00E+00 0.00E+00 0.00E+00 -8.96E-01 0.00E+00 0.00E+00
CWRS 	kg CO₂ eq. 	2.40E-03 	0.00E+00 2.40E-05 0.00E+00 0.00E+00 0.00E+00 0.00E+00 0.00E+00 0.00E+00 0.00E+00 0.00E+00 0.00E+00 0.00E+00 0.00E+00 0.00E+00
CWNRS 	kg CO₂ eq. 	2.70E+00 	0.00E+00 2.70E-02 0.00E+00 0.00E+00 0.00E+00 0.00E+00 0.00E+00 0.00E+00 0.00E+00 0.00E+00 0.00E+00 0.00E+00 0.00E+00 0.00E+00
GWP-prod kg CO₂ 	0.00E+00 	0.00E+00 0.00E+00 0.00E+00 0.00E+00 0.00E+00 0.00E+00 0.00E+00 0.00E+00 0.00E+00 0.00E+00 0.00E+00 0.00E+00 0.00E+00 0.00E+00
GWP-pack kg CO₂ 	0.00E+00 	0.00E+00 0.00E+00 0.00E+00 0.00E+00 0.00E+00 0.00E+00 0.00E+00 0.00E+00 0.00E+00 0.00E+00 0.00E+00 0.00E+00 0.00E+00 0.00E+00

-- 22 of 28 --

References

-- 23 of 28 --

Program Information
Silde 24
EPD Owner Hanson Construction Materials Pty Ltd
L14, 35 Clarence St, Sydney NSW 2000
Phone: 1300 136 464
Online: hanson.com.au
Programme Operator EPD International AB Box 210 60 SE-100 31 Stockholm Sweden
Online: www.environdec.com
Email: info@environdec.com
Regional Programme EPD Australasia, 315a Hardy St, Nelson 7010 New Zealand
Online: epd-australasia.com
Email: info@epd-Australasia.com
Process EPD Certified By Katherine McFeaters
Epsten Group, Inc.
101 Marietta St. NW, Suite 2600, Atlanta, Georgia 30303, USA
www.epstengroup.com
Accredited by: A2LA, Certificate #3142.03
Product Category Rules CEN standard EN 15804:A2 (PCR 2019:14 Construction Products, Version 1.3.4) served as the core PCR.
Environdec c-PCR-003 Concrete, concrete elements (EN 16757:2023) served as sub-PCR.
EN 15804 PCR Review The Technical Committee of the International EPD®System. Chair: Claudia A. Peña.
The review panel may be contacted via info@environdec.com.
EPD Registration Number EPD-IES-0014769:001
Independent Verification of the Declaration and Data, According to
ISO 14025:
❑ EPD process certification
❑ EPD verification
Valid From 2024-08-26
Valid To 2029-08-26
Version 1.0 2024-08-26
Description of Version Differences (if NOT VERSION 1.0) N/A
Geographical Scope Queensland - Brisbane
Important Notes EPDs within the same product category but from different programmes may not be comparable.
EPDs of construction products may not be comparable if they do not comply with EN 15804.
The EPD Owner maintains full ownership, liability and responsibility for the EPD.
Product Group Classification UN CPC 88 - Concrete, cement and plaster article manufacturing services
ANZSIC Classification 2033 Ready Mix Concrete Manufacturing
hanson.com.au | 1300 136 464
x

-- 24 of 28 --

References
Slide 25
1) Australian Life Cycle Assessment Society. (2015). Australian Life Cycle Inventory Database Initiative. Retrieved from http://www.auslci.com.au
2) National Waste Report. (2022). https://www.dcceew.gov.au/environment/protection/waste/publications/national-waste-reports. Canberra: Department of Climate
Change, Energy, the Environment and Water.
3) Ecoinvent. (2018, August 23). ecoinvent 3.5 (database). Retrieved from https://www.ecoinvent.org/database/older-versions/ecoinvent-35/ecoinvent-35.html
4) EPD International. (2024). General Programme Instructions for the International EPD® System v5.0. Retrieved from envirodec.com
5) EPD Australasia Regional Annex (2024) – Version 4.2 Retrieved from epd-australasia.com
6) European Committee for Standardisation (CEN). (2022). EN 16757:2022: Sustainability of construction works - Environmental product declarations - Product Category
Rules for concrete and concrete elements.
7) European Committee for Standardisation (CEN). (2017, February). EN 16908:2017: Cement and building lime - Environmental Product Declarations - Product
Category Rules complementary to EN 15804. Brussels.
8) European Committee for Standardisation (CEN). (2019). EN 15804:2012+A2:2019: Sustainability of construction works - Environmental product declarations - Core
rules for the product category of construction products. Brussels.
9) Google. (n.d.). Google Maps. Retrieved from https://www.google.com.au/maps/
10) International Organization for Standardization. (2015). ISO14020 Environmental Labels and Declarations - General Principles.
11) International Organization for Standardization. (2017). ISO14025 Environmental Labels and Declarations - Type III Environmental Declarations - Principles and
Procedures.
12) International Organization for Standardization. (2020). ISO 14044 Environmental Management - Life Cycle Assessment - Requirements and Guidelines.
13) McConnell, D., Holmes a Court, S., Tan, S., & Cubrilovic, N. (2022). OpenNEM. Retrieved 2023, from https://opennem.org.au/
14) Quantis. (2023). GCCA's Industry EPD Tool for Cement and Concrete. Retrieved from https://concrete-epd-tool.org/
15) Green Star Mat–4 Concrete Credit User Guide (2012). Retrieved from Mat-4 (gbca.org.au)
hanson.com.au | 1300 136 464

-- 25 of 28 --

hanson.com.au | 1300 136 464

-- 26 of 28 --

CO2 Baseline
94%
5% 1%
GWP-tot [kg CO2 eq.]
For Materials (A1-A3)
Cement
Aggregates & Sand
Others
Material Quantity Travel Distance
Cement 440 kg Truck: 100 km, Rail: 100 km
Aggregates & Sand 1821 kg Truck: 90 km
Water 197 L
Admixtures 3 L Truck: 100 km, Rail: 600 km
CO2 Baseline(simulated): 40 MPa
▪ Due to the lack of an industry wide CO2 baseline, we simulated our
own baseline mixes:
▪ Based on the Green Star Mat–4 Concrete Credit User Guide (2012)
▪ Cement reference values were added to the GCCA concrete EPD tool
▪ Default values (Australia specific)
▪ The background information (incl. assumptions, generic mix designs) can be
downloaded here: https://hanson.com.au/background-gs-benchmarks.zip
hanson.com.au | 1300 136 464

-- 27 of 28 --

CO2 Service Offer
Pre-
Project
Running
Project
Post
Project
CO2 is set to become a crucial budgeting currency in the construction
sector. As such, it must be managed accordingly. Most provided
embodied carbon emission data out there is based on estimates and
typically handed over to the customer before a project starts.
At Hanson, we believe there’s a better way to communicate carbon
values, which also eliminates the current gap of carbon monitoring options
during the construction phase in the market:
1) Pre-project: Predicting - We can provide you indicative CO2 values for
your specific project with our 3rd party verified CO2 calculator (targeted
& fast & reliable).
2) Running project: Monitoring - You get regular updates of your deliveries
and how you track towards your carbon targets (no more surprises).
3) Post-project: Verification - You’ll receive a final report and a project-
specific EPD based on actual deliveries (highest accuracy).
hanson.com.au | 1300 136 464

-- 28 of 28 --

