Environmental Product Declaration
IN ACCORDANCE WITH EN 15804+A2 & ISO 14025
Boral | 1
Environmental Product
Declaration
50MPa 20mm Enviro 50% SCM 100SL
Conc
Melbourne
EPD HUB, HUB-5556
Published on 27.02.2026, last updated on 27.02.2026, valid until 26.02.2031
In accordance with EN 15804+A2 & ISO 14025 / ISO 21930

-- 1 of 20 --

Environmental Product Declaration
IN ACCORDANCE WITH EN 15804+A2 & ISO 14025
Boral | 2
Contents
Environmental Product Declaration ..................................................................................................................1
General information ............................................................................................................................................3
Manufacturer and site ........................................................................................................................................3
EPD standards, scope and verification .............................................................................................................3
Product specification .........................................................................................................................................4
Product characteristics ......................................................................................................................................4
Environmental data summary ............................................................................................................................4
Life cycle assessment.........................................................................................................................................5
System boundaries ............................................................................................................................................5
Cut-off criteria ....................................................................................................................................................5
Validation of Data ..............................................................................................................................................5
Allocation, estimates and assumptions .............................................................................................................6
Product & manufacturing sites grouping ...........................................................................................................6
Product raw material main composition ............................................................................................................6
Substances, REACH – very high concern .........................................................................................................6
Biogenic carbon content ....................................................................................................................................6
About Boral ..........................................................................................................................................................7
Product life-cycle ...............................................................................................................................................11
Manufacturing (A1-A3) ....................................................................................................................................11
Transport and installation (A4-A5) ...................................................................................................................11
Product use and maintenance (B1-B7) ...........................................................................................................11
Product end-of-life (C1-C4, D) .........................................................................................................................11
System Diagram ..............................................................................................................................................12
LCA software and bibliography .......................................................................................................................12
Environmental impact data...............................................................................................................................13
Core environmental impact indicators – EN 15804+A2, EF 3.1 ......................................................................13
Additional environmental impact indicators – EN 15804+A2, EF 3.1 ..............................................................14
Use of natural resources .................................................................................................................................15
End of life – Waste ..........................................................................................................................................16
End of life – Output flows.................................................................................................................................17
Environmental impacts – EN 15804+A1, CML / ISO 21930 ...........................................................................17
Additional indicator – GWP-GHG ....................................................................................................................18
Scenario documentation...................................................................................................................................19
Third-party verification statement ...................................................................................................................20

-- 2 of 20 --

Environmental Product Declaration
IN ACCORDANCE WITH EN 15804+A2 & ISO 14025
Boral | 3
General information
Manufacturer and site
Manufacturer Boral Limited
Address Level 3, Triniti 2, 39 Delhi Rd, North Ryde NSW, AU
Contact details sustainability@boral.com.au
Website www.boral.com.au
Place of production Melbourne
Place(s) of raw material origin Australia
Place(s) of installation and use Australia
Period for data FY25
EPD standards, scope and verification
Program operator EPD Hub, hub@epdhub.com
Reference standard EN 15804:2012+A2:2019/AC:2021 and ISO 14025
PCR EPD Hub Core PCR version 1.2, 24 Mar 2025
cPCR EN 16757 Product Category Rules for concrete and concrete elements
Sector Construction product
Category of EPD Third party verified EPD
Scope of the EPD Cradle-to-gate (A1-3) with modules C1-4, D
EPD author Lewis Beard (Boral Construction Materials Ltd)
EPD verification
Independent verification of this EPD and data, according to ISO
14025:
 Internal verification
 External verification
EPD verifier Vera Durão, as an authorised verifier acting for EPD Hub Limited

-- 3 of 20 --

Environmental Product Declaration
IN ACCORDANCE WITH EN 15804+A2 & ISO 14025
Boral | 4
Product specification
Product name 50MPa 20mm Enviro 50% SCM 100SL Conc
Concrete type Ready-mix concrete
Product standards AS 1379 Specification and supply of concrete
Product description
Boral’s ENVIROCRETE® concrete is a lower carbon concrete product which complies
with AS 1379. It contains supplementary cementitious materials to reduce the portland
cement content. ENVIROCRETE® concrete is available with two levels of portland
cement reduction. ENVIROCRETE® 30% has a minimum portland cement reduction of
30% compared to the GBCA and ISC reference case and ENVIROCRETE® 40% has a
minimum portland cement reduction of 40% when compared to the GBCA and ISC
reference case. ENVIROCRETE® 30% and 40% are ideal for general applications
where high-performance concrete is not required.
A1-A3 Specific data (%) 99.5
Product characteristics
Compressive strength class:
S50
Strength evaluation days:
28 days
This EPD is intended for business-to-business and/or business-to-consumer communication. Life Cycle Assessment study
has been performed in accordance with the requirements of EN 15804, EPD Hub PCR version 1.2 (24 Mar 2025) and JRC
characterisation factors EF 3.1. The manufacturer has the sole ownership, liability, and responsibility for the EPD. EPDs
within the same product category but from different programs may not be comparable. EPDs of construction products may
not be comparable if they do not comply with EN 15804 and if they are not compared in a building context.
Environmental data summary
Declared unit 1 cubic metre
Declared unit mass, kg 2377
GWP-total, A1-A3 (kg CO₂e) 2.68E+02
GWP-fossil, A1-A3 (kg CO₂e) 2.68E+02
Secondary material, inputs (%) 0
Secondary material, outputs (%) 70
Total energy use, A1-A3 (kWh) 374
Net freshwater use, A1-A3 (m3) 5.19E+00

-- 4 of 20 --

Environmental Product Declaration
IN ACCORDANCE WITH EN 15804+A2 & ISO 14025
Boral | 5
Life cycle assessment
System boundaries
This EPD covers the life-cycle modules listed in the following table.
Product stage Assembly
stage
Use stage End of life stage Beyond the
system
A1 A2 A3 A4 A5 B1 B2 B3 B4 B5 B6 B7 C1 C2 C3 C4 D
x x x ND ND ND ND ND ND ND ND ND x x x x x x x
Raw materials	
Transport	
Manufacturing	
Transport	
Assembly	
Use	
Maintenance	
Repair
Replacement	
Refurbishment	
Operational energy use	
Operational water use	
Deconstruction/ demolition	
Transport	
Waste processing	
Disposal	
Reuse
Recovery	
Recycling
Modules not declared = ND
Cut-off criteria
The study does not exclude any modules or processes which are stated mandatory in the reference standard and the
applied PCR. The study does not exclude any hazardous materials or substances. There is no neglected unit process
more than 1% of total mass or energy flows. The module specific total neglected input and output flows also do not
exceed 5% of energy usage or mass.
The production of capital equipment, construction activities, and infrastructure, maintenance and operation of capital
equipment, personnel-related activities, energy and water use related to company management and sales activities
are excluded.
Validation of Data
Data collection for production, transport, and packaging was conducted using time and site-specific information, as
defined in the general information section on page 1 and 2. Upstream process calculations rely on generic data as
defined in the Bibliography section. Manufacturer-provided specific and generic data were used for the product’s
manufacturing stage. The analysis was performed in One Click LCA EPD Generator, with the 'Cut-Off, EN 15804+A2'
allocation method, and characterisation factors according to EN 15804:2012+A2:2019/AC:2021 and JRC EF 3.1.

-- 5 of 20 --

Environmental Product Declaration
IN ACCORDANCE WITH EN 15804+A2 & ISO 14025
Boral | 6
Allocation, estimates and assumptions
All allocations are done as per the reference standards and the applied PCR. In this study, allocation has been done in the
following ways:
Data type Allocation
Raw materials No allocation
Packaging materials Not applicable
Ancillary materials Allocated by mass
Manufacturing energy and waste Allocated by mass
Product & manufacturing sites grouping
Type of grouping Multiple sites
Grouping method Based on average results of product group - by total
volume
Variation in GWP-fossil for A1-A3, % Variation in GWP for modules A1-A3 is -0.4% to 1.4%
This EPD is declared as a single product manufactured at multiple sites in the Melbourne metropolitan region of Victoria.
These sites are grouped together on the basis of having the same supply chain and major production steps. Results are
averaged by production volume across the sites. There are 8 sites covered in this region: Deer Park, Tullamarine, Somerton,
Sunbury, Wollert, Melton, West Melbourne, and West Melbourne (wet).
Product raw material main composition
The product is a ready-mix concrete consisting of aggregates, cement, filler, admixtures, and water. Main material categories
as per EPD Hub GPI are shown below:
Raw material category Amount, mass- % Material origin
Metals 0 -
Minerals 100 Australia
Fossil materials 0 -
Bio-based materials 0 -
Substances, REACH – very high concern
The product does not contain any REACH SVHC substances in amounts greater than 0.1 % (1000 ppm).
Biogenic carbon content
This product does not contain any biogenic carbon content in amounts greater than 5%.

-- 6 of 20 --

Environmental Product Declaration
IN ACCORDANCE WITH EN 15804+A2 & ISO 14025
Boral | 7
About Boral
Boral is Australia’s largest vertically-integrated construction materials company.
That means we not only supply customers with outstanding raw materials like
aggregate and sand, we also develop and produce advanced construction
materials and solutions like low-carbon concretes and advanced asphalts.
Our network includes prized quarry and cement infrastructure, bitumen, construction materials recycling, asphalt and
concrete batching operations. We work year-round to help customers deliver high-profile civil works and major
infrastructure projects, as well as key residential, commercial and industrial developments.
We employ about 7,500 employees and contractors working in research, production and business support across
more than 360 locations nationwide.
For nearly 80 years, we’ve been building something great in Australia. From the surface of the Sydney Harbour Bridge to
the walls of Melbourne’s Metro Tunnel, from the asphalt at Adelaide Airport right through to much of the concrete used in
Brisbane’s Gateway Bridge and Perth’s Forrestville Airport Link, Boral has been making history around Australia.
Boral concrete has over 200 pre-mix concrete plants around Australia producing a wide range of concrete mixes in
metropolitan and country areas. Boral concrete supplies pre-mix concrete to all segments of the construction
industry including infrastructure, social, commercial and residential construction.

-- 7 of 20 --

Environmental Product Declaration
IN ACCORDANCE WITH EN 15804+A2 & ISO 14025
Boral | 8
Our integrated network
Valuable upstream and downstream operations with market leadership.
Boral moves ~50 million tonnes of products per year across its network

-- 8 of 20 --

Environmental Product Declaration
IN ACCORDANCE WITH EN 15804+A2 & ISO 14025
Boral | 9
A lower carbon concrete product
for every option
Boral’s range of lower carbon concrete products will help you achieve your
sustainability, engineering and architectural goals.
Boral Concrete’s Lower Carbon Concrete
(LCC) products can be used for all types of
structures including:
• houses
• commercial buildings
• multi-residential buildings
• high-rise buildings
• civil projects, and
• infrastructure projects.
By matching the engineering properties of each
product with the structural requirements, the
carbon footprint of the project can be reduced
for the optimal cost.
Traditional lower carbon concrete products have low
early age strength and may have higher drying
shrinkage which makes them less desirable for many
applications. In particular, they are unsuitable for
precast elements and post tensioned slabs.
Lower carbon concrete products
For all types of Structures
Boral’s Lower Carbon Concrete (LCC) products
include products with good early age strength
and superior engineering properties. They can be
used for precast and post tensioned slabs so there is
no compromise to the construction schedule and
engineers can take advantage of the superior drying
shrinkage properties.
Boral has three product ranges: ENVIROCRETE®,
ENVIROCRETE® PLUS and ENVISIA®.
ENVIROCRETE® concrete is a traditional lower
carbon concrete product, Envirocrete® plus has
better early age strength and drying shrinkage
properties and Envisia® concrete has the best early
age strength and drying shrinkage properties.
ENVISIA® concrete also has a light colour
and exhibits a very good appearance in an
off–formwork finish.

-- 9 of 20 --

Environmental Product Declaration
IN ACCORDANCE WITH EN 15804+A2 & ISO 14025
Boral | 10
1 Green Building Council of Australia (GBCA). 2 Infrastructure Sustainability Council (ISC). 3 Using the reference case from the GBCA Design and As-Built
v1.3 rating tool. 4 The portland cement reductions in the table do not apply to Tasmania. Please contact the Boral Tasmanian office. 5 For specific values
contact the local Boral office. 6 The dots indicate the relative reduction in embodied carbon. The hollow dots represent the potential relative reduction in
embodied carbon. Contact the local Boral office for specific embodied carbon values. Alternatively, they can be found in Boral’s Environmental Product
Declarations which can be downloaded from boral.com.au/EPDs.
Lower carbon
concrete
products
For all types
of structures
ENVIROCRETE®
products
Are suitable for all general
applications where good
early age strength and low
drying shrinkage are
not required.
ENVIROCRETE® PLUS
products
Have good early age strength
and can be used for some
post tensioned applications.
They also have good drying
shrinkage characteristics which
will comply with the shrinkage
requirements in most
engineering specifications.
ENVISIA®
products
Have excellent early age
strength and drying shrinkage
characteristics.
They can be used for all
standard post tensioned
concrete applications and their
low shrinkage characteristics
provides engineers and
architects with more design
options. They have a light
colour which provides
architectural benefits, and they
have excellent resistant to
chloride ingress making them
suitable for marine environments.
• Low portland cement.
• Low embodied carbon.
• General applications.
• Suitable for projects targeting
a GBCA1 or ISC2 rating.
• Low portland cement.
• Low embodied carbon.
• General applications.
• Suitable for projects targeting
a GBCA1 or ISC2 rating.
• Low portland cement.
• Low embodied carbon.
• Low drying shrinkage.
• Good early age strength,
suitable for most standard
post tension applications.
• Suitable for projects targeting
a GBCA1 or ISC2 rating.
• Low portland cement.
• Low embodied carbon.
• Very low drying shrinkage.
• Good early age strength,
suitable for all standard
post tension applications.
• Very low drying shrinkage.
• Excellent resistance to
chloride ingress.
• Light colour provides
architectural benefits.
• Suitable for projects targeting
a GBCA1 or ISC2 rating.
Environmental properties
Reduction in
Portland cement3,4,5 30% - 70% 45% - 70% 50% - 70%
Reduction in
embodied carbon6
Engineering and durability properties
Early age strength
Drying shrinkage
Durability in a
marine environment

-- 10 of 20 --

Environmental Product Declaration
IN ACCORDANCE WITH EN 15804+A2 & ISO 14025
Boral | 11
Product life-cycle
Manufacturing (A1-A3)
The environmental impacts considered for the product stage cover the manufacturing of raw materials used in the
production. Also, fuels used by machines, and handling of waste formed in the production processes at the manufacturing
facilities are included in this stage. The study also considers the material losses occurring during the manufacturing
processes as well as losses during electricity transmission and transformation. A market-based approach is used in
modelling the electricity mix utilised in the batch plant.
Ready-mix concrete production starts by transporting the binders, aggregates, and additives to the manufacturing site and
storing them into closed silos and containers. The considered transportation impacts include exhaust emissions resulting
from transportation of raw materials from suppliers to manufacturing facilities as well as the environmental impacts of the
production of the fuel used. The manufacturing, maintenance and disposal of the vehicles as well as tyre and road wear
during transportation have also been included. The transportation distances and methods are based on the known supply
chain for this product using information collected from local Boral teams, including road, rail and shipping. Where multiple
manufacturing sites are being grouped, distances are averaged across the sites.
The aggregates are dosed onto a scale and transferred to a concrete mixer. In the mixer, cement is added to the
aggregates, after which the material is mixed dry. Water and additives are then added to the mixture, followed by wet
mixing. After mixing, the concrete mass is unloaded from the mixer into the tank of the concrete agitator truck, which is
transported to the construction site.
No packaging is included as the product is transported with mixer trucks.
Transport and installation (A4-A5)
Installation includes the energy used for concrete application. This consists of the energy spent by a concrete mixer truck
and a concrete pump.
Modules not declared.
Product use and maintenance (B1-B7)
This EPD does not cover the use phase. Air, soil, and water impacts during the use phase have not been studied.
Carbonation is not taken into account in this EPD.
Modules not declared.
Product end-of-life (C1-C4, D)
At the end of its life, the concrete is assumed to be part of a concrete building that is demolished using machinery,
consuming energy in the form of diesel (C1).
The concrete recovered after demolition is delivered 50 km by truck to the nearest construction waste treatment site
(C2). It is assumed that 100% of the demolished concrete is transported to a site where this waste is processed by
crushing the blocks to gravel. About 70% of concrete can be recycled this way (C3), with an assumption that non-
reinforced concrete is being sorted (Gervasio, H. and Dimova, S., 2018. Model for Life Cycle Assessment (LCA) of
buildings. European Commission, Joint Research Centre.). The remaining 30% of concrete is assumed to be sent to the
landfill for disposal (C4). The crushed concrete received from waste treatment can be used as a replacement for virgin
gravel or for raw materials in road construction (D). The process losses of the waste treatment plant are assumed to be
negligible.

-- 11 of 20 --

Environmental Product Declaration
IN ACCORDANCE WITH EN 15804+A2 & ISO 14025
Boral | 12
System Diagram
This system shows the system boundary with dashed lines and shows included modules in green, while excluded ones
are in grey.
LCA software and bibliography
The LCA and EPD have been prepared according to the reference standards and ISO 14040/14044. Ecoinvent v3.10.1
and One Click LCA databases were used as sources of environmental data. Allocation used in Ecoinvent 3.10.1
environmental data sources follow the methodology ‘allocation, cut-off, EN 15804+A2‘.

-- 12 of 20 --

Environmental Product Declaration
IN ACCORDANCE WITH EN 15804+A2 & ISO 14025
Boral | 13
Environmental impact data
The estimated impact results are only relative statements which do not indicate the end points of the impact
categories, exceeding threshold values, safety margins or risks.
Core environmental impact indicators – EN 15804+A2, EF 3.1
Impact category Unit A1 A2 A3 A1-A3
GWP – total1 kg CO2e 2.56E+02 6.58E+00 5.62E+00 2.68E+02
GWP – fossil kg CO2e 2.56E+02 6.57E+00 5.62E+00 2.68E+02
GWP – biogenic kg CO2e 9.46E-02 1.23E-02 7.60E-04 1.08E-01
GWP – LULUC kg CO2e 9.12E-02 5.06E-05 4.66E-04 9.18E-02
Ozone
depletion pot. kg CFC-11e 1.94E-06 1.08E-06 4.97E-08 3.07E-06
Acidification
potential mol H+e 1.84E+00 2.70E-02 3.63E-02 1.90E+00
EP-freshwater2 kg Pe 4.83E-02 2.17E-04 9.12E-04 4.94E-02
EP-marine kg Ne 4.54E-01 9.07E-03 7.66E-03 4.70E-01
EP-terrestrial mol Ne 4.91E+00 1.01E-01 8.11E-02 5.09E+00
POCP
(“smog”)3 kg NMVOCe 1.31E+00 3.41E-02 2.48E-02 1.37E+00
ADP-minerals &
metals4 kg Sbe 3.67E-06 2.11E-05 2.10E-06 2.69E-05
ADP-fossil
resources MJ 1.11E+03 8.45E+01 6.82E+01 1.27E+03
Water use5 m3e depr. 2.29E+02 5.74E+01 3.69E+01 3.24E+02

-- 13 of 20 --

Environmental Product Declaration
IN ACCORDANCE WITH EN 15804+A2 & ISO 14025
Boral | 14
Impact category Unit C1 C2 C3 C4 D
GWP – total kg CO2e 4.52E+00 1.28E+01 7.28E+00 4.45E+00 -1.30E+01
GWP – fossil kg CO2e 4.52E+00 1.28E+01 7.28E+00 4.45E+00 -1.29E+01
GWP – biogenic kg CO2e 4.61E-04 2.90E-03 -7.43E-04 -1.42E-03 -4.06E-02
GWP – LULUC kg CO2e 4.63E-04 5.72E-03 7.46E-04 2.54E-03 -1.79E-02
Ozone
depletion pot. kg CFC-11e 6.92E-08 1.89E-07 1.11E-07 1.29E-07 -1.09E-06
Acidification
potential mol H+e 4.08E-02 4.36E-02 6.57E-02 3.16E-02 -8.47E-02
EP-freshwater kg Pe 1.31E-04 9.96E-04 2.10E-04 3.66E-04 -7.66E-04
EP-marine kg Ne 1.89E-02 1.43E-02 3.05E-02 1.20E-02 -1.83E-02
EP-terrestrial mol Ne 2.07E-01 1.56E-01 3.34E-01 1.31E-01 -2.39E-01
POCP (“smog”) kg NMVOCe 6.18E-02 6.43E-02 9.95E-02 4.71E-02 -6.14E-02
ADP-minerals &
metals kg Sbe 1.62E-06 3.57E-05 2.61E-06 7.07E-06 -1.30E-04
ADP-fossil
resources MJ 5.92E+01 1.86E+02 9.52E+01 1.09E+02 -1.92E+02
Water use m3e depr. 1.48E-01 9.17E-01 2.38E-01 3.15E-01 -2.56E+01
1) GWP = Global Warming Potential; 2) EP = Eutrophication potential. Required characterisation method and data are in kg P-eq. Multiply by 3,07 to
get PO4e; 3) POCP = Photochemical ozone formation; 4) ADP = Abiotic depletion potential; 5) EN 15804+A2 disclaimer for Abiotic depletion and
Water use and optional indicators except Particulate matter and Ionising radiation, human health. The results of these environmental impact indicators
shall be used with care as the uncertainties on these results are high or as there is limited experience with the indicator.
Additional environmental impact indicators – EN 15804+A2, EF 3.1
Impact category Unit A1 A2 A3 A1-A3
Particulate
matter Incidence 8.79E-06 4.69E-07 8.24E-07 1.01E-05
Ionising
radiation6 kBq U235e 3.59E-01 0.00E+00 7.11E-02 4.30E-01
Ecotoxicity
(freshwater) CTUe 1.88E+02 2.28E+01 1.08E+01 2.21E+02
Human toxicity,
cancer CTUh 2.39E-08 1.71E-09 4.22E-10 2.60E-08
Human tox.
non-cancer CTUh 6.52E-07 6.62E-08 2.85E-08 7.46E-07
SQP7 - 6.86E+02 1.98E+01 1.82E+01 7.24E+02

-- 14 of 20 --

Environmental Product Declaration
IN ACCORDANCE WITH EN 15804+A2 & ISO 14025
Boral | 15
Impact category Unit C1 C2 C3 C4 D
Particulate
matter Incidence 1.16E-06 1.28E-06 1.42E-05 7.18E-07 -1.09E-06
Ionising
radiation
kBq
U235e 2.62E-02 1.62E-01 4.22E-02 6.87E-02 -3.06E+00
Ecotoxicity
(freshwater) CTUe 3.26E+00 2.63E+01 5.24E+00 9.16E+00 -2.31E+02
Human toxicity,
cancer CTUh 4.65E-10 2.11E-09 7.49E-10 8.21E-10 -1.34E-08
Human tox.
non-cancer CTUh 7.36E-09 1.20E-07 1.19E-08 1.89E-08 -2.46E-07
SQP - 4.15E+00 1.87E+02 6.67E+00 2.15E+02 -1.85E+02
6) EN 15804+A2 disclaimer for Ionising radiation, human health. This impact category deals mainly with the eventual impact of low-dose ionising
radiation on human health of the nuclear fuel cycle. It does not consider effects due to possible nuclear accidents, occupational exposure nor due to
radioactive waste disposal in underground facilities. Potential ionising radiation from the soil, from radon and from some construction materials is also
not measured by this indicator; 7) SQP = Land use related impacts/soil quality.
Use of natural resources
Impact category Unit A1 A2 A3 A1-A3
Renew. PER
as energy8 MJ 7.86E+01 9.60E-01 6.39E-01 8.02E+01
Renew. PER as
material MJ 0.00E+00 0.00E+00 0.00E+00 0.00E+00
Total use of
renew. PER MJ 7.86E+01 9.60E-01 6.39E-01 8.02E+01
Non-re. PER
as energy MJ 1.11E+03 8.87E+01 6.88E+01 1.27E+03
Non-re. PER
as material MJ 1.06E+01 0.00E+00 -4.10E-01 1.02E+01
Total use of
non-re. PER MJ 1.12E+03 8.87E+01 6.84E+01 1.28E+03
Secondary
materials kg 7.76E-03 0.00E+00 0.00E+00 7.76E-03
Renew.
secondary fuels MJ 6.76E-06 0.00E+00 7.52E-05 8.19E-05
Non-ren.
secondary fuels MJ 0.00E+00 0.00E+00 0.00E+00 0.00E+00
Use of net fresh
water m3 3.79E+00 1.34E+00 6.99E-02 5.19E+00

-- 15 of 20 --

Environmental Product Declaration
IN ACCORDANCE WITH EN 15804+A2 & ISO 14025
Boral | 16
Impact category Unit C1 C2 C3 C4 D
Renew. PER
as energy MJ 3.75E-01 2.54E+00 6.03E-01 1.05E+00 -1.90E+01
Renew. PER as
material MJ 0.00E+00 0.00E+00 0.00E+00 0.00E+00 0.00E+00
Total use of
renew. PER MJ 3.75E-01 2.54E+00 6.03E-01 1.05E+00 -1.90E+01
Non-re. PER
as energy MJ 5.92E+01 1.86E+02 9.52E+01 1.09E+02 -1.98E+02
Non-re. PER
as material MJ 0.00E+00 0.00E+00 -7.17E+00 -3.07E+00 7.17E+00
Total use of non-
re. PER MJ 5.92E+01 1.86E+02 8.81E+01 1.06E+02 -1.91E+02
Secondary
materials kg 0.00E+00 0.00E+00 0.00E+00 0.00E+00 0.00E+00
Renew.
secondary fuels MJ 6.42E-05 1.00E-03 1.03E-04 5.69E-04 -1.54E-03
Non-ren.
secondary fuels MJ 0.00E+00 0.00E+00 0.00E+00 0.00E+00 0.00E+00
Use of net fresh
water m3 3.91E-03 2.74E-02 6.30E-03 1.14E-01 -5.95E-01
8) PER = Primary energy resources.
End of life – Waste
Impact category Unit A1 A2 A3 A1-A3
Hazardous waste kg 3.02E-02 1.17E-04 3.00E-02 6.03E-02
Non-hazardous
waste kg 5.26E+00 9.33E-01 7.83E-01 6.97E+00
Radioactive
waste kg 2.96E-04 5.39E-07 1.16E-05 3.08E-04
Impact category Unit C1 C2 C3 C4 D
Hazardous waste kg 6.59E-02 3.15E-01 1.06E-01 1.21E-01 -1.50E+00
Non-hazardous
waste kg 8.98E-01 5.82E+00 1.44E+00 2.76E+00 -2.78E+01
Radioactive
waste kg 6.43E-06 3.96E-05 1.04E-05 1.67E-05 -3.83E-04

-- 16 of 20 --

Environmental Product Declaration
IN ACCORDANCE WITH EN 15804+A2 & ISO 14025
Boral | 17
End of life – Output flows
Impact category Unit A1 A2 A3 A1-A3
Components for
re-use kg 0.00E+00 0.00E+00 0.00E+00 0.00E+00
Materials for
recycling kg 6.27E-06 0.00E+00 6.66E+01 6.66E+01
Materials for
energy recovery kg 0.00E+00 0.00E+00 0.00E+00 0.00E+00
Exported energy MJ 0.00E+00 0.00E+00 0.00E+00 0.00E+00
Exported energy
– Electricity MJ 0.00E+00 0.00E+00 0.00E+00 0.00E+00
Exported energy
– Heat MJ 0.00E+00 0.00E+00 0.00E+00 0.00E+00
Impact category Unit C1 C2 C3 C4 D
Components for
re-use kg 0.00E+00 0.00E+00 0.00E+00 0.00E+00 0.00E+00
Materials for
recycling kg 0.00E+00 0.00E+00 1.66E+03 0.00E+00 0.00E+00
Materials for
energy recovery kg 0.00E+00 0.00E+00 0.00E+00 0.00E+00 0.00E+00
Exported energy MJ 0.00E+00 0.00E+00 0.00E+00 0.00E+00 0.00E+00
Exported energy
– Electricity MJ 0.00E+00 0.00E+00 0.00E+00 0.00E+00 0.00E+00
Exported energy
– Heat MJ 0.00E+00 0.00E+00 0.00E+00 0.00E+00 0.00E+00
Environmental impacts – EN 15804+A1, CML / ISO 21930
Impact category Unit A1 A2 A3 A1-A3
Global Warming
Pot.
kg
CO2e 2.56E+02 6.56E+00 5.58E+00 2.68E+02
Ozone depletion
Pot.
kg
CFC-11e 1.56E-06 8.57E-07 4.19E-08 2.46E-06
Acidification kg
SO2e 1.23E+00 2.04E-02 2.98E-02 1.28E+00
Eutrophication kg
PO43e 3.03E-01 4.36E-03 5.44E-03 3.13E-01
POCP (“smog”) kg
C2H4e 4.41E-02 8.19E-04 1.48E-03 4.64E-02
ADP-elements kg Sbe 1.96E-06 1.44E-05 2.05E-06 1.84E-05
ADP-fossil MJ 1.72E+02 8.87E+01 6.80E+01 3.28E+02

-- 17 of 20 --

Environmental Product Declaration
IN ACCORDANCE WITH EN 15804+A2 & ISO 14025
Boral | 18
Impact category Unit C1 C2 C3 C4 D
Global Warming
Pot.
kg
CO2e 4.50E+00 1.27E+01 7.24E+00 4.41E+00 -1.60E+01
Ozone depletion
Pot.
kg
CFC-11e 5.49E-08 1.51E-07 8.83E-08 1.02E-07 -1.10E-07
Acidification kg
SO2e 2.87E-02 3.33E-02 4.62E-02 2.34E-02 -7.69E-02
Eutrophication kg
PO43e 6.71E-03 8.12E-03 1.08E-02 7.42E-03 -1.51E-02
POCP (“smog”) kg
C2H4e 2.15E-03 2.97E-03 3.46E-03 2.21E-03 -6.85E-03
ADP-elements kg Sbe 1.58E-06 3.48E-05 2.54E-06 6.93E-06 -8.78E-05
ADP-fossil MJ 5.87E+01 1.83E+02 9.46E+01 1.08E+02 -1.98E+02
Additional indicator – GWP-GHG
Impact category Unit A1 A2 A3 A1-A3
GWP-GHG9 kg
CO2e 2.56E+02 6.57E+00 5.62E+00 2.68E+02
Impact category Unit C1 C2 C3 C4 D
GWP-GHG kg
CO2e 4.52E+00 1.28E+01 7.28E+00 4.45E+00 -1.29E+01
9) This indicator includes all greenhouse gases excluding biogenic carbon dioxide uptake and emissions and biogenic carbon stored in the product.
In addition, the characterisation factors for the flows – CH4 fossil, CH4 biogenic and Dinitrogen monoxide – were updated. This indicator is identical
to the GWP-total of EN 15804:2012+A2:2019 except that the characterisation factor for biogenic CO2 is set to zero.

-- 18 of 20 --

Environmental Product Declaration
IN ACCORDANCE WITH EN 15804+A2 & ISO 14025
Boral | 19
Scenario documentation
Manufacturing energy scenario documentation
Manufacturing energy scenario documentation – A3 (Energy data source)
1. Construction, specialized activities, demolition and site preparation, Market for diesel, burned in building machine,
World, ecoinvent 3.10.1, 0.10 kgCO2e/MJ
2. Electricity, Electricity, consumption mix w/o renewables, Victoria, 2024, Australia, LCA study for country specific
consumption mixes, OneClickLCA 2025, 1.14 kgCO2e/kWh
Electricity data source: Australian Energy Update 2024, published by the Department of Climate Change, Energy, the
Environment and Water (DCCEEW)
End of life scenario documentation
Collection process – kg collected separately 0
Collection process – kg collected with mixed
construction waste 2377
Recovery process – kg for re-use 0
Recovery process – kg for recycling 1.66E+03
Recovery process – kg for energy recovery 0
Disposal (total) – kg for final deposition 7.13E+02
Scenario assumptions e.g. transportation Market for transport, freight, lorry >32 metric ton,
EURO5; 50km

-- 19 of 20 --

Environmental Product Declaration
IN ACCORDANCE WITH EN 15804+A2 & ISO 14025
Boral | 20
Third-party verification statement
EPD Hub declares that this EPD is verified in accordance with ISO 14025 by an independent, third-party verifier. The
project report on the Life Cycle Assessment and the report(s) on features of environmental relevance are filed at EPD
Hub. EPD Hub PCR and ECO Platform verification checklist are used.
EPD Hub is not able to identify any unjustified deviations from the PCR and EN 15804+A2 in the Environmental
Product Declaration and its project report.
EPD Hub maintains its independence as a third-party body; it was not involved in the execution of the LCA or in the
development of the declaration and has no conflicts of interest regarding this verification.
The company-specific data and upstream and downstream data have been examined as regards plausibility and
consistency. The publisher is responsible for ensuring the factual integrity and legal compliance of this declaration.
Verified tools
Tool verifier: Imane Uald Lamkaddam
Tool verification validity: 28 March 2025 - 27 March 2028
Xinyuan Zhang
Program assistant
The software used in creation of this LCA and EPD is verified by EPD Hub to conform to the procedural and methodological
requirements outlined in ISO 14025:2010, ISO 14040/14044, EN 15804+A2, and EPD Hub Core Product Category Rules
and General Program Instructions.

-- 20 of 20 --

