1	Created with One Click LCA N50/20 Xencrete
ENVIRONMENTAL PRODUCT DECLARATION
IN ACCORDANCE WITH EN 15804+A2 & ISO 14025
EPD HUB, HUB-5943
Published on 09.04.2026, last updated on 09.04.2026, valid until 08.04.2031
This EPD is intended for business-to-business and/or business-to-consumer communication. Life Cycle Assessment study has been performed in accordance with the
requirements of EN 15804, EPD Hub PCR version 1.2 (24 Mar 2025) and JRC characterization factors EF 3.1. The manufacturer has the sole ownership, liability, and responsibility
for the EPD. EPDs within the same product category but from different programs may not be comparable. EPDs of construction products may not be comparable if they do not
comply with EN 15804 and if they are not compared in a building context.
N50/20 Xencrete
Entire Concrete

-- 1 of 13 --

2	Created with One Click LCA N50/20 Xencrete
MANUFACTURER AND SITE
Manufacturer Entire Concrete
Address 65 STENHOUSE DRIVE, Cameron Park New
South Wales 2285
Contact details adam@entireconcrete.com.au
Website https://www.entireconcrete.com.au
Place of production Hunter Valley, NSW, Australia
Place(s) of raw
material origin
Hunter Valley, NSW, Australia
Place(s) of
installation and use
Hunter Valley, NSW, Australia
Period for data 1st Jan 2024 to 31st Dec 2024
EPD STANDARDS, SCOPE AND VERIFICATION
Program operator EPD Hub, hub@epdhub.com
Reference standard EN 15804:2012+A2:2019/AC:2021
and ISO 14025
PCR EPD Hub Core PCR version 1.2, 24 Mar 2025
cPCR EN 16757 Product Category Rules for
concrete and concrete elements
Sector Construction product
Category of EPD Third party verified EPD
Parent EPD number -
Scope of the EPD Cradle to gate with options, A4-A5, and
modules C1-C4, D
EPD author Jason Chandler, EPD on Demand
EPD verification Independent verification of this EPD and
data, according to ISO 14025:
 Internal verification
 External verification
EPD verifier Vera Durão, as an authorised verifier acting
for EPD Hub Limited
PRODUCT SPECIFICATION
Product name N50/20 Xencrete
Product reference -
Concrete type Ready-mix concrete
Product standards AS 1379-2007
Additional
characteristic -
GTIN (Global Trade Item
Number) -
NOBB (Norwegian
Building Product Database) -
A1-A3 Specific data
(%) 2.7
PRODUCT DESCRIPTION
This ready-mixed concrete product is produced in
accordance with AS1379:2007(2017) Specification and
supply of concrete. The raw materials are proportioned
so as to achieve a characteristic strength of 50MPa in
accordance with the requirements of clause 6 of that
Standard. The nominal maximum aggregate size is
20mm and the nominal consistence is 80mm slump
when measured in accordance AS1012.3.1
Determination of properties related to the consistency
of concrete - Slump test.
Application: General use concrete
PRODUCT CHARACTERISTICS
Compressive strength class:
N50
Strength evaluation days:
28 days
Exposure class:
C1
ENVIRONMENTAL DATA SUMMARY
Declared unit 1 cubic meter
Declared unit mass, kg 2272
GWP-total, A1-A3 (kg CO₂e) 310
GWP-fossil, A1-A3 (kg CO₂e) 309
Secondary material, inputs (%) 5.92
Secondary material, outputs (%) 70
Total energy use, A1-A3 (kWh) 580
Net freshwater use, A1-A3 (m3) 5.67E‐01

-- 2 of 13 --

3	Created with One Click LCA N50/20 Xencrete
WHO WE ARE
As the region’s leading independent supplier of
concrete Entire Concrete offers fast, quality assured
ready-mix concrete for projects of all sizes throughout
Newcastle, Singleton and the Hunter Valley. Beginning
in 2008, Entire Concrete has rapidly grown to become
the leading independent supplier of quality premixed
concrete products in the Greater Hunter region.
At Entire Concrete, we pride ourselves on offering
specialised concrete solutions tailored to your needs.
From residential to commercial and industrial-scale
projects, Entire Concrete has developed a reputation
for quality, safety and efficiency when it comes to our
products and our service. With a modern agitator fleet,
housing 37 trucks, from 10-wheeled concrete trucks to
smaller mini trucks, Entire Concrete is capable of
servicing projects of all sizes.
Our experienced batching team works directly with
customers to get projects completed, often exceeding
customer expectations by providing a superior result
from project start through to completion.
As a part of our continued growth within the ready-mix
sector, Entire Concrete has two industry leading
concrete plants in Cameron Park and Singleton. From
these plants, we deliver our quality product throughout
Newcastle and the Hunter Valley.
OUR COMMITMENT TO THE ENVIRONMENT
Entire Concrete is committed to implementing best
practice environmental measures. At its inception,
Entire Concrete began with the focus on local people,
products and community’s needs.
We believe it is a requirement that we actively
contribute to the local community, and as such, Entire
Concrete, the home of the green trucks, decided to go
green in 2010.
Our strategy included;
• Moving toward long term sustainability with a
view to become increasingly self-sufficient
over time.
• Installation of a concrete recycler. Installing a
concrete recycler reduces waste, eliminates
the need for excess landfill and potential soil
contaminants.
• Recycle the raw materials utilised in the
manufacturing of concrete, including
aggregates (rocks) sands, and cementitious
materials (i.e. cement powder and flash).
• Reducing Entire Concrete’s reliance on our
natural environment by harvesting the
rainwater that falls on site. Entire currently
harvests approximately 450,000 litres of
water.
• Installing a solar electricity system through
Metro Solar, an Australian-based engineering
firm who offered the new and innovative
microinverter technology.
Today, the power generated through the use of solar
technology is sufficient to power the company’s on-site
concrete recycler and water reticulation programs,
another step in the road towards onsite self-
sufficiency.
More recently we have begun incorporating the CEMI
additive to our Xencrete range of lower carbon
concretes to enable a greater use of flyash in our
concrete, continuing to lead the way in sustainability
and technical excellence.

-- 3 of 13 --

4	Created with One Click LCA N50/20 Xencrete
LIFE CYCLE ASSESSMENT
SYSTEM BOUNDARY
This EPD covers the life-cycle modules listed in the
following table.
Product stage
Assembly stage
Use stage
End of life stage
Beyond the system
boundaries
A1 A2 A3 A4 A5 B1 B2 B3 B4 B5 B6 B7 C1 C2 C3 C4 D
x x x x x N
D
N
D
N
D
N
D
N
D
N
D
N
D x x x x x
Raw materials	
Transport	
Manufacturing	
Transport	
Assembly	
Use
Maintenance	
Repair
Replacement	
Refurbishment	
Operational energy	
use	
Operational water	
use	
Deconstr./demol.	
Transport	
Waste processing	
Disposal
Reuse, Recovery,	
Recycling
Not declared = ND.
CUT-OFF CRITERIA
The study does not exclude any modules or processes
which are stated mandatory in the reference standard
and the applied PCR. The study does not exclude any
hazardous materials or substances. There is no
neglected unit process more than 1% of total mass or
energy flows. The module specific total neglected input
and output flows also do not exceed 5% of energy
usage or mass.
The production of capital equipment, construction
activities, and infrastructure, maintenance and
operation of capital equipment, personnel-related
activities, energy and water use related to company
management and sales activities are excluded.
VALIDATION OF DATA
Data collection for production, transport, and packaging
was conducted using time and site-specific information,
as defined in the general information section on page 1
and 2. Upstream process calculations rely on generic
data as defined in the Bibliography section.
Manufacturer-provided specific and generic data were
used for the product’s manufacturing stage. The
analysis was performed in One Click LCA EPD
Generator, with the 'Cut-Off, EN 15804+A2' allocation
method, and characterization factors according to EN
15804:2012+A2:2019/AC:2021 and JRC EF 3.1.
ALLOCATION, ESTIMATES AND ASSUMPTIONS
All allocations are done as per the reference standards
and the applied PCR. In this study, allocation has been
done in the following ways:
Data type Allocation
Raw materials No allocation
Packaging materials Not applicable
Ancillary materials Allocated by mass
Manufacturing energy and waste Allocated by mass
• Flyash primary supplier data has been used (EPD
#HUB-3862)
• Fuel used for mixing 1m3 of concrete was
conservatively determined based on a 10-minute
mixing time of the average load size of 5m3, for diesel
burned in the full mixing mode of the concrete agitator
barrel
• A market-based approach is used in modelling the
electricity mix utilised in the factory. Renewables have
been removed to provide a conservative approach,
with such electricity being less than 0.3% of the total
impact; this would have very little impact on the results
• Distribution Loss Factor (DLF) of 1.042 was applied to
the electricity
• Electricity is composed of 94.40% Coal, 4.38% Gas
and 1.23% Oil and contributes 1.6kg CO2e to the A1-A3
GWP Total value
• Transport factors for raw materials, Aggregates 29-
124km, Admixtures 137-206km, Cement 33-8367km
• A4, Distance of 11.9km is assumed
• A5, 3% waste, and 73.62MJ of diesel consumed
PRODUCT & MANUFACTURING SITES GROUPING
Type of grouping Multiple factories
Grouping method Based on average results of product group -
by total volume
Variation in GWP-
fossil for A1-A3, % -0.6% / +0.6%
This Environmental Product Declaration represents the
average of multiple manufacturing sites. The declared
results are based on production‑weighted data from
the reference year, reflecting the actual output of each
plant. All included plants use comparable raw
materials, mix designs, energy sources, and production
technologies relevant to the declared concrete
product.
The included facilities are: Cameron Park and
Singleton.

-- 4 of 13 --

5	Created with One Click LCA N50/20 Xencrete
The averaged dataset is considered representative of
typical production for these products within the
organisation. Variations between plants were assessed
and determined not to materially affect the
environmental profile of the declared product. Where
differences existed (e.g., energy mix, transport
distances), these were incorporated into the
production‑weighted average in accordance with EN
15804+A2 and ISO 14025. The declared results reflect
the average performance of these sites and are
representative of the company’s overall production for
this product.
PRODUCT RAW MATERIAL MAIN COMPOSITION
The product is a ready-mix concrete consisting of
aggregates, cement, filler, admixtures, and water. Main
material categories as per EPD Hub GPI are shown
below:
Raw material
category
Amount, mass- % Material origin
Metals 0
Minerals 100 Australia and Global
Fossil materials 0
Bio-based materials 0
SUBSTANCES, REACH - VERY HIGH CONCERN
The product does not contain any REACH SVHC
substances in amounts greater than 0,1 % (1000 ppm).
BIOGENIC CARBON CONTENT
Product’s biogenic carbon content at the factory gate
Biogenic carbon content in product, kg C 0
PRODUCT LIFE CYCLE
MANUFACTURING (A1-A3)
The environmental impacts considered for the product
stage cover the manufacturing of raw materials used in
the production. Also, fuels used by machines, and
handling of waste formed in the production processes
at the manufacturing facilities are included in this
stage. The study also considers the material losses
occurring during the manufacturing processes as well
as losses during electricity transmission.
Ready-mix concrete production starts by transporting
the binders, aggregates, and additives to the
manufacturing site and storing them into closed silos
and containers. The aggregates are then dosed onto a
scale and transferred to a concrete mixer. All
manufacturing sites covered by this document are ‘dry
batch’ sites whereby the mixer is also the agitator
barrel of the concrete truck. In the mixer, cement is
added to the aggregates, after which the material is
mixed dry. Water and additives are then added to the
mixture, followed by further mixing. After mixing, the
concrete mass is contained in the barrel of the
concrete mixer truck, in which it is transported to the
construction site.
No packaging is included as the product is transported
with mixer trucks.
TRANSPORT AND INSTALLATION (A4-A5)
The concrete is transported to the building site using
an average truck. Transportation impacts occurred
from final products delivery to construction site cover
fuel direct exhaust emissions, environmental impacts
of fuel production, as well as related infrastructure
emissions (A4).
Installation includes the energy used for concrete
application. This consists of the energy spent by a
concrete mixer truck and a concrete pump. A
production loss of % at installation is
assumed (A5).
PRODUCT USE AND MAINTENANCE (B1-B7)
This EPD does not cover the use phase. Air, soil, and
water impacts during the use phase have not been
studied. Carbonation is not taken into account in this
EPD.
3

-- 5 of 13 --

6	Created with One Click LCA N50/20 Xencrete
PRODUCT END OF LIFE (C1-C4, D)
At the end of its life, the concrete is assumed to be part
of a concrete building that is demolished using
machinery, consuming energy in the form of diesel
(C1).
The concrete blocks gotten after the demolition are
delivered 50 km by a truck to the nearest construction
waste treatment (C2). It is assumed that 100% of the
demolished concrete is transported to a site where this
waste is processed by, crushing the blocks to gravel.
About 70% of concrete can be recycled this way (C3),
with an assumption that non-reinforced concrete is
being sorted. The remaining 30% of concrete is
assumed to be sent to the landfill for disposal (C4). The
crushed concrete received from waste treatment can
be used as a replacement for virgin gravel or for raw
materials in road construction (D). The process losses
of the waste treatment plant are assumed to be
negligible.
LCA SOFTWARE AND BIBLIOGRAPHY
This EPD has been created using One Click LCA
Concrete EPD Generator v3.2.3. The LCA and EPD have
been prepared according to the reference standards
and ISO 14040/14044. Ecoinvent v3.10.1/3.11/3.12 and
One Click LCA databases were used as sources of
environmental data. Allocation used in Ecoinvent
3.10.1/3.11/3.12 environmental data sources follow
the methodology ‘allocation, cut-off, EN 15804+A2‘.
AS 1379 2007 - Specification and supply of concrete
AS 3600 2018 - Concrete Structures, Table 4.4
Australian energy statistics 2025 - Table O, Australian
electricity generation, by state and territory, by fuel
type, physical units.
https://www.energy.gov.au/publications/australian-
energy-update-2025
Australian Energy Market Operator - Distribution Loss
Factors For The 2024/25 Financial Year.
https://www.aemo.com.au/-
/media/files/electricity/nem/security_and_reliability/lo
ss_factors_and_regional_boundaries/2024-25-
financial-year/distribution-loss-factors-for-2024-25.pdf
Diesel used in the mixing of concrete. https://unique-
mixer.com/news/How_much_diesel_does_a_self_loadi
ng_concrete_mixer_consume_per_hour.html

-- 6 of 13 --

7	Created with One Click LCA N50/20 Xencrete
SYSTEM DIAGRAM

-- 7 of 13 --

8 N50/20 Xencrete	Created with One Click LCA
ENVIRONMENTAL IMPACT DATA
The estimated impact results are only relative statements which do not indicate the end points of the impact categories, exceeding threshold values, safety margins or risks.
CORE ENVIRONMENTAL IMPACT INDICATORS – EN 15804+A2, EF 3.1
Impact category Unit A1 A2 A3 A1-A3 A4 A5 B1 B2 B3 B4 B5 B6 B7 C1 C2 C3 C4 D
GWP – total1) kg CO2e 2.70E+02 3.61E+01 3.65E+00 3.10E+02 2.91E+00 1.75E+01 ND ND ND ND ND ND ND 4.32E+00 1.22E+01 6.96E+00 4.26E+00 ‐1.17E+01
GWP – fossil kg CO2e 2.70E+02 3.61E+01 3.65E+00 3.09E+02 2.91E+00 1.74E+01 ND ND ND ND ND ND ND 4.32E+00 1.22E+01 6.96E+00 4.25E+00 ‐1.17E+01
GWP – biogenic kg CO2e 1.03E‐01 7.43E‐03 6.12E‐04 1.11E‐01 6.59E‐04 4.13E‐03 ND ND ND ND ND ND ND 4.41E‐04 2.77E‐03 ‐7.10E‐04 ‐1.35E‐03 ‐3.67E‐02
GWP – LULUC kg CO2e 4.12E‐02 1.98E‐02 2.95E‐04 6.13E‐02 1.30E‐03 2.89E‐03 ND ND ND ND ND ND ND 4.43E‐04 5.47E‐03 7.13E‐04 2.43E‐03 ‐1.62E‐02
Ozone depletion pot. kg CFC-11e 1.32E‐06 5.24E‐07 3.88E‐08 1.88E‐06 4.30E‐08 1.83E‐07 ND ND ND ND ND ND ND 6.62E‐08 1.81E‐07 1.07E‐07 1.23E‐07 ‐9.80E‐07
Acidification potential mol H+e 1.46E+00 5.04E‐01 2.74E‐02 2.00E+00 9.92E‐03 1.31E‐01 ND ND ND ND ND ND ND 3.90E‐02 4.17E‐02 6.28E‐02 3.02E‐02 ‐7.64E‐02
EP-freshwater2) kg Pe 1.29E‐02 2.13E‐03 4.12E‐04 1.55E‐02 2.27E‐04 7.29E‐04 ND ND ND ND ND ND ND 1.25E‐04 9.52E‐04 2.01E‐04 3.50E‐04 ‐6.91E‐04
EP-marine kg Ne 1.24E‐01 1.22E‐01 9.06E‐03 2.55E‐01 3.26E‐03 4.02E‐02 ND ND ND ND ND ND ND 1.81E‐02 1.37E‐02 2.91E‐02 1.15E‐02 ‐1.65E‐02
EP-terrestrial mol Ne 4.91E+00 1.35E+00 9.80E‐02 6.36E+00 3.55E‐02 5.48E‐01 ND ND ND ND ND ND ND 1.98E‐01 1.49E‐01 3.19E‐01 1.26E‐01 ‐2.16E‐01
POCP (“smog”)3) kg
NMVOCe 1.23E+00 4.07E‐01 2.94E‐02 1.66E+00 1.46E‐02 1.57E‐01 ND ND ND ND ND ND ND 5.91E‐02 6.15E‐02 9.51E‐02 4.50E‐02 ‐5.54E‐02
ADP-minerals & metals4) kg Sbe 1.15E‐03 7.38E‐05 1.15E‐06 1.23E‐03 8.12E‐06 4.10E‐05 ND ND ND ND ND ND ND 1.55E‐06 3.41E‐05 2.50E‐06 6.76E‐06 ‐1.17E‐04
ADP-fossil resources MJ 1.43E+03 4.85E+02 4.51E+01 1.96E+03 4.22E+01 1.68E+02 ND ND ND ND ND ND ND 5.65E+01 1.77E+02 9.10E+01 1.04E+02 ‐1.74E+02
Water use5) m3e depr. 3.63E+01 2.05E+00 1.51E+01 5.34E+01 2.09E‐01 1.89E+00 ND ND ND ND ND ND ND 1.41E‐01 8.76E‐01 2.27E‐01 3.01E‐01 ‐2.31E+01
1) GWP = Global Warming Potential. 2) EP = Eutrophication potential. Required characterisation method and data are in kg P-eq. Multiply by 3,07 to get PO4e. 3) POCP = Photochemical ozone formation. 4) ADP = Abiotic depletion potential.
5) EN 15804+A2 disclaimer for Abiotic depletion and Water use and optional indicators except Particulate matter and Ionizing radiation, human health. The results of these environmental impact indicators shall be used with care as the
uncertainties on these results are high or as there is limited experience with the indicator.
removalMarker-pef1

-- 8 of 13 --

9 N50/20 Xencrete	Created with One Click LCA
ADDITIONAL (OPTIONAL) ENVIRONMENTAL IMPACT INDICATORS – EN 15804+A2, EF 3.1
Impact category Unit A1 A2 A3 A1-A3 A4 A5 B1 B2 B3 B4 B5 B6 B7 C1 C2 C3 C4 D
Particulate matter Incidence 1.42E‐05 2.43E‐06 6.32E‐07 1.73E‐05 2.91E‐07 2.88E‐06 ND ND ND ND ND ND ND 1.11E‐06 1.22E‐06 1.36E‐05 6.87E‐07 ‐9.80E‐07
Ionizing radiation6) kBq
U235e 1.58E+03 3.54E‐01 3.57E‐02 1.58E+03 3.68E‐02 4.75E+01 ND ND ND ND ND ND ND 2.50E‐02 1.55E‐01 4.03E‐02 6.56E‐02 ‐2.76E+00
Ecotoxicity (freshwater) CTUe 3.46E+02 5.61E+01 1.69E+01 4.19E+02 5.97E+00 1.92E+01 ND ND ND ND ND ND ND 3.11E+00 2.51E+01 5.01E+00 8.76E+00 ‐2.08E+02
Human toxicity. cancer CTUh 3.64E‐07 6.96E‐09 3.05E‐10 3.71E‐07 4.80E‐10 1.20E‐08 ND ND ND ND ND ND ND 4.44E‐10 2.02E‐09 7.16E‐10 7.84E‐10 ‐1.21E‐08
Human tox. non-cancer CTUh 1.27E‐05 2.35E‐07 1.32E‐08 1.29E‐05 2.73E‐08 4.04E‐07 ND ND ND ND ND ND ND 7.04E‐09 1.15E‐07 1.13E‐08 1.80E‐08 ‐2.22E‐07
SQP7) - 1.61E+03 3.00E+02 6.48E+00 1.91E+03 4.25E+01 7.71E+01 ND ND ND ND ND ND ND 3.96E+00 1.79E+02 6.38E+00 2.06E+02 ‐1.67E+02
6) EN 15804+A2 disclaimer for Ionizing radiation. human health. This impact category deals mainly with the eventual impact of low dose ionizing radiation on human health of the nuclear fuel cycle. It does not consider effects due to
possible nuclear accidents. occupational exposure nor due to radioactive waste disposal in underground facilities. Potential ionizing radiation from the soil. from radon and from some construction materials is also not measured by this
indicator. 7) SQP = Land use related impacts/soil quality. removalMarker-pef2
USE OF NATURAL RESOURCES
Impact category Unit A1 A2 A3 A1-A3 A4 A5 B1 B2 B3 B4 B5 B6 B7 C1 C2 C3 C4 D
Renew. PER as energy8) MJ 5.41E+01 5.72E+00 3.60E‐01 6.02E+01 5.79E‐01 2.55E+00 ND ND ND ND ND ND ND 3.58E‐01 2.43E+00 5.77E‐01 1.01E+00 ‐1.72E+01
Renew. PER as material MJ 0.00E+00 0.00E+00 0.00E+00 0.00E+00 0.00E+00 0.00E+00 ND ND ND ND ND ND ND 0.00E+00 0.00E+00 0.00E+00 0.00E+00 0.00E+00
Total use of renew. PER MJ 5.41E+01 5.72E+00 3.60E‐01 6.02E+01 5.79E‐01 2.55E+00 ND ND ND ND ND ND ND 3.58E‐01 2.43E+00 5.77E‐01 1.01E+00 ‐1.72E+01
Non-re. PER as energy MJ 1.45E+03 4.85E+02 4.54E+01 1.99E+03 4.22E+01 1.68E+02 ND ND ND ND ND ND ND 5.65E+01 1.77E+02 9.10E+01 1.04E+02 ‐1.78E+02
Non-re. PER as material MJ 0.00E+00 0.00E+00 0.00E+00 0.00E+00 0.00E+00 0.00E+00 ND ND ND ND ND ND ND 0.00E+00 0.00E+00 0.00E+00 0.00E+00 0.00E+00
Total use of non-re. PER MJ 1.45E+03 4.85E+02 4.54E+01 1.99E+03 4.22E+01 1.68E+02 ND ND ND ND ND ND ND 5.65E+01 1.77E+02 9.10E+01 1.04E+02 ‐1.78E+02
Secondary materials kg 1.35E+02 0.00E+00 0.00E+00 1.35E+02 0.00E+00 0.00E+00 ND ND ND ND ND ND ND 0.00E+00 0.00E+00 0.00E+00 0.00E+00 0.00E+00
Renew. secondary fuels MJ 4.01E+01 1.76E‐03 4.28E‐05 4.01E+01 2.28E‐04 1.20E+00 ND ND ND ND ND ND ND 6.14E‐05 9.59E‐04 9.88E‐05 5.43E‐04 ‐1.39E‐03
Non-ren. secondary
fuels MJ 1.29E+00 0.00E+00 0.00E+00 1.29E+00 0.00E+00 3.87E‐02 ND ND ND ND ND ND ND 0.00E+00 0.00E+00 0.00E+00 0.00E+00 0.00E+00
Use of net fresh water m3 4.80E‐01 5.74E‐02 2.89E‐02 5.67E‐01 6.24E‐03 2.78E‐02 ND ND ND ND ND ND ND 3.74E‐03 2.62E‐02 6.02E‐03 1.09E‐01 ‐5.37E‐01
8) PER = Primary energy resources.

-- 9 of 13 --

10 N50/20 Xencrete	Created with One Click LCA
END OF LIFE – WASTE
Impact category Unit A1 A2 A3 A1-A3 A4 A5 B1 B2 B3 B4 B5 B6 B7 C1 C2 C3 C4 D
Hazardous waste kg 2.33E‐01 7.96E‐01 3.13E‐02 1.06E+00 7.15E‐02 1.57E‐01 ND ND ND ND ND ND ND 6.29E‐02 3.01E‐01 1.01E‐01 1.15E‐01 ‐1.35E+00
Non-hazardous waste kg 4.60E+00 1.31E+01 5.88E‐01 1.83E+01 1.32E+00 2.34E+00 ND ND ND ND ND ND ND 8.58E‐01 5.56E+00 1.38E+00 2.64E+00 ‐2.50E+01
Radioactive waste kg 4.21E‐04 8.66E‐05 6.39E‐06 5.14E‐04 9.00E‐06 2.81E‐05 ND ND ND ND ND ND ND 6.15E‐06 3.78E‐05 9.89E‐06 1.60E‐05 ‐3.45E‐04
END OF LIFE – OUTPUT FLOWS
Impact category Unit A1 A2 A3 A1-A3 A4 A5 B1 B2 B3 B4 B5 B6 B7 C1 C2 C3 C4 D
Components for re-use kg 0.00E+00 0.00E+00 0.00E+00 0.00E+00 0.00E+00 0.00E+00 ND ND ND ND ND ND ND 0.00E+00 0.00E+00 0.00E+00 0.00E+00 0.00E+00
Materials for recycling kg 1.92E‐11 0.00E+00 1.81E+01 1.81E+01 0.00E+00 4.83E+01 ND ND ND ND ND ND ND 0.00E+00 0.00E+00 1.59E+03 0.00E+00 0.00E+00
Materials for energy rec Kg 1.01E‐19 0.00E+00 0.00E+00 1.01E‐19 0.00E+00 3.02E‐21 ND ND ND ND ND ND ND 0.00E+00 0.00E+00 0.00E+00 0.00E+00 0.00E+00
Exported energy MJ 0.00E+00 0.00E+00 0.00E+00 0.00E+00 0.00E+00 0.00E+00 ND ND ND ND ND ND ND 0.00E+00 0.00E+00 0.00E+00 0.00E+00 0.00E+00
Exported energy:
Electricity MJ 0.00E+00 0.00E+00 0.00E+00 0.00E+00 0.00E+00 0.00E+00 ND ND ND ND ND ND ND 0.00E+00 0.00E+00 0.00E+00 0.00E+00 0.00E+00
Exported energy: Heat MJ 0.00E+00 0.00E+00 0.00E+00 0.00E+00 0.00E+00 0.00E+00 ND ND ND ND ND ND ND 0.00E+00 0.00E+00 0.00E+00 0.00E+00 0.00E+00
ENVIRONMENTAL IMPACTS – EN 15804+A1. CML
Impact category Unit A1 A2 A3 A1-A3 A4 A5 B1 B2 B3 B4 B5 B6 B7 C1 C2 C3 C4 D
Global Warming Pot. kg CO2e 2.70E+02 3.59E+01 3.63E+00 3.09E+02 2.89E+00 1.74E+01 ND ND ND ND ND ND ND 4.30E+00 1.22E+01 6.92E+00 4.22E+00 ‐1.45E+01
Ozone depletion Pot. kg CFC-11e 6.49E‐06 4.17E‐07 3.17E‐08 6.94E‐06 3.43E‐08 3.08E‐07 ND ND ND ND ND ND ND 5.24E‐08 1.44E‐07 8.44E‐08 9.79E‐08 ‐9.97E‐08
Acidification kg SO2e 6.10E‐01 4.04E‐01 2.10E‐02 1.04E+00 7.58E‐03 8.10E‐02 ND ND ND ND ND ND ND 2.74E‐02 3.18E‐02 4.42E‐02 2.23E‐02 ‐6.94E‐02
Eutrophication kg PO43e 1.56E‐01 4.81E‐02 4.30E‐03 2.08E‐01 1.85E‐03 1.80E‐02 ND ND ND ND ND ND ND 6.41E‐03 7.76E‐03 1.03E‐02 7.10E‐03 ‐1.36E‐02
POCP (“smog”) kg C2H4e 2.66E‐02 2.20E‐02 1.27E‐03 4.98E‐02 6.75E‐04 5.27E‐03 ND ND ND ND ND ND ND 2.06E‐03 2.84E‐03 3.31E‐03 2.11E‐03 ‐6.18E‐03
ADP-elements kg Sbe 1.15E‐03 7.22E‐05 1.12E‐06 1.22E‐03 7.92E‐06 4.07E‐05 ND ND ND ND ND ND ND 1.51E‐06 3.33E‐05 2.43E‐06 6.63E‐06 ‐7.92E‐05
ADP-fossil MJ 1.43E+03 4.80E+02 4.49E+01 1.96E+03 4.17E+01 1.67E+02 ND ND ND ND ND ND ND 5.61E+01 1.75E+02 9.04E+01 1.03E+02 ‐1.78E+02

-- 10 of 13 --

11 N50/20 Xencrete	Created with One Click LCA
ADDITIONAL INDICATOR – GWP-GHG
Impact category Unit A1 A2 A3 A1-A3 A4 A5 B1 B2 B3 B4 B5 B6 B7 C1 C2 C3 C4 D
GWP-GHG 9) kg CO2e 2.70E+02 3.61E+01 3.65E+00 3.09E+02 2.91E+00 1.74E+01 ND ND ND ND ND ND ND 4.32E+00 1.22E+01 6.96E+00 4.26E+00 ‐1.17E+01
9) This indicator includes all greenhouse gases excluding biogenic carbon dioxide uptake and emissions and biogenic carbon stored in the product. In addition. the characterisation factors for the flows - CH4 fossil. CH4 biogenic and Dinitrogen
monoxide - were updated. This indicator is identical to the GWP-total of EN 15804:2012+A2:2019 except that the characterization factor for biogenic CO2 is set to zero.

-- 11 of 13 --

12	Created with One Click LCA N20/20 Xencrete
SCENARIO DOCUMENTATION
DATA SOURCES
Manufacturing energy scenario documentation – A3 (Energy data source)
1. Construction, specialized activities, demolition and site preparation, Diesel. burned in building machine,
World, ecoinvent 3.11, 0.10 kgCO2e/MJ
2. Electricity, Electricity, consumption mix w/o renewables, New South Wales, 2024, Australia, LCA study
for country specific consumption mixes, OneClickLCA 2025, 1.14 kgCO2e/kWh
Installation scenario documentation - A5 (Diesel consumption)
1. Diesel, burned in building machine, World, ecoinvent 3.10.1, 0.1 kg CO2e/MJ
TRANSPORT SCENARIO DOCUMENTATION - A4
Scenario parameter Value
Vehicle type used for transport (e.g., long distance
truck, boat, etc.) / Vehicle type. Commission
Directive 2007/37/EC (European Emission Standard)
Concrete mixer truck
Distance, km 11.9
Capacity utilization (including empty return) % 50 %
Bulk density of transported products / kg/m3 2272
Volume capacity utilization factor (factor: =1 or <1 or
≥1 for compressed or nested packaged products) 1
INSTALLATION SCENARIO DOCUMENTATION - A5
Scenario parameter Value
Ancillary materials for installation (specified by
material) / kg or other units as appropriate 0
Water use / m³ 0
Other resource use / kg 0
Waste materials on the building site before waste
processing. generated by the product's installation
(specified by type) / kg
6.82E+01
Output materials as result of waste processing at the
building site e.g. collection for recycling / kg 4.77E+01
Output materials as result of waste processing at the
building site e.g. collection for disposal / kg 2.04E+01
Direct emissions to ambient air, soil and water / kg 0
END OF LIFE SCENARIO DOCUMENTATION
Scenario information Value
Collection process – kg collected separately 0
Collection process – kg collected with mixed
construction waste 2272
Recovery process – kg for re-use 0
Recovery process – kg for recycling 1.59E+03
Recovery process – kg for energy recovery 0
Disposal (total) – kg for final deposition 6.82E+02
Scenario assumptions e.g. transportation Market for transport, freight, lorry >32 metric ton,
EURO5; 50km

-- 12 of 13 --

13	Created with One Click LCA N50/20 Xencrete
THIRD-PARTY VERIFICATION STATEMENT
EPD Hub declares that this EPD is verified in accordance with ISO 14025 by an independent. third-party verifier. The
project report on the Life Cycle Assessment and the report(s) on features of environmental relevance are filed at EPD
Hub. EPD Hub PCR and ECO Platform verification checklist are used.
EPD Hub is not able to identify any unjustified deviations from the PCR and EN 15804+A2 in the Environmental Product
Declaration and its project report.
EPD Hub maintains its independence as a third-party body; it was not involved in the execution of the LCA or in the
development of the declaration and has no conflicts of interest regarding this verification.
The company-specific data and upstream and downstream data have been examined as regards plausibility and
consistency. The publisher is responsible for ensuring the factual integrity and legal compliance of this declaration.
Program assistant: Xinyuan Zhang
The software used in creation of this LCA and EPD is verified by EPD Hub to conform to the procedural and
methodological requirements outlined in ISO 14025:2010. ISO 14040/14044. EN 15804+A2. and EPD Hub Core Product
Category Rules and General Program Instructions.
Verified tools
Tool verifier: Imane Uald Lamkaddam
Tool verification validity: 28 March 2025 - 27 March 2028

-- 13 of 13 --

