1	Created with One Click LCA ATILTS4020100Enhanced
ENVIRONMENTAL PRODUCT DECLARATION
IN ACCORDANCE WITH EN 15804+A2 & ISO 14025
EPD HUB, HUB-5480
Published on 20.02.2026, last updated on 20.02.2026, valid until 19.02.2031
This EPD is intended for business-to-business and/or business-to-consumer communication. Life Cycle Assessment study has been performed in accordance with the
requirements of EN 15804, EPD Hub PCR version 1.2 (24 Mar 2025) and JRC characterization factors EF 3.1. The manufacturer has the sole ownership, liability, and responsibility
for the EPD. EPDs within the same product category but from different programs may not be comparable. EPDs of construction products may not be comparable if they do not
comply with EN 15804 and if they are not compared in a building context.
ATILTS4020100Enhanced
Tandy Concrete

-- 1 of 13 --

2	Created with One Click LCA ATILTS4020100Enhanced
MANUFACTURER AND SITE
Manufacturer Tandy Concrete
Address 21 Mackay Slade Point Road, Mackay,
Australia
Contact details sales@tandygroup.com.au
Website www.tandygroup.com.au
Place of production 21 Mackay Slade Point Road, Mackay,
Australia
Place(s) of raw
material origin
Mackay, Australia
Place(s) of
installation and use
Mackay, Australia
Period for data 1st July 2024 to 30th June 2025
EPD STANDARDS, SCOPE AND VERIFICATION
Program operator EPD Hub, hub@epdhub.com
Reference standard EN 15804:2012+A2:2019/AC:2021
and ISO 14025
PCR EPD Hub Core PCR version 1.2, 24 Mar 2025
cPCR EN 16757 Product Category Rules for
concrete and concrete elements
Sector Construction product
Category of EPD Third party verified EPD
Parent EPD number -
Scope of the EPD Cradle to gate with options, A4-A5, and
modules C1-C4, D
EPD author Niki Jackson
EPD verification Independent verification of this EPD and
data, according to ISO 14025:
 Internal verification
 External verification
EPD verifier Vera Durão, as an authorised verifier acting
for EPD Hub Limited
PRODUCT SPECIFICATION
Product name ATILTS4020100Enhanced
Product reference -
Concrete type Ready-mix concrete
Product standards EN 206
Additional
characteristic -
GTIN (Global Trade Item
Number) -
NOBB (Norwegian
Building Product Database) -
A1-A3 Specific data
(%) 99
PRODUCT DESCRIPTION
Tandy 40MPa Tiltup up concrete is designed to comply
with the requirements of AS1379 - Specification and
supply of concrete. Our technical expertise ensures
that tilt up panels made with this concrete gain
sufficient early strength to enable their lifting and
placing without damage to the panel.
Application: Tilt Up Panels
PRODUCT CHARACTERISTICS
Compressive strength class:
S40
Strength evaluation days:
28 days
Exposure class:
B2
ENVIRONMENTAL DATA SUMMARY
Declared unit 1 cubic meter
Declared unit mass, kg 2408
GWP-total, A1-A3 (kg CO₂e) 280
GWP-fossil, A1-A3 (kg CO₂e) 280
Secondary material, inputs (%) 0,6
Secondary material, outputs (%) 70
Total energy use, A1-A3 (kWh) 215
Net freshwater use, A1-A3 (m3) 6,73E‐01

-- 2 of 13 --

3	Created with One Click LCA ATILTS4020100Enhanced
WHO WE ARE
Tandy Concrete is an independently family-owned
Australian pre-mixed concrete supply company proudly
established in 1968. As part of the Tandy Group
employing over 100 staff across Queensland. We have
grown to be become a trusted and reliable concrete
supplier throughout Central Queensland.
We supply high-quality pre-mix concrete produced to
Australian Standards ensuring our customers receive
consistent and reliable materials to all construction
applications. All raw materials are sourced from
trusted suppliers and meet or exceed the required
specifications.
We operate fixed concrete batch plants in Airlie Beach,
Mackay, Marian, Rockhampton and Yeppoon. We can
also provide mobile site plants for major projects and
remote locations. Our modern well-maintained
transport fleet ensures we can confidently meet the
evolving needs of our customers.
We offer a full range of concrete products including not
limited to:
• N & S Grade (20–50+ MPa)
• Flowable fill
• Stabilised sands
• Block fills
• Spray mixes
• Shotcrete
Our fixed and mobile plants are supported by modern
fleet of agitator trucks, including six-metre, nine-metre
and mini agitators. These trucks can be moved from
any of sites to meet the specific needs of each project.
Through vertical integration Tandy Group also own and
operate TMR approved hard rock quarries and multiple
sand plants allowing us to maintain consistent quality,
dependable supply and competitive pricing.
Tandy Concrete has contributed to numerous
significant projects including but not limited to:
Project Name: Location:
Catherine McAuley Mackay
Resource Centre of Excellence Mackay
Jenmar Mackay
Richglen Mackay
Aldi Mackay/Airlie
Shute Harbour Units Airlie Beach
Followmont Transport Mackay
Hastings Deering Stage 2 Mackay
Bunnings Stores Mackay
Hastings Deering Stage 1 Mackay
Alliance Aircraft Hanger Rockhampton
Project Name: Location:
Mental Health Unit Rockhampton
St Brendan’s College Yeppoon
Edge Apartments 12 Story Rockhampton
Echelon Apartments 9 Story Rockhampton
Hospital Bridge Mackay
Gargett Bridge Gargett
Hay Point Expansion – HPX 3 Hay Point
We are equally proud to support local builders
delivering high quality concrete solutions for
residential, commercial, and civil applications across
the region.
QUALITY MANAGEMENT
Tandy Concrete is committed to maintaining the
highest standards of quality across all operations. Our
quality management processes ensure every load of
concrete meets industry, regulatory, and customer
requirements.
Our Quality Assurance Measures
Regular Raw Material Testing
All raw materials are tested regularly by external NATA-
certified laboratories to ensure compliance and
performance.
Approved Material Sources
All aggregates and raw materials used in concrete
production are sourced exclusively from Department of
Transport & Main Roads (DTMR) source assessed sites.
Compliance with Australian Standards
All concrete is manufactured in accordance with
Australian Standard AS 1379 and all cement powders
and chemical additives comply with their respective
Australian Standards.
Documented Mix Designs
Every batch is produced to approved mix designs with
detailed records of all additives logged, stored, and
traceable in our Axi batch software.
Plant Calibration
All concrete plants undergo full weights and measures
recalibration every six months by NATA-accredited
calibrators.
Fleet & Insurance
Our transport fleet is fully insured, including $30
million third-party property damage coverage.

-- 3 of 13 --

4	Created with One Click LCA ATILTS4020100Enhanced
INNOVATION & CONTINUOUS IMPROVEMENT
Innovation has always been integral to the way we op-
erate. Over the years Tandy Concrete has delivered
many industry firsts, driven by our willingness to ex-
plore new solutions rather than limiting the services
we provide. We continually invest in research, testing,
and collaboration to ensure our products meet the
evolving needs of our customers and the industries we
support.
Recent examples of our innovative concrete solutions
include:
High-strength underwater concrete:
A specialized liquid concrete mix designed with an anti-
washout admixture capable of being pumped 20
meters underwater while maintaining structural
integrity. This mix was developed for pylon
remediation works in the Ocean at Hay Point Coal
Terminal.
High-performance fiber-reinforced mix:
A custom fiber concrete mix design that delivered both
exceptional strength and superior finish ability
engineered specifically for super-flat flooring
applications during the Hastings Deering robotic pallet
racking up-grade.
Lightweight concrete utilizing polystyrene beads:
A carefully engineered lightweight mix incorporating
expanded polystyrene beads to significantly reduce
density and overall concrete weight. This solution is
ideal for projects requiring lower loading on existing
concrete structures, enabling safe upgrades and
extensions without compromising structural
performance. This mix was developed for a
multimillion-dollar waterfront mansion on Airlie
Beaches waterfront.
These projects demonstrate our commitment to
pushing boundaries, solving complex challenges, and
delivering tailored solutions that meet the highest
technical standards.
CONCLUSION
Tandy Concrete remains committed to delivering high-
performing concrete solutions backed by reliability,
technical expertise, and a genuine focus on customer
success. With a strong regional footprint, integrated
supply chain, and an ongoing drive for innovation we
continue to support Central Queensland’s growth
providing the foundations for projects of every scale.
Our history, capability, and dedication ensure we are
well positioned to meet the challenges of today and
the opportunities of tomorrow.

-- 4 of 13 --

5	Created with One Click LCA ATILTS4020100Enhanced
LIFE CYCLE ASSESSMENT
SYSTEM BOUNDARY
This EPD covers the life-cycle modules listed in the
following table.
Product stage
Assembly stage
Use stage
End of life stage
Beyond the system
boundaries
A1 A2 A3 A4 A5 B1 B2 B3 B4 B5 B6 B7 C1 C2 C3 C4 D
x x x x x N
D
N
D
N
D
N
D
N
D
N
D
N
D x x x x x
Raw materials	
Transport	
Manufacturing	
Transport	
Assembly	
Use
Maintenance	
Repair
Replacement	
Refurbishment	
Operational energy	
use	
Operational water	
use	
Deconstr./demol.	
Transport	
Waste processing	
Disposal
Reuse, Recovery,	
Recycling
Not declared = ND.
CUT-OFF CRITERIA
The study does not exclude any modules or processes
which are stated mandatory in the reference standard
and the applied PCR. The study does not exclude any
hazardous materials or substances. There is no
neglected unit process more than 1% of total mass or
energy flows. The module specific total neglected input
and output flows also do not exceed 5% of energy
usage or mass.
The production of capital equipment, construction
activities, and infrastructure, maintenance and
operation of capital equipment, personnel-related
activities, energy and water use related to company
management and sales activities are excluded.
VALIDATION OF DATA
Data collection for production, transport, and packaging
was conducted using time and site-specific information,
as defined in the general information section on page 1
and 2. Upstream process calculations rely on generic
data as defined in the Bibliography section.
Manufacturer-provided specific and generic data were
used for the product’s manufacturing stage. The
analysis was performed in One Click LCA EPD
Generator, with the 'Cut-Off, EN 15804+A2' allocation
method, and characterization factors according to EN
15804:2012+A2:2019/AC:2021 and JRC EF 3.1.
ALLOCATION, ESTIMATES AND ASSUMPTIONS
All allocations are done as per the reference standards
and the applied PCR. In this study, allocation has been
done in the following ways:
Data type Allocation
Raw materials No allocation
Packaging materials Not applicable
Ancillary materials Allocated by mass
Manufacturing energy and waste Allocated by mass
• Economic allocation has been applied to the fly ash in
the upstream generic process
• Fuel used for mixing 1m3 of concrete was
determined based on a 10-minute mixing time of the
average load size of 6.2m3, for diesel burned in the full
mixing mode of the concrete agitator barrel
• A market-based approach is used in modelling the
electricity mix utilised in the factory. Renewables have
been removed to provide a conservative approach,
with electricity being less than 0.3% of the total
impact; this would have very little impact on the results
• Distribution Loss Factor (DLF) of 1.033 was applied to
the electricity
• Electricity is composed of 81.10% Coal, 16.66% Gas
and 2.24% Oil
• Transport factors for raw materials, Aggregates 31-
54km, Admixtures 950-980km, Cement 430-450km
• A4, Distance of 11km is assumed
• A5, 3% waste, and 73.62MJ of diesel consumed
PRODUCT & MANUFACTURING SITES GROUPING
Type of grouping No grouping
Grouping method Not applicable
Variation in GWP-fossil for A1-A3, % -
This EPD is product and factory specific.
PRODUCT RAW MATERIAL MAIN COMPOSITION
The product is a ready-mix concrete consisting of
aggregates, cement, filler, admixtures, and water. Main
material categories as per EPD Hub GPI are shown
below:
Raw material
category
Amount, mass- % Material origin
Metals 0 -
Minerals 100 Australia
Fossil materials 0 -
Bio-based materials 0 -

-- 5 of 13 --

6	Created with One Click LCA ATILTS4020100Enhanced
SUBSTANCES, REACH - VERY HIGH CONCERN
The product does not contain any REACH SVHC
substances in amounts greater than 0,1 % (1000 ppm).
BIOGENIC CARBON CONTENT
Product’s biogenic carbon content at the factory gate
Biogenic carbon content in product, kg C 0

-- 6 of 13 --

7	Created with One Click LCA ATILTS4020100Enhanced
PRODUCT LIFE CYCLE
MANUFACTURING (A1-A3)
The environmental impacts considered for the product
stage cover the manufacturing of raw materials used in
the production. Also, fuels used by machines, and
handling of waste formed in the production processes
at the manufacturing facilities are included in this
stage. The study also considers the material losses
occurring during the manufacturing processes as well
as losses during electricity transmission.
The use of green energy in manufacturing is
demonstrated through contractual instruments (GOs,
RECs, etc.), and its use is ensured throughout the
validity period of this EPD.
Ready-mix concrete production starts by transporting
the binders, aggregates, and additives to the
manufacturing site and storing them into closed silos
and containers. The aggregates are then dosed onto a
scale and transferred to a concrete mixer. In the mixer,
cement is added to the aggregates, after which the
material is mixed dry. Water and additives are then
added to the mixture, followed by wet mixing. After
mixing, the concrete mass is unloaded from the mixer
into the tank of the concrete mixer truck, which is
transported to the construction site.
No packaging is included as the product is transported
with mixer trucks.
TRANSPORT AND INSTALLATION (A4-A5)
The concrete is transported to the building site using
an average lorry. Transportation impacts occurred from
final products delivery to construction site cover fuel
direct exhaust emissions, environmental impacts of
fuel production, as well as related infrastructure
emissions (A4).
Installation includes the energy used for concrete
application. This consists of the energy spent by a
concrete mixer truck and a concrete pump. A
production loss of % at installation is assumed (A5).
PRODUCT USE AND MAINTENANCE (B1-B7)
This EPD does not cover the use phase. Air, soil, and
water impacts during the use phase have not been
studied. Carbonation is not taken into account in this
EPD.
PRODUCT END OF LIFE (C1-C4, D)
At the end of its life, the concrete is assumed to be part
of a concrete building that is demolished using
machinery, consuming energy in the form of diesel
(C1).
The concrete blocks gotten after the demolition are
delivered 50 km by a lorry to the nearest construction
waste treatment (C2). It is assumed that 100% of the
demolished concrete is transported to a site where this
waste is processed by, crushing the blocks to gravel.
About 70% of concrete can be recycled this way (C3),
with an assumption that non-reinforced concrete is
being sorted. The remaining 30% of concrete is
assumed to be sent to the landfill for disposal (C4). The
crushed concrete received from waste treatment can
be used as a replacement for virgin gravel or for raw
materials in road construction (D). The process losses
of the waste treatment plant are assumed to be
negligible.
LCA SOFTWARE AND BIBLIOGRAPHY
This EPD has been created using One Click LCA
Concrete EPD Generator v3.2.1. The LCA and EPD have
been prepared according to the reference standards
and ISO 14040/14044. Ecoinvent v3.10.1/3.11 and One
Click LCA databases were used as sources of
environmental data. Allocation used in Ecoinvent
3.10.1/3.11 environmental data sources follow the
methodology ‘allocation, cut-off, EN 15804+A2‘.
AS 1379 2007 - Specification and supply of concrete
AS 3600 2018 - Concrete Structures, Table 4.4
Australian energy statistics 2025 - Table O, Australian
electricity generation, by state and territory, by fuel
type, physical units.
https://www.energy.gov.au/publications/australian-
energy-update-2025
Australian Energy Market Operator - Distribution Loss
Factors For The 2024/25 Financial Year.
https://www.aemo.com.au/-
/media/files/electricity/nem/security_and_reliability/lo
ss_factors_and_regional_boundaries/2024-25-
financial-year/distribution-loss-factors-for-2024-25.pdf
Diesel used in the mixing of concrete. https://unique-
mixer.com/news/How_much_diesel_does_a_self_loadi
ng_concrete_mixer_consume_per_hour.html
3

-- 7 of 13 --

8	Created with One Click LCA ATILTS4020100Enhanced
MANUFACTURING PROCESS DIAGRAM (A1-A3)

-- 8 of 13 --

9 ATILTS4020100Enhanced	Created with One Click LCA
ENVIRONMENTAL IMPACT DATA
The estimated impact results are only relative statements which do not indicate the end points of the impact categories, exceeding threshold values, safety margins or risks.
CORE ENVIRONMENTAL IMPACT INDICATORS – EN 15804+A2, EF 3.1
Impact category Unit A1 A2 A3 A1-A3 A4 A5 B1 B2 B3 B4 B5 B6 B7 C1 C2 C3 C4 D
GWP – total1) kg CO2e 2,59E+02 1,77E+01 3,39E+00 2,80E+02 2,85E+00 1,66E+01 ND ND ND ND ND ND ND 4,58E+00 1,30E+01 7,38E+00 4,51E+00 ‐1,35E+01
GWP – fossil kg CO2e 2,59E+02 1,77E+01 3,39E+00 2,80E+02 2,85E+00 1,66E+01 ND ND ND ND ND ND ND 4,58E+00 1,30E+01 7,38E+00 4,51E+00 ‐1,35E+01
GWP – biogenic kg CO2e ‐3,32E‐02 8,29E‐03 3,75E‐04 ‐2,46E‐02 6,46E‐04 5,64E‐05 ND ND ND ND ND ND ND 4,67E‐04 2,94E‐03 ‐7,53E‐04 ‐1,43E‐03 ‐4,24E‐02
GWP – LULUC kg CO2e 1,58E‐02 1,34E‐02 3,31E‐04 2,96E‐02 1,28E‐03 1,95E‐03 ND ND ND ND ND ND ND 4,69E‐04 5,80E‐03 7,56E‐04 2,58E‐03 ‐1,87E‐02
Ozone depletion pot. kg CFC-11e 2,98E‐06 2,31E‐07 5,33E‐08 3,27E‐06 4,21E‐08 2,25E‐07 ND ND ND ND ND ND ND 7,01E‐08 1,91E‐07 1,13E‐07 1,31E‐07 ‐1,13E‐06
Acidification potential mol H+e 9,42E‐01 1,11E‐01 2,73E‐02 1,08E+00 9,72E‐03 1,04E‐01 ND ND ND ND ND ND ND 4,14E‐02 4,42E‐02 6,66E‐02 3,20E‐02 ‐8,83E‐02
EP-freshwater2) kg Pe 4,40E‐02 2,34E‐03 2,35E‐04 4,66E‐02 2,22E‐04 1,67E‐03 ND ND ND ND ND ND ND 1,32E‐04 1,01E‐03 2,13E‐04 3,71E‐04 ‐7,99E‐04
EP-marine kg Ne 4,56E‐02 4,22E‐02 1,09E‐02 9,87E‐02 3,19E‐03 3,57E‐02 ND ND ND ND ND ND ND 1,92E‐02 1,45E‐02 3,09E‐02 1,22E‐02 ‐1,91E‐02
EP-terrestrial mol Ne 2,22E+00 4,59E‐01 1,19E‐01 2,80E+00 3,48E‐02 4,42E‐01 ND ND ND ND ND ND ND 2,10E‐01 1,58E‐01 3,38E‐01 1,33E‐01 ‐2,50E‐01
POCP (“smog”)3) kg
NMVOCe 5,31E‐01 1,45E‐01 3,57E‐02 7,12E‐01 1,43E‐02 1,29E‐01 ND ND ND ND ND ND ND 6,26E‐02 6,51E‐02 1,01E‐01 4,77E‐02 ‐6,41E‐02
ADP-minerals & metals4) kg Sbe 2,03E‐05 4,72E‐05 1,27E‐06 6,88E‐05 7,95E‐06 6,32E‐06 ND ND ND ND ND ND ND 1,64E‐06 3,62E‐05 2,64E‐06 7,16E‐06 ‐1,36E‐04
ADP-fossil resources MJ 3,88E+02 2,38E+02 4,37E+01 6,69E+02 4,14E+01 1,30E+02 ND ND ND ND ND ND ND 5,99E+01 1,88E+02 9,65E+01 1,11E+02 ‐2,01E+02
Water use5) m3e depr. 4,73E+01 1,91E+00 7,24E+00 5,65E+01 2,04E‐01 1,99E+00 ND ND ND ND ND ND ND 1,50E‐01 9,29E‐01 2,41E‐01 3,19E‐01 ‐2,67E+01
1) GWP = Global Warming Potential. 2) EP = Eutrophication potential. Required characterisation method and data are in kg P-eq. Multiply by 3,07 to get PO4e. 3) POCP = Photochemical ozone formation. 4) ADP = Abiotic depletion potential.
5) EN 15804+A2 disclaimer for Abiotic depletion and Water use and optional indicators except Particulate matter and Ionizing radiation, human health. The results of these environmental impact indicators shall be used with care as the
uncertainties on these results are high or as there is limited experience with the indicator.
removalMarker-pef1

-- 9 of 13 --

10 ATILTS4020100Enhanced	Created with One Click LCA
ADDITIONAL (OPTIONAL) ENVIRONMENTAL IMPACT INDICATORS – EN 15804+A2, EF 3.1
Impact category Unit A1 A2 A3 A1-A3 A4 A5 B1 B2 B3 B4 B5 B6 B7 C1 C2 C3 C4 D
Particulate matter Incidence 7,52E‐06 2,09E‐06 7,53E‐07 1,04E‐05 2,85E‐07 2,70E‐06 ND ND ND ND ND ND ND 1,18E‐06 1,30E‐06 1,44E‐05 7,28E‐07 ‐1,13E‐06
Ionizing radiation6) kBq
U235e 8,46E+02 4,70E‐01 2,72E‐02 8,46E+02 3,60E‐02 2,54E+01 ND ND ND ND ND ND ND 2,65E‐02 1,64E‐01 4,27E‐02 6,96E‐02 ‐3,19E+00
Ecotoxicity (freshwater) CTUe 4,02E+02 4,23E+01 3,68E+00 4,48E+02 5,85E+00 2,02E+01 ND ND ND ND ND ND ND 3,30E+00 2,66E+01 5,31E+00 9,28E+00 ‐2,41E+02
Human toxicity, cancer CTUh 4,18E‐07 3,69E‐09 3,15E‐10 4,22E‐07 4,71E‐10 1,35E‐08 ND ND ND ND ND ND ND 4,71E‐10 2,14E‐09 7,58E‐10 8,31E‐10 ‐1,40E‐08
Human tox. non-cancer CTUh 1,30E‐05 1,38E‐07 9,20E‐09 1,31E‐05 2,68E‐08 4,12E‐07 ND ND ND ND ND ND ND 7,46E‐09 1,22E‐07 1,20E‐08 1,91E‐08 ‐2,57E‐07
SQP7) - 7,39E+02 1,94E+02 6,09E+00 9,39E+02 4,17E+01 4,86E+01 ND ND ND ND ND ND ND 4,20E+00 1,89E+02 6,76E+00 2,18E+02 ‐1,93E+02
6) EN 15804+A2 disclaimer for Ionizing radiation, human health. This impact category deals mainly with the eventual impact of low dose ionizing radiation on human health of the nuclear fuel cycle. It does not consider effects due to
possible nuclear accidents, occupational exposure nor due to radioactive waste disposal in underground facilities. Potential ionizing radiation from the soil, from radon and from some construction materials is also not measured by this
indicator. 7) SQP = Land use related impacts/soil quality.
removalMarker-pef2
USE OF NATURAL RESOURCES
Impact category Unit A1 A2 A3 A1-A3 A4 A5 B1 B2 B3 B4 B5 B6 B7 C1 C2 C3 C4 D
Renew. PER as energy8) MJ 1,35E+01 7,65E+00 3,13E‐01 2,15E+01 5,67E‐01 1,40E+00 ND ND ND ND ND ND ND 3,80E‐01 2,58E+00 6,11E‐01 1,07E+00 ‐1,98E+01
Renew. PER as material MJ 0,00E+00 0,00E+00 0,00E+00 0,00E+00 0,00E+00 0,00E+00 ND ND ND ND ND ND ND 0,00E+00 0,00E+00 0,00E+00 0,00E+00 0,00E+00
Total use of renew. PER MJ 1,35E+01 7,65E+00 3,13E‐01 2,15E+01 5,67E‐01 1,40E+00 ND ND ND ND ND ND ND 3,80E‐01 2,58E+00 6,11E‐01 1,07E+00 ‐1,98E+01
Non-re. PER as energy MJ 3,72E+02 2,38E+02 4,38E+01 6,54E+02 4,14E+01 1,29E+02 ND ND ND ND ND ND ND 5,99E+01 1,88E+02 9,65E+01 1,11E+02 ‐2,06E+02
Non-re. PER as material MJ 0,00E+00 0,00E+00 0,00E+00 0,00E+00 0,00E+00 0,00E+00 ND ND ND ND ND ND ND 0,00E+00 0,00E+00 0,00E+00 0,00E+00 0,00E+00
Total use of non-re. PER MJ 3,72E+02 2,38E+02 4,38E+01 6,54E+02 4,14E+01 1,29E+02 ND ND ND ND ND ND ND 5,99E+01 1,88E+02 9,65E+01 1,11E+02 ‐2,06E+02
Secondary materials kg 1,45E+01 2,18E‐01 1,41E‐02 1,47E+01 1,76E‐02 4,87E‐01 ND ND ND ND ND ND ND 2,49E‐02 8,01E‐02 4,01E‐02 2,78E‐02 ‐2,32E‐01
Renew. secondary fuels MJ 1,19E‐06 1,25E‐03 4,84E‐05 1,29E‐03 2,24E‐04 2,01E‐04 ND ND ND ND ND ND ND 6,51E‐05 1,02E‐03 1,05E‐04 5,76E‐04 ‐1,60E‐03
Non-ren. secondary
fuels MJ 9,98E+01 0,00E+00 0,00E+00 9,98E+01 0,00E+00 2,99E+00 ND ND ND ND ND ND ND 0,00E+00 0,00E+00 0,00E+00 0,00E+00 0,00E+00
Use of net fresh water m3 6,07E‐01 5,02E‐02 1,50E‐02 6,73E‐01 6,12E‐03 3,12E‐02 ND ND ND ND ND ND ND 3,96E‐03 2,78E‐02 6,38E‐03 1,15E‐01 ‐6,21E‐01
8) PER = Primary energy resources.

-- 10 of 13 --

11 ATILTS4020100Enhanced	Created with One Click LCA
END OF LIFE – WASTE
Impact category Unit A1 A2 A3 A1-A3 A4 A5 B1 B2 B3 B4 B5 B6 B7 C1 C2 C3 C4 D
Hazardous waste kg 2,62E+00 7,81E‐01 3,90E‐02 3,44E+00 7,01E‐02 2,29E‐01 ND ND ND ND ND ND ND 6,67E‐02 3,19E‐01 1,07E‐01 1,22E‐01 ‐1,56E+00
Non-hazardous waste kg 5,03E+01 1,36E+01 6,05E‐01 6,45E+01 1,30E+00 3,74E+00 ND ND ND ND ND ND ND 9,09E‐01 5,90E+00 1,46E+00 2,79E+00 ‐2,90E+01
Radioactive waste kg 6,66E‐04 1,15E‐04 5,52E‐06 7,87E‐04 8,82E‐06 3,64E‐05 ND ND ND ND ND ND ND 6,51E‐06 4,01E‐05 1,05E‐05 1,70E‐05 ‐3,99E‐04
END OF LIFE – OUTPUT FLOWS
Impact category Unit A1 A2 A3 A1-A3 A4 A5 B1 B2 B3 B4 B5 B6 B7 C1 C2 C3 C4 D
Components for re-use kg 0,00E+00 0,00E+00 0,00E+00 0,00E+00 0,00E+00 0,00E+00 ND ND ND ND ND ND ND 0,00E+00 0,00E+00 0,00E+00 0,00E+00 0,00E+00
Materials for recycling kg 0,00E+00 0,00E+00 1,50E+01 1,50E+01 0,00E+00 5,10E+01 ND ND ND ND ND ND ND 0,00E+00 0,00E+00 1,69E+03 0,00E+00 0,00E+00
Materials for energy rec Kg 0,00E+00 0,00E+00 0,00E+00 0,00E+00 0,00E+00 0,00E+00 ND ND ND ND ND ND ND 0,00E+00 0,00E+00 0,00E+00 0,00E+00 0,00E+00
Exported energy MJ 0,00E+00 0,00E+00 0,00E+00 0,00E+00 0,00E+00 0,00E+00 ND ND ND ND ND ND ND 0,00E+00 0,00E+00 0,00E+00 0,00E+00 0,00E+00
Exported energy:
Electricity MJ 0,00E+00 0,00E+00 0,00E+00 0,00E+00 0,00E+00 0,00E+00 ND ND ND ND ND ND ND 0,00E+00 0,00E+00 0,00E+00 0,00E+00 0,00E+00
Exported energy: Heat MJ 0,00E+00 0,00E+00 0,00E+00 0,00E+00 0,00E+00 0,00E+00 ND ND ND ND ND ND ND 0,00E+00 0,00E+00 0,00E+00 0,00E+00 0,00E+00
ENVIRONMENTAL IMPACTS – EN 15804+A1, CML
Impact category Unit A1 A2 A3 A1-A3 A4 A5 B1 B2 B3 B4 B5 B6 B7 C1 C2 C3 C4 D
Global Warming Pot. kg CO2e 2,59E+02 1,76E+01 3,37E+00 2,80E+02 2,84E+00 1,66E+01 ND ND ND ND ND ND ND 4,56E+00 1,29E+01 7,34E+00 4,47E+00 ‐1,67E+01
Ozone depletion Pot. kg CFC-11e 1,09E‐06 1,85E‐07 4,35E‐08 1,32E‐06 3,36E‐08 1,40E‐07 ND ND ND ND ND ND ND 5,56E‐08 1,53E‐07 8,95E‐08 1,04E‐07 ‐1,15E‐07
Acidification kg SO2e 7,81E‐02 8,27E‐02 2,00E‐02 1,81E‐01 7,42E‐03 5,56E‐02 ND ND ND ND ND ND ND 2,91E‐02 3,37E‐02 4,68E‐02 2,37E‐02 ‐8,03E‐02
Eutrophication kg PO43e 4,75E‐02 1,81E‐02 4,39E‐03 7,00E‐02 1,81E‐03 1,39E‐02 ND ND ND ND ND ND ND 6,79E‐03 8,22E‐03 1,09E‐02 7,52E‐03 ‐1,58E‐02
POCP (“smog”) kg C2H4e 6,85E‐03 6,46E‐03 1,36E‐03 1,47E‐02 6,62E‐04 4,23E‐03 ND ND ND ND ND ND ND 2,18E‐03 3,01E‐03 3,51E‐03 2,24E‐03 ‐7,15E‐03
ADP-elements kg Sbe 2,03E‐05 4,60E‐05 1,23E‐06 6,75E‐05 7,76E‐06 6,17E‐06 ND ND ND ND ND ND ND 1,60E‐06 3,53E‐05 2,57E‐06 7,02E‐06 ‐9,16E‐05
ADP-fossil MJ 3,86E+02 2,31E+02 4,34E+01 6,60E+02 4,08E+01 1,28E+02 ND ND ND ND ND ND ND 5,95E+01 1,85E+02 9,58E+01 1,10E+02 ‐2,06E+02

-- 11 of 13 --

12 ATILTS4020100Enhanced	Created with One Click LCA
ADDITIONAL INDICATOR – GWP-GHG
Impact category Unit A1 A2 A3 A1-A3 A4 A5 B1 B2 B3 B4 B5 B6 B7 C1 C2 C3 C4 D
GWP-GHG 9) kg CO2e 2,59E+02 1,77E+01 3,39E+00 2,80E+02 2,85E+00 1,66E+01 ND ND ND ND ND ND ND 4,58E+00 1,30E+01 7,38E+00 4,51E+00 ‐1,35E+01
9) This indicator includes all greenhouse gases excluding biogenic carbon dioxide uptake and emissions and biogenic carbon stored in the product. In addition, the characterisation factors for the flows - CH4 fossil, CH4 biogenic and Dinitrogen
monoxide - were updated. This indicator is identical to the GWP-total of EN 15804:2012+A2:2019 except that the characterization factor for biogenic CO2 is set to zero.
SCENARIO DOCUMENTATION
DATA SOURCES
Manufacturing energy scenario documentation – A3 (Energy data source)
1. Construction, specialized activities, demolition and site preparation, Diesel, burned in building machine,
World, ecoinvent 3.10.1, 0.10 kgCO2e/MJ
2. Electricity, Electricity, consumption mix w/o renewables, Queensland, 2024, Australia, LCA study for
country specific consumption mixes, OneClickLCA 2025, 1.08 kgCO2e/kWh
Installation scenario documentation - A5 (Diesel consumption)
1. Diesel, burned in building machine, World, ecoinvent 3.10.1, 0.1 kg CO2e/MJ
TRANSPORT SCENARIO DOCUMENTATION - A4
Scenario parameter Value
Vehicle type used for transport (e.g., long distance
truck, boat, etc.) / Vehicle type, Commission
Directive 2007/37/EC (European Emission Standard)
Concrete mixer truck
Distance, km 11
Capacity utilization (including empty return) % 50 %
Bulk density of transported products / kg/m3 2,41E+03
Volume capacity utilization factor (factor: =1 or <1 or
≥1 for compressed or nested packaged products) 1
INSTALLATION SCENARIO DOCUMENTATION - A5
Scenario parameter Value
Ancillary materials for installation (specified by
material) / kg or other units as appropriate 0
Water use / m³ 0
Other resource use / kg 0
Waste materials on the building site before waste
processing, generated by the product's installation
(specified by type) / kg
7,22E+01
Output materials as result of waste processing at the
building site e.g. collection for recycling / kg 5,06E+01
Output materials as result of waste processing at the
building site e.g. collection for disposal / kg 2,17E+01
Direct emissions to ambient air, soil and water / kg 0
END OF LIFE SCENARIO DOCUMENTATION
Scenario information Value
Collection process – kg collected separately 0
Collection process – kg collected with mixed
construction waste 2408
Recovery process – kg for re-use 0
Recovery process – kg for recycling 1,69E+03
Recovery process – kg for energy recovery 0
Disposal (total) – kg for final deposition 7,22E+02
Scenario assumptions e.g. transportation Market for transport, freight, lorry >32 metric ton,
EURO5; 50km

-- 12 of 13 --

13	Created with One Click LCA ATILTS4020100Enhanced
THIRD-PARTY VERIFICATION STATEMENT
EPD Hub declares that this EPD is verified in accordance with ISO 14025 by an independent, third-party verifier. The
project report on the Life Cycle Assessment and the report(s) on features of environmental relevance are filed at EPD
Hub. EPD Hub PCR and ECO Platform verification checklist are used.
EPD Hub is not able to identify any unjustified deviations from the PCR and EN 15804+A2 in the Environmental Product
Declaration and its project report.
EPD Hub maintains its independence as a third-party body; it was not involved in the execution of the LCA or in the
development of the declaration and has no conflicts of interest regarding this verification.
The company-specific data and upstream and downstream data have been examined as regards plausibility and
consistency. The publisher is responsible for ensuring the factual integrity and legal compliance of this declaration.
Program assistant: Xinyuan Zhang
The software used in creation of this LCA and EPD is verified by EPD Hub to conform to the procedural and
methodological requirements outlined in ISO 14025:2010, ISO 14040/14044, EN 15804+A2, and EPD Hub Core Product
Category Rules and General Program Instructions.
Verified tools
Tool verifier: Imane Uald Lamkaddam
Tool verification validity: 28 March 2025 - 27 March 2028

-- 13 of 13 --

